updated_kvs instead of s', renamed tm to cl and km to svr

txn-data-consistency/Serializable_2PC_2PL.thy
@@ -8,25 +8,25 @@ subsection \<open>2PC Event system & Refinement from ET_ES to tps\<close>
 
 subsubsection \<open>State\<close>
 
-datatype state_km = working | prepared | read_lock | write_lock | no_lock | notokay | committed | aborted
-datatype state_tm = tm_init | tm_prepared | tm_committed | tm_aborted
+datatype state_svr = working | prepared | read_lock | write_lock | no_lock | notokay | committed | aborted
+datatype state_cl = cl_init | cl_prepared | cl_committed | cl_aborted
 
 \<comment>\<open>Client State\<close>
-record cl_state =
-  tm_state :: state_tm
+record cl_conf =
+  cl_state :: state_cl
   cl_sn :: nat
   cl_view :: view
 
 \<comment>\<open>Server State\<close>
-record 'v svr_state =
-  km_state :: "txid0 \<Rightarrow> state_km"
+record 'v svr_conf =
+  svr_state :: "txid0 \<Rightarrow> state_svr"
   svr_vl :: "'v v_list"
   svr_key_fp :: "txid0 \<Rightarrow> 'v key_fp"
 
 \<comment>\<open>System Global State: Clients and key Servers\<close>
 record 'v global_state =
-  cls :: "cl_id \<Rightarrow> cl_state"
-  svrs :: "key \<Rightarrow> 'v svr_state"
+  cls :: "cl_id \<Rightarrow> cl_conf"
+  svrs :: "key \<Rightarrow> 'v svr_conf"
 
 \<comment> \<open>Translator functions\<close>
 
@@ -35,36 +35,36 @@ abbreviation get_txn_cl :: "cl_id \<Rightarrow> 'v global_state \<Rightarrow> tx
 
 subsubsection \<open>Simulation function\<close>
 
-abbreviation eligible_reads :: "(txid0 \<Rightarrow> state_tm) \<Rightarrow> (txid0 \<Rightarrow> state_km) \<Rightarrow>
+abbreviation eligible_reads :: "(txid0 \<Rightarrow> state_cl) \<Rightarrow> (txid0 \<Rightarrow> state_svr) \<Rightarrow>
   (txid0 \<Rightarrow> 'v key_fp) \<Rightarrow> txid0 \<Rightarrow> bool" where
-  "eligible_reads tStm tSkm tFk t \<equiv>
-    tStm t = tm_committed \<and> tSkm t \<in> {read_lock, write_lock} \<and> tFk t R \<noteq> None"
+  "eligible_reads tCls tSvrs tFk t \<equiv>
+    tCls t = cl_committed \<and> tSvrs t \<in> {read_lock, write_lock} \<and> tFk t R \<noteq> None"
 
-definition update_kv_reads_all_txn :: "(txid0 \<Rightarrow> state_tm) \<Rightarrow> (txid0 \<Rightarrow> state_km) \<Rightarrow>
+definition update_kv_reads_all_txn :: "(txid0 \<Rightarrow> state_cl) \<Rightarrow> (txid0 \<Rightarrow> state_svr) \<Rightarrow>
   (txid0 \<Rightarrow> 'v key_fp) \<Rightarrow> 'v v_list \<Rightarrow> 'v v_list" where
-  "update_kv_reads_all_txn tStm tSkm tFk vl =
+  "update_kv_reads_all_txn tCls tSvrs tFk vl =
     (let uk = full_view vl; lv = last_version vl uk in
-     vl [Max uk := lv \<lparr>v_readerset := (v_readerset lv) \<union> {t. eligible_reads tStm tSkm tFk t}\<rparr>])"
+     vl [Max uk := lv \<lparr>v_readerset := (v_readerset lv) \<union> {t. eligible_reads tCls tSvrs tFk t}\<rparr>])"
 
-abbreviation the_wr_t :: "(txid0 \<Rightarrow> state_km) \<Rightarrow> txid0" where
-  "the_wr_t tSkm \<equiv> (THE t. tSkm t = write_lock)"
+abbreviation the_wr_t :: "(txid0 \<Rightarrow> state_svr) \<Rightarrow> txid0" where
+  "the_wr_t tSvrs \<equiv> (THE t. tSvrs t = write_lock)"
 
-definition update_kv_writes_all_txn :: "(txid0 \<Rightarrow> state_tm) \<Rightarrow> (txid0 \<Rightarrow> state_km) \<Rightarrow>
+definition update_kv_writes_all_txn :: "(txid0 \<Rightarrow> state_cl) \<Rightarrow> (txid0 \<Rightarrow> state_svr) \<Rightarrow>
   (txid0 \<Rightarrow> 'v key_fp) \<Rightarrow> 'v v_list \<Rightarrow> 'v v_list" where
-  "update_kv_writes_all_txn tStm tSkm tFk vl =
-    (if (\<exists>t. tStm t = tm_committed \<and> tSkm t = write_lock) then
-        update_kv_writes (the_wr_t tSkm) (tFk (the_wr_t tSkm)) vl
+  "update_kv_writes_all_txn tCls tSvrs tFk vl =
+    (if (\<exists>t. tCls t = cl_committed \<and> tSvrs t = write_lock) then
+        update_kv_writes (the_wr_t tSvrs) (tFk (the_wr_t tSvrs)) vl
      else vl)"
 
-definition update_kv_all_txn :: "(txid0 \<Rightarrow> state_tm) \<Rightarrow> (txid0 \<Rightarrow> state_km) \<Rightarrow>
+definition update_kv_all_txn :: "(txid0 \<Rightarrow> state_cl) \<Rightarrow> (txid0 \<Rightarrow> state_svr) \<Rightarrow>
   (txid0 \<Rightarrow> 'v key_fp) \<Rightarrow> 'v v_list \<Rightarrow> 'v v_list" where
-  "update_kv_all_txn tStm tSkm tFk =
-    (update_kv_writes_all_txn tStm tSkm tFk) o (update_kv_reads_all_txn tStm tSkm tFk)"
+  "update_kv_all_txn tCls tSvrs tFk =
+    (update_kv_writes_all_txn tCls tSvrs tFk) o (update_kv_reads_all_txn tCls tSvrs tFk)"
 
 definition kvs_of_gs :: "'v global_state \<Rightarrow> 'v kv_store" where
   "kvs_of_gs gs = (\<lambda>k.
-   update_kv_all_txn (\<lambda>t. tm_state (cls gs (get_cl_txn t)))
-    (km_state (svrs gs k)) (svr_key_fp (svrs gs k)) (svr_vl (svrs gs k)))"
+   update_kv_all_txn (\<lambda>t. cl_state (cls gs (get_cl_txn t)))
+    (svr_state (svrs gs k)) (svr_key_fp (svrs gs k)) (svr_vl (svrs gs k)))"
 
 definition views_of_gs :: "'v global_state \<Rightarrow> (cl_id \<Rightarrow> view)" where
   "views_of_gs gs = (\<lambda>cl. cl_view (cls gs cl))"
@@ -81,162 +81,171 @@ subsubsection \<open>Events\<close>
 
 datatype 'v ev = Prepare key txid0 | RLock key 'v txid0 | WLock key 'v "'v option" txid0 |
   NoLock key txid0 | NOK key txid0 | Commit key txid0 | Abort key txid0 |
-  User_Commit cl_id | TM_Commit cl_id sqn view "'v fingerpr"| TM_Abort cl_id | TM_ReadyC cl_id |
-  TM_ReadyA cl_id | Skip2
+  User_Commit cl_id | Cl_Commit cl_id sqn view "'v fingerpr"| Cl_Abort cl_id | Cl_ReadyC cl_id |
+  Cl_ReadyA cl_id | Skip2
 
-definition km_t'_unchanged where
-  "km_t'_unchanged t k svrss svrss' \<equiv> (\<forall>t'. t' \<noteq> t \<longrightarrow>
+definition svr_t'_unchanged where
+  "svr_t'_unchanged t k svrss svrss' \<equiv> (\<forall>t'. t' \<noteq> t \<longrightarrow>
      svr_key_fp (svrss' k) t' = svr_key_fp (svrss k) t' \<and>
-     km_state (svrss' k) t' = km_state (svrss k) t')"
+     svr_state (svrss' k) t' = svr_state (svrss k) t')"
 
 definition other_insts_unchanged where
   "other_insts_unchanged k svrss svrss' \<equiv> (\<forall>k'. k' \<noteq> k \<longrightarrow> svrss' k' = svrss k')"
 
-definition tm_km_k'_t'_unchanged where
-  "tm_km_k'_t'_unchanged k s s' t \<equiv> cls s' = cls s \<and>
-    other_insts_unchanged k (svrs s) (svrs s') \<and> km_t'_unchanged t k (svrs s) (svrs s')"
+definition cl_svr_k'_t'_unchanged where
+  "cl_svr_k'_t'_unchanged k s s' t \<equiv> cls s' = cls s \<and>
+    other_insts_unchanged k (svrs s) (svrs s') \<and> svr_t'_unchanged t k (svrs s) (svrs s')"
 
-definition km_tm_cl'_unchanged where
-  "km_tm_cl'_unchanged cl s s' \<equiv> svrs s' = svrs s \<and> other_insts_unchanged cl (cls s) (cls s')"
+definition svr_cl_cl'_unchanged where
+  "svr_cl_cl'_unchanged cl s s' \<equiv> svrs s' = svrs s \<and> other_insts_unchanged cl (cls s) (cls s')"
 
-lemmas km_unchanged_defs = tm_km_k'_t'_unchanged_def other_insts_unchanged_def km_t'_unchanged_def
-lemmas tm_unchanged_defs = km_tm_cl'_unchanged_def other_insts_unchanged_def
-lemmas unchanged_defs = km_unchanged_defs km_tm_cl'_unchanged_def
+lemmas svr_unchanged_defs = cl_svr_k'_t'_unchanged_def other_insts_unchanged_def svr_t'_unchanged_def
+lemmas cl_unchanged_defs = svr_cl_cl'_unchanged_def other_insts_unchanged_def
+lemmas unchanged_defs = svr_unchanged_defs svr_cl_cl'_unchanged_def
 
 definition tid_match :: "'v global_state \<Rightarrow> txid0 \<Rightarrow> bool" where
   "tid_match s t \<equiv> cl_sn (cls s (get_cl_txn t)) = get_sn_txn t"
 
-abbreviation km_state_trans where
-  "km_state_trans s k s' t from_stat to_stat \<equiv>
-      km_state (svrs s k) t = from_stat
+abbreviation svr_state_trans where
+  "svr_state_trans s k s' t from_stat to_stat \<equiv>
+      svr_state (svrs s k) t = from_stat
     \<and> svr_vl (svrs s' k) = svr_vl (svrs s k)
     \<and> svr_key_fp (svrs s' k) = svr_key_fp (svrs s k)
-    \<and> km_state (svrs s' k) t = to_stat
-    \<and> tm_km_k'_t'_unchanged k s s' t
+    \<and> svr_state (svrs s' k) t = to_stat
+    \<and> cl_svr_k'_t'_unchanged k s s' t
     \<and> tid_match s t"
+
+abbreviation is_locked :: "state_svr \<Rightarrow> bool" where
+  "is_locked svr_st \<equiv> svr_st \<in> {read_lock, write_lock, no_lock}"
+
+definition updated_kvs :: "'v global_state \<Rightarrow> cl_id \<Rightarrow> 'v kv_store" where
+  "updated_kvs s cl \<equiv> (\<lambda>k. update_kv_all_txn
+    (\<lambda>t. cl_state (cls (s \<lparr> cls := (cls s)
+      (cl := cls s cl \<lparr> cl_state := cl_committed \<rparr> ) \<rparr>) (get_cl_txn t)))
+    (svr_state (svrs s k)) (svr_key_fp (svrs s k)) (svr_vl (svrs s k)))"
 
 definition prepare where
   "prepare s k s' t \<equiv>
-    tm_state (cls s (get_cl_txn t)) = tm_prepared
-    \<and> km_state_trans s k s' t working prepared"
+    cl_state (cls s (get_cl_txn t)) = cl_prepared
+    \<and> svr_state_trans s k s' t working prepared"
 
 definition acquire_rd_lock where \<comment>\<open>Read Lock acquired\<close>
   "acquire_rd_lock s k v s' t \<equiv>
-    tm_state (cls s (get_cl_txn t)) = tm_prepared
-    \<and> (\<forall>t'. km_state (svrs s k) t' \<noteq> write_lock)
-    \<and> km_state (svrs s k) t = prepared
+    cl_state (cls s (get_cl_txn t)) = cl_prepared
+    \<and> (\<forall>t'. svr_state (svrs s k) t' \<noteq> write_lock)
+    \<and> svr_state (svrs s k) t = prepared
     \<and> svr_vl (svrs s' k) = svr_vl (svrs s k)
     \<and> v = v_value (last_version (svr_vl (svrs s k)) (full_view (svr_vl (svrs s k))))
     \<and> svr_key_fp (svrs s' k) t W = None
     \<and> svr_key_fp (svrs s' k) t R = Some v
-    \<and> km_state (svrs s' k) t = read_lock
-    \<and> tm_km_k'_t'_unchanged k s s' t
+    \<and> svr_state (svrs s' k) t = read_lock
+    \<and> cl_svr_k'_t'_unchanged k s s' t
     \<and> tid_match s t"
 
 definition acquire_wr_lock where \<comment>\<open>Write Lock acquired\<close>
   "acquire_wr_lock s k v ov s' t \<equiv>
-    tm_state (cls s (get_cl_txn t)) = tm_prepared
-    \<and> (\<forall>t'. km_state (svrs s k) t' \<notin> {write_lock, read_lock})
-    \<and> km_state (svrs s k) t = prepared
+    cl_state (cls s (get_cl_txn t)) = cl_prepared
+    \<and> (\<forall>t'. svr_state (svrs s k) t' \<notin> {write_lock, read_lock})
+    \<and> svr_state (svrs s k) t = prepared
     \<and> svr_vl (svrs s' k) = svr_vl (svrs s k)
     \<and> (ov = None \<or>
        ov = Some (v_value (last_version (svr_vl (svrs s k)) (full_view (svr_vl (svrs s k))))))
     \<and> svr_key_fp (svrs s' k) t W = Some v
     \<and> svr_key_fp (svrs s' k) t R = ov
-    \<and> km_state (svrs s' k) t = write_lock
-    \<and> tm_km_k'_t'_unchanged k s s' t
+    \<and> svr_state (svrs s' k) t = write_lock
+    \<and> cl_svr_k'_t'_unchanged k s s' t
     \<and> tid_match s t"
 
 definition acquire_no_lock where \<comment>\<open>No Lock needed\<close>
   "acquire_no_lock s k s' t \<equiv>
-    tm_state (cls s (get_cl_txn t)) = tm_prepared
+    cl_state (cls s (get_cl_txn t)) = cl_prepared
     \<and> svr_key_fp (svrs s' k) t W = None
     \<and> svr_key_fp (svrs s' k) t R = None
-    \<and> km_state_trans s k s' t prepared no_lock"
+    \<and> svr_state_trans s k s' t prepared no_lock"
 
 definition nok where \<comment>\<open>Lock not available\<close>
   "nok s k s' t \<equiv>
-    tm_state (cls s (get_cl_txn t)) = tm_prepared
-    \<and> km_state_trans s k s' t prepared notokay"
+    cl_state (cls s (get_cl_txn t)) = cl_prepared
+    \<and> svr_state_trans s k s' t prepared notokay"
 
 definition commit where
   "commit s k s' t \<equiv>
-    km_state (svrs s k) t \<in> {read_lock, write_lock, no_lock}
-    \<and> tm_state (cls s (get_cl_txn t)) = tm_committed
+    is_locked (svr_state (svrs s k) t)
+    \<and> cl_state (cls s (get_cl_txn t)) = cl_committed
     \<and> svr_vl (svrs s' k) =
         update_kv_key t (svr_key_fp (svrs s k) t) (full_view (svr_vl (svrs s k))) (svr_vl (svrs s k))
-    \<and> km_state (svrs s' k) t = committed
+    \<and> svr_state (svrs s' k) t = committed
     \<and> svr_key_fp (svrs s' k) t = svr_key_fp (svrs s k) t
-    \<and> tm_km_k'_t'_unchanged k s s' t
+    \<and> cl_svr_k'_t'_unchanged k s s' t
     \<and> tid_match s t"
 
 definition abort where \<comment>\<open>Locks released (aborted)\<close>
   "abort s k s' t \<equiv>
-    km_state (svrs s k) t \<in> {read_lock, write_lock, no_lock, notokay}
-    \<and> tm_state (cls s (get_cl_txn t)) = tm_aborted
+    svr_state (svrs s k) t \<in> {read_lock, write_lock, no_lock, notokay}
+    \<and> cl_state (cls s (get_cl_txn t)) = cl_aborted
     \<and> svr_vl (svrs s' k) = svr_vl (svrs s k)
-    \<and> km_state (svrs s' k) t = aborted
+    \<and> svr_state (svrs s' k) t = aborted
     \<and> svr_key_fp (svrs s' k) t = svr_key_fp (svrs s k) t
-    \<and> tm_km_k'_t'_unchanged k s s' t
+    \<and> cl_svr_k'_t'_unchanged k s s' t
     \<and> tid_match s t"
 
 definition user_commit where
   "user_commit s s' cl \<equiv>
-    tm_state (cls s cl) = tm_init
-    \<and> tm_state (cls s' cl) = tm_prepared
+    cl_state (cls s cl) = cl_init
+    \<and> cl_state (cls s' cl) = cl_prepared
     \<and> cl_sn (cls s' cl) = cl_sn (cls s cl)
     \<and> cl_view (cls s' cl) = cl_view (cls s cl)
-    \<and> km_tm_cl'_unchanged cl s s'"
+    \<and> svr_cl_cl'_unchanged cl s s'"
 
-definition tm_commit where
-  "tm_commit s s' cl sn u'' F \<equiv>
-    tm_state (cls s cl) = tm_prepared
-    \<and> (\<forall>k. km_state (svrs s k) (get_txn_cl cl s) \<in> {read_lock, write_lock, no_lock})
-    \<and> tm_state (cls s' cl) = tm_committed
-    \<and> cl_sn (cls s' cl) = cl_sn (cls s cl)
-    \<and> cl_view (cls s' cl) = (\<lambda>k. full_view (kvs_of_gs s' k))
-    \<and> km_tm_cl'_unchanged cl s s'
-    \<and> sn = cl_sn (cls s cl)
-    \<and> u'' = (\<lambda>k. full_view (kvs_of_gs s k))
-    \<and> F = (\<lambda>k. svr_key_fp (svrs s k) (get_txn_cl cl s))"
+definition cl_commit where
+  "cl_commit s s' cl sn u'' F \<equiv>
+    sn = cl_sn (cls s cl) \<and>
+    u'' = (\<lambda>k. full_view (kvs_of_gs s k)) \<and>
+    F = (\<lambda>k. svr_key_fp (svrs s k) (get_txn_cl cl s)) \<and>
+    cl_state (cls s cl) = cl_prepared \<and>
+    (\<forall>k. is_locked (svr_state (svrs s k) (get_txn_cl cl s))) \<and>
+    cl_state (cls s' cl) = cl_committed \<and>
+    cl_sn (cls s' cl) = cl_sn (cls s cl) \<and>
+    cl_view (cls s' cl) = full_view o (updated_kvs s cl) \<and>
+    svr_cl_cl'_unchanged cl s s'"
 
-definition tm_abort where
-  "tm_abort s s' cl \<equiv>
-    tm_state (cls s cl) = tm_prepared
-    \<and> (\<exists>k. km_state (svrs s k) (get_txn_cl cl s) = notokay)
-    \<and> (\<forall>k. km_state (svrs s k) (get_txn_cl cl s) \<in> {read_lock, write_lock, no_lock, notokay})
-    \<and> tm_state (cls s' cl) = tm_aborted
+definition cl_abort where
+  "cl_abort s s' cl \<equiv>
+    cl_state (cls s cl) = cl_prepared
+    \<and> (\<exists>k. svr_state (svrs s k) (get_txn_cl cl s) = notokay)
+    \<and> (\<forall>k. svr_state (svrs s k) (get_txn_cl cl s) \<in> {read_lock, write_lock, no_lock, notokay})
+    \<and> cl_state (cls s' cl) = cl_aborted
     \<and> cl_sn (cls s' cl) = cl_sn (cls s cl)
     \<and> cl_view (cls s' cl) = cl_view (cls s cl)
-    \<and> km_tm_cl'_unchanged cl s s'"
+    \<and> svr_cl_cl'_unchanged cl s s'"
 
-definition tm_ready_c where
-  "tm_ready_c s s' cl \<equiv>
-    tm_state (cls s cl) = tm_committed
-    \<and> (\<forall>k. km_state (svrs s k) (get_txn_cl cl s) = committed)
-    \<and> tm_state (cls s' cl) = tm_init
+definition cl_ready_c where
+  "cl_ready_c s s' cl \<equiv>
+    cl_state (cls s cl) = cl_committed
+    \<and> (\<forall>k. svr_state (svrs s k) (get_txn_cl cl s) = committed)
+    \<and> cl_state (cls s' cl) = cl_init
     \<and> cl_sn (cls s' cl) = Suc (cl_sn (cls s cl))
     \<and> cl_view (cls s' cl) = cl_view (cls s cl)
-    \<and> km_tm_cl'_unchanged cl s s'"
+    \<and> svr_cl_cl'_unchanged cl s s'"
 
-definition tm_ready_a where
-  "tm_ready_a s s' cl \<equiv>
-    tm_state (cls s cl) = tm_aborted
-    \<and> (\<forall>k. km_state (svrs s k) (get_txn_cl cl s) = aborted)
-    \<and> tm_state (cls s' cl) = tm_init
+definition cl_ready_a where
+  "cl_ready_a s s' cl \<equiv>
+    cl_state (cls s cl) = cl_aborted
+    \<and> (\<forall>k. svr_state (svrs s k) (get_txn_cl cl s) = aborted)
+    \<and> cl_state (cls s' cl) = cl_init
     \<and> cl_sn (cls s' cl) = Suc (cl_sn (cls s cl))
     \<and> cl_view (cls s' cl) = cl_view (cls s cl)
-    \<and> km_tm_cl'_unchanged cl s s'"
+    \<and> svr_cl_cl'_unchanged cl s s'"
 
 
 subsubsection \<open>The Event System\<close>
 
 definition gs_init :: "'v global_state" where
   "gs_init \<equiv> \<lparr> 
-    cls = (\<lambda>cl. \<lparr> tm_state = tm_init,
+    cls = (\<lambda>cl. \<lparr> cl_state = cl_init,
                  cl_sn = 0,
                  cl_view = view_init \<rparr>),
-    svrs = (\<lambda>k. \<lparr> km_state = (\<lambda>t. working),
+    svrs = (\<lambda>k. \<lparr> svr_state = (\<lambda>t. working),
                  svr_vl = [version_init],
                  svr_key_fp = (\<lambda>t. Map.empty)\<rparr>)
   \<rparr>"
@@ -250,10 +259,10 @@ fun gs_trans :: "'v global_state \<Rightarrow> 'v ev \<Rightarrow> 'v global_sta
   "gs_trans s (Commit k t)          s' \<longleftrightarrow> commit s k s' t" |
   "gs_trans s (Abort k t)           s' \<longleftrightarrow> abort s k s' t" |
   "gs_trans s (User_Commit cl)      s' \<longleftrightarrow> user_commit s s' cl" |
-  "gs_trans s (TM_Commit cl sn u F) s' \<longleftrightarrow> tm_commit s s' cl sn u F" |
-  "gs_trans s (TM_Abort cl)         s' \<longleftrightarrow> tm_abort s s' cl" |
-  "gs_trans s (TM_ReadyC cl)        s' \<longleftrightarrow> tm_ready_c s s' cl" |
-  "gs_trans s (TM_ReadyA cl)        s' \<longleftrightarrow> tm_ready_a s s' cl" |
+  "gs_trans s (Cl_Commit cl sn u F) s' \<longleftrightarrow> cl_commit s s' cl sn u F" |
+  "gs_trans s (Cl_Abort cl)         s' \<longleftrightarrow> cl_abort s s' cl" |
+  "gs_trans s (Cl_ReadyC cl)        s' \<longleftrightarrow> cl_ready_c s s' cl" |
+  "gs_trans s (Cl_ReadyA cl)        s' \<longleftrightarrow> cl_ready_a s s' cl" |
   "gs_trans s Skip2                 s' \<longleftrightarrow> s' = s"
 
 definition tps :: "('v ev, 'v global_state) ES" where
@@ -264,7 +273,7 @@ definition tps :: "('v ev, 'v global_state) ES" where
 
 lemmas tps_trans_defs = prepare_def acquire_rd_lock_def acquire_wr_lock_def
                         acquire_no_lock_def nok_def commit_def abort_def
-                        user_commit_def tm_commit_def tm_abort_def tm_ready_c_def tm_ready_a_def
+                        user_commit_def cl_commit_def cl_abort_def cl_ready_c_def cl_ready_a_def
 
 lemmas tps_defs = tps_def gs_init_def
 
@@ -273,7 +282,7 @@ lemma tps_trans [simp]: "trans tps = gs_trans" by (simp add: tps_def)
 subsubsection \<open>Mediator function\<close>
 
 fun med :: "'v ev \<Rightarrow> 'v label" where
-  "med (TM_Commit cl sn u F) = ET cl sn u F" |
+  "med (Cl_Commit cl sn u F) = ET cl sn u F" |
   "med _ = ETSkip"
 
 end
