txn-data-consistency/Serializable_2PC_2PL_Invariants.thy
@@ -7,37 +7,37 @@ begin
 \<comment> \<open>Invariant about future and past transactions svrs\<close>
 
 definition TIDFutureKm where
-  "TIDFutureKm s cl \<longleftrightarrow> (\<forall>n k. n > cl_sn (cls s cl) \<longrightarrow> km_state (svrs s k) (Tn_cl n cl) = working)"
+  "TIDFutureKm s cl \<longleftrightarrow> (\<forall>n k. n > cl_sn (cls s cl) \<longrightarrow> svr_state (svrs s k) (Tn_cl n cl) = working)"
 
 definition TIDPastKm where
-  "TIDPastKm s cl \<longleftrightarrow> (\<forall>n k. n < cl_sn (cls s cl) \<longrightarrow> km_state (svrs s k) (Tn_cl n cl) \<in> {committed, aborted})"
+  "TIDPastKm s cl \<longleftrightarrow> (\<forall>n k. n < cl_sn (cls s cl) \<longrightarrow> svr_state (svrs s k) (Tn_cl n cl) \<in> {committed, aborted})"
 
 lemma other_sn_idle:
   assumes "TIDFutureKm s cl" and "TIDPastKm s cl"
     and "get_cl_txn t = cl" and "get_sn_txn t \<noteq> cl_sn (cls s cl)"
-  shows "\<And>k. km_state (svrs s k) t \<in> {working, committed, aborted}"
+  shows "\<And>k. svr_state (svrs s k) t \<in> {working, committed, aborted}"
   oops
 
 \<comment> \<open>Lock Invariants\<close>
 
 definition RLockInv where
-  "RLockInv s k \<longleftrightarrow> (\<forall>t. km_state (svrs s k) t = read_lock \<longrightarrow> (\<forall>t. km_state (svrs s k) t \<noteq> write_lock))"
+  "RLockInv s k \<longleftrightarrow> (\<forall>t. svr_state (svrs s k) t = read_lock \<longrightarrow> (\<forall>t. svr_state (svrs s k) t \<noteq> write_lock))"
 
 definition WLockInv where
-  "WLockInv s k \<longleftrightarrow> (\<forall>t. km_state (svrs s k) t \<noteq> write_lock) \<or> (\<exists>! t. km_state (svrs s k) t = write_lock)"
+  "WLockInv s k \<longleftrightarrow> (\<forall>t. svr_state (svrs s k) t \<noteq> write_lock) \<or> (\<exists>! t. svr_state (svrs s k) t = write_lock)"
 
 \<comment> \<open>Invariants for fingerprint, knowing the lock (km status)\<close>
 
 definition RLockFpInv where
-  "RLockFpInv s k \<longleftrightarrow> (\<forall>t. km_state (svrs s k) t = read_lock \<longrightarrow>
+  "RLockFpInv s k \<longleftrightarrow> (\<forall>t. svr_state (svrs s k) t = read_lock \<longrightarrow>
     svr_key_fp (svrs s k) t W = None \<and>
     svr_key_fp (svrs s k) t R \<noteq> None)"
 
 definition WLockFpInv where
-  "WLockFpInv s k \<longleftrightarrow> (\<forall>t. km_state (svrs s k) t = write_lock \<longrightarrow> svr_key_fp (svrs s k) t W \<noteq> None)"
+  "WLockFpInv s k \<longleftrightarrow> (\<forall>t. svr_state (svrs s k) t = write_lock \<longrightarrow> svr_key_fp (svrs s k) t W \<noteq> None)"
 
 definition NoLockFpInv where
-  "NoLockFpInv s k \<longleftrightarrow> (\<forall>t. km_state (svrs s k) t = no_lock \<longrightarrow>
+  "NoLockFpInv s k \<longleftrightarrow> (\<forall>t. svr_state (svrs s k) t = no_lock \<longrightarrow>
     svr_key_fp (svrs s k) t W = None \<and>
     svr_key_fp (svrs s k) t R = None)"
 
@@ -53,40 +53,40 @@ definition KVSLen where
 
 subsubsection \<open>Lemmas for kvs_of_gs changing by different events\<close>
 
-lemma kvs_of_gs_km_inv:
+lemma kvs_of_gs_svr_inv:
   assumes "WLockInv s k" and "RLockInv s k"
-    and "(\<forall>t. km_state (svrs s k) t \<noteq> write_lock) \<or> 
-              km_state (svrs s' k) t \<noteq> write_lock"
-    and "tm_state (cls s (get_cl_txn t)) \<noteq> tm_committed"
+    and "(\<forall>t. svr_state (svrs s k) t \<noteq> write_lock) \<or> 
+              svr_state (svrs s' k) t \<noteq> write_lock"
+    and "cl_state (cls s (get_cl_txn t)) \<noteq> cl_committed"
     and "\<And>k. svr_vl (svrs s' k) = svr_vl (svrs s k)"
-    and "tm_km_k'_t'_unchanged k s s' t"
+    and "cl_svr_k'_t'_unchanged k s s' t"
   shows "kvs_of_gs s' = kvs_of_gs s"
   oops
 
-lemma kvs_of_gs_tm_inv:
+lemma kvs_of_gs_cl_inv:
   assumes "TIDFutureKm s cl" and "TIDPastKm s cl"
-    and "tm_state (cls s cl) \<noteq> tm_committed \<or>
-         (\<forall>k. km_state (svrs s k) (get_txn_cl cl s) = committed)"
-    and "tm_state (cls s' cl) \<noteq> tm_committed"
-    and "km_tm_cl'_unchanged cl s s'"
+    and "cl_state (cls s cl) \<noteq> cl_committed \<or>
+         (\<forall>k. svr_state (svrs s k) (get_txn_cl cl s) = committed)"
+    and "cl_state (cls s' cl) \<noteq> cl_committed"
+    and "svr_cl_cl'_unchanged cl s s'"
   shows "kvs_of_gs s' = kvs_of_gs s"
   oops
 
-lemma update_kv_all_tm_commit_no_lock_inv:
+lemma update_kv_all_cl_commit_no_lock_inv:
   assumes "TIDPastKm s cl" and "TIDFutureKm s cl"
-    and "tm_state (cls s cl) = tm_prepared"
-    and "tm_state (cls s' cl) = tm_committed"
+    and "cl_state (cls s cl) = cl_prepared"
+    and "cl_state (cls s' cl) = cl_committed"
     and "other_insts_unchanged cl (cls s) (cls s')"
-    and "km_state (svrs s k) (get_txn_cl cl s) = no_lock"
-  shows "update_kv_all_txn (\<lambda>t. tm_state (cls s' (get_cl_txn t))) (km_state (svrs s k))
+    and "svr_state (svrs s k) (get_txn_cl cl s) = no_lock"
+  shows "update_kv_all_txn (\<lambda>t. cl_state (cls s' (get_cl_txn t))) (svr_state (svrs s k))
           (svr_key_fp (svrs s k)) (svr_vl (svrs s k)) =
-         update_kv_all_txn (\<lambda>t. tm_state (cls s (get_cl_txn t))) (km_state (svrs s k))
+         update_kv_all_txn (\<lambda>t. cl_state (cls s (get_cl_txn t))) (svr_state (svrs s k))
           (svr_key_fp (svrs s k)) (svr_vl (svrs s k))"
   oops
 
 (*All events*)
-abbreviation not_tm_commit where
-  "not_tm_commit e \<equiv> \<forall>cl sn u F. e \<noteq> TM_Commit cl sn u F"
+abbreviation not_cl_commit where
+  "not_cl_commit e \<equiv> \<forall>cl sn u F. e \<noteq> Cl_Commit cl sn u F"
 
 abbreviation invariant_list_kvs where
   "invariant_list_kvs s \<equiv> \<forall>cl k. TIDFutureKm s cl \<and> TIDPastKm s cl \<and> RLockInv s k \<and> WLockInv s k \<and>
@@ -95,15 +95,15 @@ abbreviation invariant_list_kvs where
 lemma kvs_of_gs_inv:
   assumes "gs_trans s e s'"
     and "invariant_list_kvs s"
-    and "not_tm_commit e"
+    and "not_cl_commit e"
   shows "kvs_of_gs s' = kvs_of_gs s"
   oops
 
 \<comment> \<open>More specific lemmas about TM commit\<close>
 lemma kvs_of_gs_commit_length_increasing:
-  assumes "tm_state (cls s cl) = tm_prepared"
-    and "tm_state (cls s' cl) = tm_committed"
-    and "km_tm_cl'_unchanged cl s s'"
+  assumes "cl_state (cls s cl) = cl_prepared"
+    and "cl_state (cls s' cl) = cl_committed"
+    and "svr_cl_cl'_unchanged cl s s'"
   shows "length (kvs_of_gs s k) \<le> length (kvs_of_gs s' k)"
   oops
 
@@ -117,36 +117,36 @@ lemma kvs_of_gs_length_increasing:
 
 lemma svr_vl_read_lock_commit_eq_length:
   assumes "RLockFpInv s k"
-    and "km_state (svrs s k) t = read_lock"
+    and "svr_state (svrs s k) t = read_lock"
     and "svr_vl (svrs s' k) =
           update_kv_key t (svr_key_fp (svrs s k) t) (full_view (svr_vl (svrs s k))) (svr_vl (svrs s k))"
   shows "length (svr_vl (svrs s' k)) = length (svr_vl (svrs s k))"
   oops
 
 definition RLockFpContentInv where
-  "RLockFpContentInv s k \<longleftrightarrow> (\<forall>t. km_state (svrs s k) t = read_lock \<longrightarrow>
+  "RLockFpContentInv s k \<longleftrightarrow> (\<forall>t. svr_state (svrs s k) t = read_lock \<longrightarrow>
     svr_key_fp (svrs s k) t R =
       Some (v_value (last_version (svr_vl (svrs s k)) (full_view (svr_vl (svrs s k))))))"
 
 definition WLockFpContentInv where
-  "WLockFpContentInv s k \<longleftrightarrow> (\<forall>t. km_state (svrs s k) t = write_lock \<longrightarrow>
+  "WLockFpContentInv s k \<longleftrightarrow> (\<forall>t. svr_state (svrs s k) t = write_lock \<longrightarrow>
     svr_key_fp (svrs s k) t R = None \<or>
     svr_key_fp (svrs s k) t R =
       Some (v_value (last_version (svr_vl (svrs s k)) (full_view (svr_vl (svrs s k))))))"
 
 lemma svr_vl_kvs_eq_length:
   assumes "WLockInv s k" and "RLockInv s k"
-    and "tm_state (cls s cl) = tm_prepared"
-    and "km_state (svrs s k) (get_txn_cl cl s) \<in> {read_lock, write_lock}"
+    and "cl_state (cls s cl) = cl_prepared"
+    and "svr_state (svrs s k) (get_txn_cl cl s) \<in> {read_lock, write_lock}"
   shows "length (kvs_of_gs s k) = length (svr_vl (svrs s k))"
   oops
 
 \<comment> \<open>Lemmas for view growth after commit\<close>
 
 lemma committed_kvs_view_grows:
-  assumes "tm_state (cls s cl) = tm_prepared"
-    and "tm_state (cls s' cl) = tm_committed"
-    and "km_tm_cl'_unchanged cl s s'"
+  assumes "cl_state (cls s cl) = cl_prepared"
+    and "cl_state (cls s' cl) = cl_committed"
+    and "svr_cl_cl'_unchanged cl s s'"
   shows "(\<lambda>k. full_view (kvs_of_gs s k)) \<sqsubseteq> (\<lambda>k. full_view (kvs_of_gs s' k))"
   oops
   
@@ -159,30 +159,30 @@ lemma updated_vl_view_grows:
 
 lemma cl_view_inv:
   assumes "gs_trans s e s'"
-    and "not_tm_commit e"
+    and "not_cl_commit e"
   shows "cl_view (cls s' cl) = cl_view (cls s cl)"
   oops
 
 definition TMFullView where
   "TMFullView s cl \<longleftrightarrow> cl_view (cls s cl) \<sqsubseteq> (\<lambda>k. full_view (kvs_of_gs s k))"
 
-\<comment> \<open>TM_commit updating kv\<close>
+\<comment> \<open>Cl_commit updating kv\<close>
 
-lemma kvs_of_gs_tm_commit:
+lemma kvs_of_gs_cl_commit:
   assumes "TIDFutureKm s cl" and "TIDPastKm s cl"
     and "WLockInv s k" and "WLockFpInv s k"
     and "RLockInv s k" and "RLockFpInv s k"
     and "NoLockFpInv s k" and "KVSNonEmp s"
-    and "tm_state (cls s cl) = tm_prepared"
-    and "km_state (svrs s k) (get_txn_cl cl s) \<in> {read_lock, write_lock, no_lock}"
-    and "tm_state (cls s' cl) = tm_committed"
+    and "cl_state (cls s cl) = cl_prepared"
+    and "svr_state (svrs s k) (get_txn_cl cl s) \<in> {read_lock, write_lock, no_lock}"
+    and "cl_state (cls s' cl) = cl_committed"
     and "other_insts_unchanged cl (cls s) (cls s')"
-  shows "update_kv_all_txn (\<lambda>t. tm_state (cls s' (get_cl_txn t))) (km_state (svrs s k))
+  shows "update_kv_all_txn (\<lambda>t. cl_state (cls s' (get_cl_txn t))) (svr_state (svrs s k))
           (svr_key_fp (svrs s k)) (svr_vl (svrs s k)) =
     update_kv_key (get_txn_cl cl s) (svr_key_fp (svrs s k) (get_txn_cl cl s))
-      (full_view (update_kv_all_txn (\<lambda>t. tm_state (cls s (get_cl_txn t))) (km_state (svrs s k))
+      (full_view (update_kv_all_txn (\<lambda>t. cl_state (cls s (get_cl_txn t))) (svr_state (svrs s k))
         (svr_key_fp (svrs s k)) (svr_vl (svrs s k))))
-      (update_kv_all_txn (\<lambda>t. tm_state (cls s (get_cl_txn t))) (km_state (svrs s k))
+      (update_kv_all_txn (\<lambda>t. cl_state (cls s (get_cl_txn t))) (svr_state (svrs s k))
         (svr_key_fp (svrs s k)) (svr_vl (svrs s k)))"
   oops
 
@@ -193,12 +193,12 @@ lemma get_sqns_other_cl_inv:
     and "\<And>k. WLockInv s k" and "\<And>k. WLockFpInv s k"
     and "\<And>k. RLockInv s k" and "\<And>k. RLockFpInv s k"
     and "\<And>k. NoLockFpInv s k" and "KVSNonEmp s"
-    and "tm_state (cls s cl) = tm_prepared"
-    and "tm_state (cls s' cl) = tm_committed"
-    and "\<And>k. km_state (svrs s k) (get_txn_cl cl s) = read_lock \<or>
-             km_state (svrs s k) (get_txn_cl cl s) = write_lock \<or> 
-             km_state (svrs s k) (get_txn_cl cl s) = no_lock"
-    and "km_tm_cl'_unchanged cl s s'"
+    and "cl_state (cls s cl) = cl_prepared"
+    and "cl_state (cls s' cl) = cl_committed"
+    and "\<And>k. svr_state (svrs s k) (get_txn_cl cl s) = read_lock \<or>
+             svr_state (svrs s k) (get_txn_cl cl s) = write_lock \<or> 
+             svr_state (svrs s k) (get_txn_cl cl s) = no_lock"
+    and "svr_cl_cl'_unchanged cl s s'"
     and "cl' \<noteq> cl"
   shows "get_sqns (kvs_of_gs s') cl' = get_sqns (kvs_of_gs s) cl'"
   oops
@@ -208,9 +208,9 @@ lemma new_t_is_in_writers:
     and "\<And>k. WLockInv s k" and "\<And>k. WLockFpInv s k"
     and "\<And>k. RLockInv s k" and "\<And>k. RLockFpInv s k"
     and "\<And>k. NoLockFpInv s k" and "KVSNonEmp s"
-    and "tm_state (cls s cl) = tm_prepared"
-    and "tm_state (cls s' cl) = tm_committed"
-    and "km_state (svrs s k) (get_txn_cl cl s) = write_lock"
+    and "cl_state (cls s cl) = cl_prepared"
+    and "cl_state (cls s' cl) = cl_committed"
+    and "svr_state (svrs s k) (get_txn_cl cl s) = write_lock"
     and "other_insts_unchanged cl (cls s) (cls s')"
     and "svrs s' = svrs s"
   shows "vl_writers_sqns (kvs_of_gs s' k) cl = vl_writers_sqns (kvs_of_gs s k) cl \<union> {cl_sn (cls s cl)}"
@@ -221,9 +221,9 @@ lemma new_t_is_in_writers2:
     and "\<And>k. WLockInv s k" and "\<And>k. WLockFpInv s k"
     and "\<And>k. RLockInv s k" and "\<And>k. RLockFpInv s k"
     and "\<And>k. NoLockFpInv s k" and "KVSNonEmp s"
-    and "tm_state (cls s cl) = tm_prepared"
-    and "tm_state (cls s' cl) = tm_committed"
-    and "km_state (svrs s k) (get_txn_cl cl s) = read_lock"
+    and "cl_state (cls s cl) = cl_prepared"
+    and "cl_state (cls s' cl) = cl_committed"
+    and "svr_state (svrs s k) (get_txn_cl cl s) = read_lock"
     and "other_insts_unchanged cl (cls s) (cls s')"
     and "svrs s' = svrs s"
   shows "vl_writers_sqns (kvs_of_gs s' k) cl = vl_writers_sqns (kvs_of_gs s k) cl"
@@ -234,9 +234,9 @@ lemma new_t_is_in_readers:
     and "\<And>k. WLockInv s k" and "\<And>k. WLockFpInv s k"
     and "\<And>k. RLockInv s k" and "\<And>k. RLockFpInv s k"
     and "\<And>k. NoLockFpInv s k" and "KVSNonEmp s"
-    and "tm_state (cls s cl) = tm_prepared"
-    and "tm_state (cls s' cl) = tm_committed"
-    and "km_state (svrs s k) (get_txn_cl cl s) = read_lock"
+    and "cl_state (cls s cl) = cl_prepared"
+    and "cl_state (cls s' cl) = cl_committed"
+    and "svr_state (svrs s k) (get_txn_cl cl s) = read_lock"
     and "other_insts_unchanged cl (cls s) (cls s')"
     and "svrs s' = svrs s"
   shows "vl_readers_sqns (kvs_of_gs s' k) cl = vl_readers_sqns (kvs_of_gs s k) cl \<union> {cl_sn (cls s cl)}"
@@ -247,9 +247,9 @@ lemma new_t_is_in_readers2:
     and "\<And>k. WLockInv s k" and "\<And>k. WLockFpInv s k"
     and "\<And>k. RLockInv s k" and "\<And>k. RLockFpInv s k"
     and "\<And>k. NoLockFpInv s k" and "KVSNonEmp s"
-    and "tm_state (cls s cl) = tm_prepared"
-    and "tm_state (cls s' cl) = tm_committed"
-    and "km_state (svrs s k) (get_txn_cl cl s) = write_lock"
+    and "cl_state (cls s cl) = cl_prepared"
+    and "cl_state (cls s' cl) = cl_committed"
+    and "svr_state (svrs s k) (get_txn_cl cl s) = write_lock"
     and "svr_key_fp (svrs s k) (get_txn_cl cl s) R \<noteq> None"
     and "other_insts_unchanged cl (cls s) (cls s')"
     and "svrs s' = svrs s"
@@ -261,93 +261,93 @@ lemma new_t_is_in_readers3:
     and "\<And>k. WLockInv s k" and "\<And>k. WLockFpInv s k"
     and "\<And>k. RLockInv s k" and "\<And>k. RLockFpInv s k"
     and "\<And>k. NoLockFpInv s k" and "KVSNonEmp s"
-    and "tm_state (cls s cl) = tm_prepared"
-    and "tm_state (cls s' cl) = tm_committed"
-    and "km_state (svrs s k) (get_txn_cl cl s) = write_lock"
+    and "cl_state (cls s cl) = cl_prepared"
+    and "cl_state (cls s' cl) = cl_committed"
+    and "svr_state (svrs s k) (get_txn_cl cl s) = write_lock"
     and "svr_key_fp (svrs s k) (get_txn_cl cl s) R = None"
     and "other_insts_unchanged cl (cls s) (cls s')"
     and "svrs s' = svrs s"
   shows "vl_readers_sqns (kvs_of_gs s' k) cl = vl_readers_sqns (kvs_of_gs s k) cl"
   oops
 
-lemma kvs_writers_tm_commit_grows:
+lemma kvs_writers_cl_commit_grows:
   assumes "TIDFutureKm s cl" and "TIDPastKm s cl"
     and "\<And>k. WLockInv s k" and "\<And>k. WLockFpInv s k"
     and "\<And>k. RLockInv s k" and "\<And>k. RLockFpInv s k"
     and "\<And>k. NoLockFpInv s k" and "KVSNonEmp s"
-    and "tm_state (cls s cl) = tm_prepared"
-    and "tm_state (cls s' cl) = tm_committed"
-    and "\<forall>k. km_state (svrs s k) (get_txn_cl cl s) \<in> {read_lock, write_lock, no_lock}"
-    and "km_state (svrs s k) (get_txn_cl cl s) = write_lock"
+    and "cl_state (cls s cl) = cl_prepared"
+    and "cl_state (cls s' cl) = cl_committed"
+    and "\<forall>k. svr_state (svrs s k) (get_txn_cl cl s) \<in> {read_lock, write_lock, no_lock}"
+    and "svr_state (svrs s k) (get_txn_cl cl s) = write_lock"
     and "other_insts_unchanged cl (cls s) (cls s')"
     and "svrs s' = svrs s"
   shows "kvs_writers_sqns (kvs_of_gs s') cl = kvs_writers_sqns (kvs_of_gs s) cl \<union> {cl_sn (cls s cl)}"
   oops
 
-lemma kvs_writers_tm_commit_doesnt_grow:
+lemma kvs_writers_cl_commit_doesnt_grow:
   assumes "TIDFutureKm s cl" and "TIDPastKm s cl"
     and "\<And>k. WLockInv s k" and "\<And>k. WLockFpInv s k"
     and "\<And>k. RLockInv s k" and "\<And>k. RLockFpInv s k"
     and "\<And>k. NoLockFpInv s k" and "KVSNonEmp s"
-    and "tm_state (cls s cl) = tm_prepared"
-    and "tm_state (cls s' cl) = tm_committed"
-    and "\<forall>k. km_state (svrs s k) (get_txn_cl cl s) \<in> {read_lock, no_lock}"
+    and "cl_state (cls s cl) = cl_prepared"
+    and "cl_state (cls s' cl) = cl_committed"
+    and "\<forall>k. svr_state (svrs s k) (get_txn_cl cl s) \<in> {read_lock, no_lock}"
     and "other_insts_unchanged cl (cls s) (cls s')"
     and "svrs s' = svrs s"
   shows "kvs_writers_sqns (kvs_of_gs s') cl = kvs_writers_sqns (kvs_of_gs s) cl"
   oops
 
-lemma kvs_readers_sqns_tm_commit_grows:
+lemma kvs_readers_sqns_cl_commit_grows:
   assumes "TIDFutureKm s cl" and "TIDPastKm s cl"
     and "\<And>k. WLockInv s k" and "\<And>k. WLockFpInv s k"
     and "\<And>k. RLockInv s k" and "\<And>k. RLockFpInv s k"
     and "\<And>k. NoLockFpInv s k" and "KVSNonEmp s"
-    and "tm_state (cls s cl) = tm_prepared"
-    and "tm_state (cls s' cl) = tm_committed"
-    and "\<forall>k. km_state (svrs s k) (get_txn_cl cl s) \<in> {read_lock, write_lock, no_lock}"
-    and "km_state (svrs s k) (get_txn_cl cl s) = read_lock \<or>
-         (km_state (svrs s k) (get_txn_cl cl s) = write_lock \<and>
+    and "cl_state (cls s cl) = cl_prepared"
+    and "cl_state (cls s' cl) = cl_committed"
+    and "\<forall>k. svr_state (svrs s k) (get_txn_cl cl s) \<in> {read_lock, write_lock, no_lock}"
+    and "svr_state (svrs s k) (get_txn_cl cl s) = read_lock \<or>
+         (svr_state (svrs s k) (get_txn_cl cl s) = write_lock \<and>
           svr_key_fp (svrs s k) (get_txn_cl cl s) R \<noteq> None)"
     and "other_insts_unchanged cl (cls s) (cls s')"
     and "svrs s' = svrs s"
   shows "kvs_readers_sqns (kvs_of_gs s') cl = kvs_readers_sqns (kvs_of_gs s) cl \<union> {cl_sn (cls s cl)}"
   oops
 
-lemma kvs_readers_sqns_tm_commit_doesnt_grow:
+lemma kvs_readers_sqns_cl_commit_doesnt_grow:
   assumes "TIDFutureKm s cl" and "TIDPastKm s cl"
     and "\<And>k. WLockInv s k" and "\<And>k. WLockFpInv s k"
     and "\<And>k. RLockInv s k" and "\<And>k. RLockFpInv s k"
     and "\<And>k. NoLockFpInv s k" and "KVSNonEmp s"
-    and "tm_state (cls s cl) = tm_prepared"
-    and "tm_state (cls s' cl) = tm_committed"
-    and "\<forall>k. km_state (svrs s k) (get_txn_cl cl s) \<in> {write_lock, no_lock}"
-    and "\<forall>k. km_state (svrs s k) (get_txn_cl cl s) \<noteq> write_lock \<or>
+    and "cl_state (cls s cl) = cl_prepared"
+    and "cl_state (cls s' cl) = cl_committed"
+    and "\<forall>k. svr_state (svrs s k) (get_txn_cl cl s) \<in> {write_lock, no_lock}"
+    and "\<forall>k. svr_state (svrs s k) (get_txn_cl cl s) \<noteq> write_lock \<or>
              svr_key_fp (svrs s k) (get_txn_cl cl s) R = None"
     and "other_insts_unchanged cl (cls s) (cls s')"
     and "svrs s' = svrs s"
   shows "kvs_readers_sqns (kvs_of_gs s') cl = kvs_readers_sqns (kvs_of_gs s) cl"
   oops
 
-lemma get_sqns_tm_commit_grows:
+lemma get_sqns_cl_commit_grows:
   assumes "TIDFutureKm s cl" and "TIDPastKm s cl"
     and "\<And>k. WLockInv s k" and "\<And>k. WLockFpInv s k"
     and "\<And>k. RLockInv s k" and "\<And>k. RLockFpInv s k"
     and "\<And>k. NoLockFpInv s k" and "KVSNonEmp s"
-    and "tm_state (cls s cl) = tm_prepared"
-    and "tm_state (cls s' cl) = tm_committed"
-    and "\<And>k. km_state (svrs s k) (get_txn_cl cl s) \<in> {read_lock, write_lock, no_lock}"
+    and "cl_state (cls s cl) = cl_prepared"
+    and "cl_state (cls s' cl) = cl_committed"
+    and "\<And>k. svr_state (svrs s k) (get_txn_cl cl s) \<in> {read_lock, write_lock, no_lock}"
     and "other_insts_unchanged cl (cls s) (cls s')"
     and "svrs s' = svrs s"
   shows "get_sqns (kvs_of_gs s') cl =
-         (if \<forall>k. km_state (svrs s k) (get_txn_cl cl s) = no_lock then
+         (if \<forall>k. svr_state (svrs s k) (get_txn_cl cl s) = no_lock then
           get_sqns (kvs_of_gs s) cl else
           get_sqns (kvs_of_gs s) cl \<union> {cl_sn (cls s cl)})"
   oops
 
 definition SqnInv where
   "SqnInv s cl \<longleftrightarrow>
-    (tm_state (cls s cl) \<noteq> tm_committed \<longrightarrow> (\<forall>m \<in> get_sqns (kvs_of_gs s) cl. m < cl_sn (cls s cl))) \<and>
-    (tm_state (cls s cl) = tm_committed \<longrightarrow> (\<forall>m \<in> get_sqns (kvs_of_gs s) cl. m \<le> cl_sn (cls s cl)))"
+    (cl_state (cls s cl) \<noteq> cl_committed \<longrightarrow> (\<forall>m \<in> get_sqns (kvs_of_gs s) cl. m < cl_sn (cls s cl))) \<and>
+    (cl_state (cls s cl) = cl_committed \<longrightarrow> (\<forall>m \<in> get_sqns (kvs_of_gs s) cl. m \<le> cl_sn (cls s cl)))"
 
 
 \<comment> \<open>Lemmas for proving view wellformedness of cl_view\<close>
@@ -355,30 +355,30 @@ definition SqnInv where
 lemma kvs_of_gs_version_order:
   assumes "TIDPastKm s cl" and "TIDFutureKm s cl" and "WLockInv s k" and "RLockInv s k" and "KVSNonEmp s"
     and "i \<in> full_view (kvs_of_gs s k)"
-    and "tm_state (cls s cl) = tm_prepared"
-    and "tm_state (cls s' cl) = tm_committed"
-    and "km_state (svrs s k) (get_txn_cl cl s) \<in> {read_lock, write_lock, no_lock}"
-    and "km_tm_cl'_unchanged cl s s'"
+    and "cl_state (cls s cl) = cl_prepared"
+    and "cl_state (cls s' cl) = cl_committed"
+    and "svr_state (svrs s k) (get_txn_cl cl s) \<in> {read_lock, write_lock, no_lock}"
+    and "svr_cl_cl'_unchanged cl s s'"
   shows "kvs_of_gs s k ! i \<sqsubseteq>\<^sub>v\<^sub>e\<^sub>r kvs_of_gs s' k ! i"
   oops
 
 lemma new_version_index:
   assumes "TIDPastKm s cl" and "TIDFutureKm s cl"
     and "WLockInv s k" and "KVSNonEmp s"
-    and "tm_state (cls s cl) = tm_prepared"
-    and "tm_state (cls s' cl) = tm_committed"
-    and "km_state (svrs s k) (get_txn_cl cl s) = write_lock"
+    and "cl_state (cls s cl) = cl_prepared"
+    and "cl_state (cls s' cl) = cl_committed"
+    and "svr_state (svrs s k) (get_txn_cl cl s) = write_lock"
     and "other_insts_unchanged cl (cls s) (cls s')"
-    and "i \<in> full_view (update_kv_all_txn (\<lambda>t. tm_state (cls s' (get_cl_txn t)))
-    (km_state (svrs s k)) (svr_key_fp (svrs s k)) (svr_vl (svrs s k)))"
-    and "i \<notin> full_view (update_kv_all_txn (\<lambda>t. tm_state (cls s (get_cl_txn t)))
-    (km_state (svrs s k)) (svr_key_fp (svrs s k)) (svr_vl (svrs s k)))"
+    and "i \<in> full_view (update_kv_all_txn (\<lambda>t. cl_state (cls s' (get_cl_txn t)))
+    (svr_state (svrs s k)) (svr_key_fp (svrs s k)) (svr_vl (svrs s k)))"
+    and "i \<notin> full_view (update_kv_all_txn (\<lambda>t. cl_state (cls s (get_cl_txn t)))
+    (svr_state (svrs s k)) (svr_key_fp (svrs s k)) (svr_vl (svrs s k)))"
   shows "i = length (svr_vl (svrs s k))"
   oops
 
 lemma t_is_fresh:
   assumes "SqnInv s cl"
-    and "tm_state (cls s cl) = tm_prepared"
+    and "cl_state (cls s cl) = cl_prepared"
   shows "get_txn_cl cl s \<in> next_txids (kvs_of_gs s) cl"
   oops
 
@@ -387,10 +387,10 @@ lemma kvs_of_gs_view_atomic:
     and "\<And>k. WLockInv s k" and "\<And>k. WLockFpInv s k"
     and "\<And>k. RLockInv s k" and "\<And>k. NoLockFpInv s k"
     and "SqnInv s cl" and "KVSNonEmp s"
-    and "tm_state (cls s cl) = tm_prepared"
-    and "tm_state (cls s' cl) = tm_committed"
-    and "\<forall>k. km_state (svrs s k) (get_txn_cl cl s) \<in> {read_lock, write_lock, no_lock}"
-    and "km_tm_cl'_unchanged cl s s'"
+    and "cl_state (cls s cl) = cl_prepared"
+    and "cl_state (cls s' cl) = cl_committed"
+    and "\<forall>k. svr_state (svrs s k) (get_txn_cl cl s) \<in> {read_lock, write_lock, no_lock}"
+    and "svr_cl_cl'_unchanged cl s s'"
   shows "view_atomic (kvs_of_gs s') (\<lambda>k. full_view (kvs_of_gs s k))"
   oops
 
