txn-data-consistency/Serializable_2PC_2PL_proof.thy
@@ -17,7 +17,7 @@ lemma expanding_feature3':
 \<comment> \<open>Invariant about future and past transactions svrs\<close>
 
 definition TIDFutureKm where
-  "TIDFutureKm s cl \<longleftrightarrow> (\<forall>n k. n > cl_sn (cls s cl) \<longrightarrow> km_state (svrs s k) (Tn_cl n cl) = working)"
+  "TIDFutureKm s cl \<longleftrightarrow> (\<forall>n k. n > cl_sn (cls s cl) \<longrightarrow> svr_state (svrs s k) (Tn_cl n cl) = working)"
 
 lemmas TIDFutureKmI = TIDFutureKm_def[THEN iffD2, rule_format]
 lemmas TIDFutureKmE[elim] = TIDFutureKm_def[THEN iffD1, elim_format, rule_format]
@@ -33,70 +33,70 @@ next
   proof (cases e)
     case (Prepare x31 x32)
     then show ?thesis using reach_trans
-      apply (auto simp add: tps_trans_defs km_unchanged_defs tid_match_def TIDFutureKm_def)
+      apply (auto simp add: tps_trans_defs svr_unchanged_defs tid_match_def TIDFutureKm_def)
       subgoal for n k apply (cases "(Tn_cl n x) = x32"; cases "k = x31", auto) done.
   next
     case (RLock x41 x42 x43)
     then show ?thesis using reach_trans
-      apply (auto simp add: tps_trans_defs km_unchanged_defs TIDFutureKm_def)
-      by (metis state_km.distinct(1))
+      apply (auto simp add: tps_trans_defs svr_unchanged_defs TIDFutureKm_def)
+      by (metis state_svr.distinct(1))
   next
     case (WLock x51 x52 x53 x54)
     then show ?thesis using reach_trans
-      apply (auto simp add: tps_trans_defs km_unchanged_defs TIDFutureKm_def)
-      by (metis state_km.distinct(1))+
+      apply (auto simp add: tps_trans_defs svr_unchanged_defs TIDFutureKm_def)
+      by (metis state_svr.distinct(1))+
   next
     case (NoLock x61 x62)
     then show ?thesis using reach_trans
-      apply (auto simp add: tps_trans_defs km_unchanged_defs TIDFutureKm_def)
-      by (metis state_km.distinct(1))
+      apply (auto simp add: tps_trans_defs svr_unchanged_defs TIDFutureKm_def)
+      by (metis state_svr.distinct(1))
   next
     case (NOK x71 x72)
     then show ?thesis using reach_trans
-      apply (auto simp add: tps_trans_defs km_unchanged_defs TIDFutureKm_def)
-      by (metis state_km.distinct(1))+
+      apply (auto simp add: tps_trans_defs svr_unchanged_defs TIDFutureKm_def)
+      by (metis state_svr.distinct(1))+
   next
     case (Commit x81 x82)
     then show ?thesis using reach_trans
-      apply (auto simp add: tps_trans_defs km_unchanged_defs TIDFutureKm_def)
-      apply (metis state_km.distinct(3))
-      apply (metis state_km.distinct(5))
-      by (metis state_km.distinct(7))
+      apply (auto simp add: tps_trans_defs svr_unchanged_defs TIDFutureKm_def)
+      apply (metis state_svr.distinct(3))
+      apply (metis state_svr.distinct(5))
+      by (metis state_svr.distinct(7))
   next
     case (Abort x91 x92)
     then show ?thesis using reach_trans
-      apply (auto simp add: tps_trans_defs km_unchanged_defs TIDFutureKm_def)
-      apply (metis state_km.distinct(3))
-      apply (metis state_km.distinct(5))
-      apply (metis state_km.distinct(7))
-      by (metis state_km.distinct(9))
+      apply (auto simp add: tps_trans_defs svr_unchanged_defs TIDFutureKm_def)
+      apply (metis state_svr.distinct(3))
+      apply (metis state_svr.distinct(5))
+      apply (metis state_svr.distinct(7))
+      by (metis state_svr.distinct(9))
   next
     case (User_Commit x10)
     then show ?thesis using reach_trans
-      by (auto simp add: tps_trans_defs tm_unchanged_defs TIDFutureKm_def, metis)
+      by (auto simp add: tps_trans_defs cl_unchanged_defs TIDFutureKm_def, metis)
   next
-    case (TM_Commit x111 x112 x113 x114)
+    case (Cl_Commit x111 x112 x113 x114)
     then show ?thesis using reach_trans
-      by (auto simp add: tps_trans_defs tm_unchanged_defs TIDFutureKm_def, metis)
+      by (auto simp add: tps_trans_defs cl_unchanged_defs TIDFutureKm_def, metis)
   next
-    case (TM_Abort x12a)
+    case (Cl_Abort x12a)
     then show ?thesis using reach_trans
-      by (auto simp add: tps_trans_defs tm_unchanged_defs TIDFutureKm_def, metis)
+      by (auto simp add: tps_trans_defs cl_unchanged_defs TIDFutureKm_def, metis)
   next
-    case (TM_ReadyC x13a)
+    case (Cl_ReadyC x13a)
     then show ?thesis using reach_trans
-      apply (auto simp add: tps_trans_defs tm_unchanged_defs TIDFutureKm_def)
+      apply (auto simp add: tps_trans_defs cl_unchanged_defs TIDFutureKm_def)
       by (metis Suc_lessD)
   next
-    case (TM_ReadyA x14)
+    case (Cl_ReadyA x14)
     then show ?thesis using reach_trans
-      apply (auto simp add: tps_trans_defs tm_unchanged_defs TIDFutureKm_def)
+      apply (auto simp add: tps_trans_defs cl_unchanged_defs TIDFutureKm_def)
       by (metis Suc_lessD)
   qed simp
 qed
 
 definition TIDPastKm where
-  "TIDPastKm s cl \<longleftrightarrow> (\<forall>n k. n < cl_sn (cls s cl) \<longrightarrow> km_state (svrs s k) (Tn_cl n cl) \<in> {committed, aborted})"
+  "TIDPastKm s cl \<longleftrightarrow> (\<forall>n k. n < cl_sn (cls s cl) \<longrightarrow> svr_state (svrs s k) (Tn_cl n cl) \<in> {committed, aborted})"
 
 lemmas TIDPastKmI = TIDPastKm_def[THEN iffD2, rule_format]
 lemmas TIDPastKmE[elim] = TIDPastKm_def[THEN iffD1, elim_format, rule_format]
@@ -112,57 +112,57 @@ next
   proof (cases e)
     case (Prepare x31 x32)
     then show ?thesis using reach_trans
-      apply (auto simp add: tps_trans_defs km_unchanged_defs TIDPastKm_def)
-      by (metis state_km.distinct(11) state_km.distinct(13))
+      apply (auto simp add: tps_trans_defs svr_unchanged_defs TIDPastKm_def)
+      by (metis state_svr.distinct(11) state_svr.distinct(13))
   next
     case (RLock x41 x42 x43)
     then show ?thesis using reach_trans
-      apply (auto simp add: tps_trans_defs km_unchanged_defs TIDPastKm_def)
-      by (metis state_km.distinct(23) state_km.distinct(25))
+      apply (auto simp add: tps_trans_defs svr_unchanged_defs TIDPastKm_def)
+      by (metis state_svr.distinct(23) state_svr.distinct(25))
   next
     case (WLock x51 x52 x53 x54)
     then show ?thesis using reach_trans
-      apply (auto simp add: tps_trans_defs km_unchanged_defs TIDPastKm_def)
-      by (metis state_km.distinct(23) state_km.distinct(25))+
+      apply (auto simp add: tps_trans_defs svr_unchanged_defs TIDPastKm_def)
+      by (metis state_svr.distinct(23) state_svr.distinct(25))+
   next
     case (NoLock x61 x62)
     then show ?thesis using reach_trans
-      apply (auto simp add: tps_trans_defs km_unchanged_defs TIDPastKm_def)
-      by (metis state_km.distinct(23) state_km.distinct(25))
+      apply (auto simp add: tps_trans_defs svr_unchanged_defs TIDPastKm_def)
+      by (metis state_svr.distinct(23) state_svr.distinct(25))
   next
     case (NOK x71 x72)
     then show ?thesis using reach_trans
-      apply (auto simp add: tps_trans_defs km_unchanged_defs TIDPastKm_def)
-      by (metis state_km.distinct(23) state_km.distinct(25))+
+      apply (auto simp add: tps_trans_defs svr_unchanged_defs TIDPastKm_def)
+      by (metis state_svr.distinct(23) state_svr.distinct(25))+
   next
     case (Commit x81 x82)
     then show ?thesis using reach_trans
-      by (auto simp add: tps_trans_defs km_unchanged_defs TIDPastKm_def, fastforce+)
+      by (auto simp add: tps_trans_defs svr_unchanged_defs TIDPastKm_def, fastforce+)
   next
     case (Abort x91 x92)
     then show ?thesis using reach_trans
-      by (auto simp add: tps_trans_defs km_unchanged_defs TIDPastKm_def, fastforce+)
+      by (auto simp add: tps_trans_defs svr_unchanged_defs TIDPastKm_def, fastforce+)
   next
     case (User_Commit x10)
     then show ?thesis using reach_trans
-      by (auto simp add: tps_trans_defs tm_unchanged_defs TIDPastKm_def, metis)
+      by (auto simp add: tps_trans_defs cl_unchanged_defs TIDPastKm_def, metis)
   next
-    case (TM_Commit x111 x112 x113 x114)
+    case (Cl_Commit x111 x112 x113 x114)
     then show ?thesis using reach_trans
-      by (auto simp add: tps_trans_defs tm_unchanged_defs TIDPastKm_def, metis)
+      by (auto simp add: tps_trans_defs cl_unchanged_defs TIDPastKm_def, metis)
   next
-    case (TM_Abort x12a)
+    case (Cl_Abort x12a)
     then show ?thesis using reach_trans
-      by (auto simp add: tps_trans_defs tm_unchanged_defs TIDPastKm_def, metis)
+      by (auto simp add: tps_trans_defs cl_unchanged_defs TIDPastKm_def, metis)
   next
-    case (TM_ReadyC x13a)
+    case (Cl_ReadyC x13a)
     then show ?thesis using reach_trans
-      apply (auto simp add: tps_trans_defs tm_unchanged_defs TIDPastKm_def)
+      apply (auto simp add: tps_trans_defs cl_unchanged_defs TIDPastKm_def)
         by (metis less_antisym)
   next
-    case (TM_ReadyA x14)
+    case (Cl_ReadyA x14)
     then show ?thesis using reach_trans
-      apply (auto simp add: tps_trans_defs tm_unchanged_defs TIDPastKm_def)
+      apply (auto simp add: tps_trans_defs cl_unchanged_defs TIDPastKm_def)
         by (metis less_antisym)
   qed auto
 qed
@@ -170,7 +170,7 @@ qed
 \<comment> \<open>Lock Invariants\<close>
 
 definition RLockInv where
-  "RLockInv s k \<longleftrightarrow> (\<forall>t. km_state (svrs s k) t = read_lock \<longrightarrow> (\<forall>t. km_state (svrs s k) t \<noteq> write_lock))"
+  "RLockInv s k \<longleftrightarrow> (\<forall>t. svr_state (svrs s k) t = read_lock \<longrightarrow> (\<forall>t. svr_state (svrs s k) t \<noteq> write_lock))"
 
 lemmas RLockInvI = RLockInv_def[THEN iffD2, rule_format]
 lemmas RLockInvE[elim] = RLockInv_def[THEN iffD1, elim_format, rule_format]
@@ -186,51 +186,51 @@ next
   proof (induction e)
     case (Prepare x1 x2)
     then show ?case using reach_trans
-      apply (auto simp add: tps_trans_defs km_unchanged_defs RLockInv_def)
-      by (metis state_km.distinct(15) state_km.distinct(17))
+      apply (auto simp add: tps_trans_defs svr_unchanged_defs RLockInv_def)
+      by (metis state_svr.distinct(15) state_svr.distinct(17))
   next
     case (RLock x1 x2 x3)
     then show ?case using reach_trans
-      apply (auto simp add: tps_trans_defs km_unchanged_defs RLockInv_def)
-      by (metis state_km.distinct(27))
+      apply (auto simp add: tps_trans_defs svr_unchanged_defs RLockInv_def)
+      by (metis state_svr.distinct(27))
   next
     case (WLock x1 x2 x3 x4)
     then show ?case using reach_trans
-      apply (auto simp add: tps_trans_defs km_unchanged_defs RLockInv_def)
-      by (metis state_km.distinct(27))+
+      apply (auto simp add: tps_trans_defs svr_unchanged_defs RLockInv_def)
+      by (metis state_svr.distinct(27))+
   next
     case (NoLock x1 x2)
     then show ?case using reach_trans
-      apply (auto simp add: tps_trans_defs km_unchanged_defs RLockInv_def)
-      by (metis state_km.distinct(30) state_km.distinct(38))
+      apply (auto simp add: tps_trans_defs svr_unchanged_defs RLockInv_def)
+      by (metis state_svr.distinct(30) state_svr.distinct(38))
   next
     case (NOK x1 x2)
     then show ?case using reach_trans
-      apply (auto simp add: tps_trans_defs km_unchanged_defs RLockInv_def)
-      by (metis state_km.distinct(31) state_km.distinct(39))
-      (*apply (metis state_km.distinct(31))
-      apply (metis state_km.distinct(31))
-      by (metis state_km.distinct(40))*)
+      apply (auto simp add: tps_trans_defs svr_unchanged_defs RLockInv_def)
+      by (metis state_svr.distinct(31) state_svr.distinct(39))
+      (*apply (metis state_svr.distinct(31))
+      apply (metis state_svr.distinct(31))
+      by (metis state_svr.distinct(40))*)
   next
     case (Commit x1 x2)
     then show ?case using reach_trans
-      apply (auto simp add: tps_trans_defs km_unchanged_defs RLockInv_def)
-      apply (metis state_km.distinct(42))
-      apply (metis state_km.distinct(34))
-      by (metis state_km.distinct(34) state_km.distinct(42))
+      apply (auto simp add: tps_trans_defs svr_unchanged_defs RLockInv_def)
+      apply (metis state_svr.distinct(42))
+      apply (metis state_svr.distinct(34))
+      by (metis state_svr.distinct(34) state_svr.distinct(42))
   next
     case (Abort x1 x2)
     then show ?case using reach_trans
-      apply (auto simp add: tps_trans_defs km_unchanged_defs RLockInv_def)
-      apply (metis state_km.distinct(44))
-      apply (metis state_km.distinct(36))
-      apply (metis state_km.distinct(36) state_km.distinct(44))
-      by (metis state_km.distinct(35) state_km.distinct(44))
-  qed (auto simp add: tps_trans_defs tm_unchanged_defs RLockInv_def)
+      apply (auto simp add: tps_trans_defs svr_unchanged_defs RLockInv_def)
+      apply (metis state_svr.distinct(44))
+      apply (metis state_svr.distinct(36))
+      apply (metis state_svr.distinct(36) state_svr.distinct(44))
+      by (metis state_svr.distinct(35) state_svr.distinct(44))
+  qed (auto simp add: tps_trans_defs cl_unchanged_defs RLockInv_def)
 qed
 
 definition WLockInv where
-  "WLockInv s k \<longleftrightarrow> (\<forall>t. km_state (svrs s k) t \<noteq> write_lock) \<or> (\<exists>! t. km_state (svrs s k) t = write_lock)"
+  "WLockInv s k \<longleftrightarrow> (\<forall>t. svr_state (svrs s k) t \<noteq> write_lock) \<or> (\<exists>! t. svr_state (svrs s k) t = write_lock)"
 
 lemmas WLockInvI = WLockInv_def[THEN iffD2, rule_format]
 lemmas WLockInvE[elim] = WLockInv_def[THEN iffD1, elim_format, rule_format]
@@ -246,47 +246,47 @@ next
   proof (cases e)
     case (Prepare x31 x32)
     then show ?thesis using reach_trans
-      apply (auto simp add: tps_trans_defs km_unchanged_defs WLockInv_def)
-      by (metis state_km.distinct(17))
+      apply (auto simp add: tps_trans_defs svr_unchanged_defs WLockInv_def)
+      by (metis state_svr.distinct(17))
   next
     case (RLock x41 x42 x43)
     then show ?thesis using reach_trans
-      apply (auto simp add: tps_trans_defs km_unchanged_defs WLockInv_def)
-      by (metis state_km.distinct(27))
+      apply (auto simp add: tps_trans_defs svr_unchanged_defs WLockInv_def)
+      by (metis state_svr.distinct(27))
   next
     case (WLock x51 x52 x53 x54)
     then show ?thesis using reach_trans
-      apply (auto simp add: tps_trans_defs km_unchanged_defs WLockInv_def)
+      apply (auto simp add: tps_trans_defs svr_unchanged_defs WLockInv_def)
       by metis+
   next
     case (NoLock x61 x62)
     then show ?thesis using reach_trans
-      apply (auto simp add: tps_trans_defs km_unchanged_defs WLockInv_def)
-      by (metis state_km.distinct(37))
+      apply (auto simp add: tps_trans_defs svr_unchanged_defs WLockInv_def)
+      by (metis state_svr.distinct(37))
   next
     case (NOK x71 x72)
     then show ?thesis using reach_trans
-      apply (auto simp add: tps_trans_defs km_unchanged_defs WLockInv_def)
-      by (metis state_km.distinct(39))+
+      apply (auto simp add: tps_trans_defs svr_unchanged_defs WLockInv_def)
+      by (metis state_svr.distinct(39))+
   next
     case (Commit x81 x82)
     then show ?thesis using reach_trans
-      apply (auto simp add: tps_trans_defs km_unchanged_defs WLockInv_def)
-      by (metis state_km.distinct(41))+
+      apply (auto simp add: tps_trans_defs svr_unchanged_defs WLockInv_def)
+      by (metis state_svr.distinct(41))+
   next
     case (Abort x91 x92)
     then show ?thesis using reach_trans
-      apply (auto simp add: tps_trans_defs km_unchanged_defs WLockInv_def)
-      by (metis state_km.distinct(43))+
-  qed (auto simp add: tps_trans_defs tm_unchanged_defs WLockInv_def)
+      apply (auto simp add: tps_trans_defs svr_unchanged_defs WLockInv_def)
+      by (metis state_svr.distinct(43))+
+  qed (auto simp add: tps_trans_defs cl_unchanged_defs WLockInv_def)
 qed
 
 \<comment> \<open>Simulation function lemmas\<close>
 
 lemma the_wr_tI:
-  assumes "km_state (svrs s k) t = write_lock"
+  assumes "svr_state (svrs s k) t = write_lock"
       and "WLockInv s k"
-  shows "the_wr_t (km_state (svrs s k)) = t"
+  shows "the_wr_t (svr_state (svrs s k)) = t"
   using assms
   by blast
 
@@ -341,30 +341,30 @@ lemma update_kv_all_txn_non_empty [simp]:
   by (metis update_kv_all_txn_length_increasing le_zero_eq length_0_conv)
 
 lemma read_only_update [simp]:
-  assumes "\<And>t. km_state (svrs s k) t \<noteq> write_lock"
-  shows "update_kv_all_txn tStm (km_state (svrs s k)) tFk vl =
-         update_kv_reads_all_txn tStm (km_state (svrs s k)) tFk vl"
+  assumes "\<And>t. svr_state (svrs s k) t \<noteq> write_lock"
+  shows "update_kv_all_txn tStm (svr_state (svrs s k)) tFk vl =
+         update_kv_reads_all_txn tStm (svr_state (svrs s k)) tFk vl"
   using assms
   by (auto simp add: update_kv_all_txn_def update_kv_writes_all_txn_def)
 
 lemma read_only_update':
   assumes "RLockInv s k"
-    and "km_state (svrs s k) t = read_lock"
-  shows "update_kv_all_txn tStm (km_state (svrs s k)) tFk vl =
-         update_kv_reads_all_txn tStm (km_state (svrs s k)) tFk vl"
+    and "svr_state (svrs s k) t = read_lock"
+  shows "update_kv_all_txn tStm (svr_state (svrs s k)) tFk vl =
+         update_kv_reads_all_txn tStm (svr_state (svrs s k)) tFk vl"
   using assms
   by (meson RLockInv_def read_only_update)
 
 lemma writer_update_before:
   assumes "WLockInv s k"
-    and "tm_state (cls s cl) = tm_prepared"
-    and "km_state (svrs s k) (get_txn_cl cl s) = write_lock"
-  shows "update_kv_all_txn (\<lambda>t. tm_state (cls s (get_cl_txn t))) (km_state (svrs s k)) tFk vl =
-         update_kv_reads_all_txn (\<lambda>t. tm_state (cls s (get_cl_txn t))) (km_state (svrs s k)) tFk vl"
+    and "cl_state (cls s cl) = cl_prepared"
+    and "svr_state (svrs s k) (get_txn_cl cl s) = write_lock"
+  shows "update_kv_all_txn (\<lambda>t. cl_state (cls s (get_cl_txn t))) (svr_state (svrs s k)) tFk vl =
+         update_kv_reads_all_txn (\<lambda>t. cl_state (cls s (get_cl_txn t))) (svr_state (svrs s k)) tFk vl"
   using assms
   apply (auto simp add: update_kv_all_txn_def update_kv_writes_all_txn_def update_kv_writes_def
       WLockInv_def split: option.split)
-  by (metis state_tm.distinct(7) txid0.sel(2))
+  by (metis state_cl.distinct(7) txid0.sel(2))
 
 
 \<comment> \<open>lemmas for unchanged elements in svrs\<close>
@@ -393,7 +393,7 @@ lemma eq_for_all_cl:
 lemma other_sn_idle:  
   assumes "TIDFutureKm s cl" and "TIDPastKm s cl"
     and "get_cl_txn t = cl" and "get_sn_txn t \<noteq> cl_sn (cls s cl)"
-  shows "\<And>k. km_state (svrs s k) t \<in> {working, committed, aborted}"
+  shows "\<And>k. svr_state (svrs s k) t \<in> {working, committed, aborted}"
   using assms
   apply (auto simp add: TIDFutureKm_def TIDPastKm_def)
   apply (cases "get_sn_txn t > cl_sn (cls s cl)")
@@ -403,7 +403,7 @@ lemma other_sn_idle:
 \<comment> \<open>Invariants for fingerprint, knowing the lock (svrs status)\<close>
 
 definition RLockFpInv where
-  "RLockFpInv s k \<longleftrightarrow> (\<forall>t. km_state (svrs s k) t = read_lock \<longrightarrow>
+  "RLockFpInv s k \<longleftrightarrow> (\<forall>t. svr_state (svrs s k) t = read_lock \<longrightarrow>
     svr_key_fp (svrs s k) t W = None \<and>
     svr_key_fp (svrs s k) t R \<noteq> None)"
 
@@ -420,43 +420,43 @@ next
   proof (cases e)
     case (Prepare x31 x32)
     then show ?thesis using reach_trans
-      apply (auto simp add: tps_trans_defs km_unchanged_defs RLockFpInv_def)
-      by (metis state_km.distinct(15))+
+      apply (auto simp add: tps_trans_defs svr_unchanged_defs RLockFpInv_def)
+      by (metis state_svr.distinct(15))+
   next
     case (RLock x41 x42 x43)
     then show ?thesis using reach_trans
-      apply (auto simp add: tps_trans_defs km_unchanged_defs RLockFpInv_def)
+      apply (auto simp add: tps_trans_defs svr_unchanged_defs RLockFpInv_def)
       by metis+
   next
     case (WLock x51 x52 x53 x54)
     then show ?thesis using reach_trans
-      apply (auto simp add: tps_trans_defs km_unchanged_defs RLockFpInv_def)
-      by (metis state_km.distinct(27))+
+      apply (auto simp add: tps_trans_defs svr_unchanged_defs RLockFpInv_def)
+      by (metis state_svr.distinct(27))+
   next
     case (NoLock x61 x62)
     then show ?thesis using reach_trans
-      apply (auto simp add: tps_trans_defs km_unchanged_defs RLockFpInv_def)
-      by (metis state_km.distinct(29))+
+      apply (auto simp add: tps_trans_defs svr_unchanged_defs RLockFpInv_def)
+      by (metis state_svr.distinct(29))+
   next
     case (NOK x71 x72)
     then show ?thesis using reach_trans
-      apply (auto simp add: tps_trans_defs km_unchanged_defs RLockFpInv_def)
-      by (metis state_km.distinct(31))+
+      apply (auto simp add: tps_trans_defs svr_unchanged_defs RLockFpInv_def)
+      by (metis state_svr.distinct(31))+
   next
     case (Commit x81 x82)
     then show ?thesis using reach_trans
-      apply (auto simp add: tps_trans_defs km_unchanged_defs RLockFpInv_def)
-      by (metis state_km.distinct(33))+
+      apply (auto simp add: tps_trans_defs svr_unchanged_defs RLockFpInv_def)
+      by (metis state_svr.distinct(33))+
   next
     case (Abort x91 x92)
     then show ?thesis using reach_trans
-      apply (auto simp add: tps_trans_defs km_unchanged_defs RLockFpInv_def)
-      by (metis state_km.distinct(35))+
-  qed (auto simp add: tps_trans_defs tm_unchanged_defs RLockFpInv_def)
+      apply (auto simp add: tps_trans_defs svr_unchanged_defs RLockFpInv_def)
+      by (metis state_svr.distinct(35))+
+  qed (auto simp add: tps_trans_defs cl_unchanged_defs RLockFpInv_def)
 qed
 
 definition WLockFpInv where
-  "WLockFpInv s k \<longleftrightarrow> (\<forall>t. km_state (svrs s k) t = write_lock \<longrightarrow> svr_key_fp (svrs s k) t W \<noteq> None)"
+  "WLockFpInv s k \<longleftrightarrow> (\<forall>t. svr_state (svrs s k) t = write_lock \<longrightarrow> svr_key_fp (svrs s k) t W \<noteq> None)"
 
 lemmas WLockFpInvI = WLockFpInv_def[THEN iffD2, rule_format]
 lemmas WLockFpInvE[elim] = WLockFpInv_def[THEN iffD1, elim_format, rule_format]
@@ -471,43 +471,43 @@ next
   proof (cases e)
     case (Prepare x31 x32)
     then show ?thesis using reach_trans
-      apply (auto simp add: tps_trans_defs km_unchanged_defs WLockFpInv_def)
-      by (metis state_km.distinct(17))
+      apply (auto simp add: tps_trans_defs svr_unchanged_defs WLockFpInv_def)
+      by (metis state_svr.distinct(17))
   next
     case (RLock x41 x42 x43)
     then show ?thesis using reach_trans
-      apply (auto simp add: tps_trans_defs km_unchanged_defs WLockFpInv_def)
-      by (metis state_km.distinct(27))
+      apply (auto simp add: tps_trans_defs svr_unchanged_defs WLockFpInv_def)
+      by (metis state_svr.distinct(27))
   next
     case (WLock x51 x52 x53 x54)
     then show ?thesis using reach_trans
-      apply (auto simp add: tps_trans_defs km_unchanged_defs WLockFpInv_def)
+      apply (auto simp add: tps_trans_defs svr_unchanged_defs WLockFpInv_def)
       by metis+
   next
     case (NoLock x61 x62)
     then show ?thesis using reach_trans
-      apply (auto simp add: tps_trans_defs km_unchanged_defs WLockFpInv_def)
-      by (metis state_km.distinct(37))
+      apply (auto simp add: tps_trans_defs svr_unchanged_defs WLockFpInv_def)
+      by (metis state_svr.distinct(37))
   next
     case (NOK x71 x72)
     then show ?thesis using reach_trans
-      apply (auto simp add: tps_trans_defs km_unchanged_defs WLockFpInv_def)
-      by (metis state_km.distinct(39))
+      apply (auto simp add: tps_trans_defs svr_unchanged_defs WLockFpInv_def)
+      by (metis state_svr.distinct(39))
   next
     case (Commit x81 x82)
     then show ?thesis using reach_trans
-      apply (auto simp add: tps_trans_defs km_unchanged_defs WLockFpInv_def)
-      by (metis state_km.distinct(41))+
+      apply (auto simp add: tps_trans_defs svr_unchanged_defs WLockFpInv_def)
+      by (metis state_svr.distinct(41))+
   next
     case (Abort x91 x92)
     then show ?thesis using reach_trans
-      apply (auto simp add: tps_trans_defs km_unchanged_defs WLockFpInv_def)
-      by (metis state_km.distinct(43))+
-  qed (auto simp add: tps_trans_defs tm_unchanged_defs WLockFpInv_def)
+      apply (auto simp add: tps_trans_defs svr_unchanged_defs WLockFpInv_def)
+      by (metis state_svr.distinct(43))+
+  qed (auto simp add: tps_trans_defs cl_unchanged_defs WLockFpInv_def)
 qed
 
 definition NoLockFpInv where
-  "NoLockFpInv s k \<longleftrightarrow> (\<forall>t. km_state (svrs s k) t = no_lock \<longrightarrow>
+  "NoLockFpInv s k \<longleftrightarrow> (\<forall>t. svr_state (svrs s k) t = no_lock \<longrightarrow>
     svr_key_fp (svrs s k) t W = None \<and>
     svr_key_fp (svrs s k) t R = None)"
 
@@ -524,47 +524,47 @@ next
   proof (cases e)
     case (Prepare x31 x32)
     then show ?thesis using reach_trans
-      apply (auto simp add: tps_trans_defs km_unchanged_defs NoLockFpInv_def)
-      by (metis state_km.distinct(19))+
+      apply (auto simp add: tps_trans_defs svr_unchanged_defs NoLockFpInv_def)
+      by (metis state_svr.distinct(19))+
   next
     case (RLock x41 x42 x43)
     then show ?thesis using reach_trans
-      apply (auto simp add: tps_trans_defs km_unchanged_defs NoLockFpInv_def)
-      by (metis state_km.distinct(29))+
+      apply (auto simp add: tps_trans_defs svr_unchanged_defs NoLockFpInv_def)
+      by (metis state_svr.distinct(29))+
   next
     case (WLock x51 x52 x53 x54)
     then show ?thesis using reach_trans
-      apply (auto simp add: tps_trans_defs km_unchanged_defs NoLockFpInv_def)
-      apply (metis state_km.distinct(37), metis)
-      by (metis state_km.distinct(37))+
+      apply (auto simp add: tps_trans_defs svr_unchanged_defs NoLockFpInv_def)
+      apply (metis state_svr.distinct(37), metis)
+      by (metis state_svr.distinct(37))+
   next
     case (NoLock x61 x62)
     then show ?thesis using reach_trans
-      apply (auto simp add: tps_trans_defs km_unchanged_defs NoLockFpInv_def)
+      apply (auto simp add: tps_trans_defs svr_unchanged_defs NoLockFpInv_def)
       by metis+
   next
     case (NOK x71 x72)
     then show ?thesis using reach_trans
-      apply (auto simp add: tps_trans_defs km_unchanged_defs NoLockFpInv_def)
-      by (metis state_km.distinct(45))+
+      apply (auto simp add: tps_trans_defs svr_unchanged_defs NoLockFpInv_def)
+      by (metis state_svr.distinct(45))+
   next
     case (Commit x81 x82)
     then show ?thesis using reach_trans
-      apply (auto simp add: tps_trans_defs km_unchanged_defs NoLockFpInv_def)
-      by (metis state_km.distinct(47))+
+      apply (auto simp add: tps_trans_defs svr_unchanged_defs NoLockFpInv_def)
+      by (metis state_svr.distinct(47))+
   next
     case (Abort x91 x92)
     then show ?thesis using reach_trans
-      apply (auto simp add: tps_trans_defs km_unchanged_defs NoLockFpInv_def)
-      by (metis state_km.distinct(49))+
-  qed (auto simp add: tps_trans_defs tm_unchanged_defs NoLockFpInv_def)
+      apply (auto simp add: tps_trans_defs svr_unchanged_defs NoLockFpInv_def)
+      by (metis state_svr.distinct(49))+
+  qed (auto simp add: tps_trans_defs cl_unchanged_defs NoLockFpInv_def)
 qed
 
 lemma the_wr_t_fp:
   assumes "\<And>k. WLockInv s k"
     and "\<And>k. WLockFpInv s k"
-    and "km_state (svrs s k) t = write_lock"
-  shows "svr_key_fp (svrs s k) (the_wr_t (km_state (svrs s k))) W \<noteq> None"
+    and "svr_state (svrs s k) t = write_lock"
+  shows "svr_key_fp (svrs s k) (the_wr_t (svr_state (svrs s k))) W \<noteq> None"
   using assms by (auto simp add: WLockInv_def WLockFpInv_def the_wr_tI)
 
 \<comment> \<open>Invariants about kv store\<close>
@@ -585,7 +585,7 @@ next
   proof (induction e)
     case (Commit x1 x2)
     then show ?case using reach_trans
-      apply (auto simp add: KVSNonEmp_def tps_trans_defs km_unchanged_defs)
+      apply (auto simp add: KVSNonEmp_def tps_trans_defs svr_unchanged_defs)
       apply (metis bot_nat_0.not_eq_extremum full_view_def full_view_update_kv_writes
             length_0_conv lessThan_iff update_kv_writes_key_decides_length)
       apply (metis length_greater_0_conv update_kv_writes_key_decides_length
@@ -621,16 +621,16 @@ subsubsection \<open>Lemmas for kvs_of_gs changing by different events\<close>
 (*KM events*)
 
 \<comment> \<open>eligible reads and read updates\<close>
-lemma eligible_reads_km_inv:
+lemma eligible_reads_svr_inv:
   assumes "RLockInv s k"
-    and "(km_state (svrs s k) t \<notin> {write_lock, read_lock} \<and>
-          km_state (svrs s' k) t = km_state (svrs s k) t) \<or>
-          tm_state (cls s (get_cl_txn t)) \<noteq> tm_committed"
-    and "tm_km_k'_t'_unchanged k s s' t"
+    and "(svr_state (svrs s k) t \<notin> {write_lock, read_lock} \<and>
+          svr_state (svrs s' k) t = svr_state (svrs s k) t) \<or>
+          cl_state (cls s (get_cl_txn t)) \<noteq> cl_committed"
+    and "cl_svr_k'_t'_unchanged k s s' t"
   shows "
-  eligible_reads (\<lambda>t. tm_state (cls s' (get_cl_txn t))) (km_state (svrs s' k)) (svr_key_fp (svrs s' k)) t' =
-  eligible_reads (\<lambda>t. tm_state (cls s (get_cl_txn t))) (km_state (svrs s k)) (svr_key_fp (svrs s k)) t'"
-  using assms apply (cases "t' = t"; simp add: km_unchanged_defs) by metis
+  eligible_reads (\<lambda>t. cl_state (cls s' (get_cl_txn t))) (svr_state (svrs s' k)) (svr_key_fp (svrs s' k)) t' =
+  eligible_reads (\<lambda>t. cl_state (cls s (get_cl_txn t))) (svr_state (svrs s k)) (svr_key_fp (svrs s k)) t'"
+  using assms apply (cases "t' = t"; simp add: svr_unchanged_defs) by metis
 
 lemma none_eligible: "vl[Max (full_view vl) := last_version vl (full_view vl)
   \<lparr>v_readerset := v_readerset (last_version vl (full_view vl)) \<union> {}\<rparr>] = vl"
@@ -638,34 +638,34 @@ lemma none_eligible: "vl[Max (full_view vl) := last_version vl (full_view vl)
 
 lemma eligible_reads_read_lock_inv:
   assumes "RLockFpInv s k"
-    and "km_state (svrs s k) t = read_lock"
-    and "tm_state (cls s (get_cl_txn t)) = tm_committed"
-    and "tm_km_k'_t'_unchanged k s s' t"
-  shows "{t. eligible_reads (\<lambda>t. tm_state (cls s (get_cl_txn t))) (km_state (svrs s k))
+    and "svr_state (svrs s k) t = read_lock"
+    and "cl_state (cls s (get_cl_txn t)) = cl_committed"
+    and "cl_svr_k'_t'_unchanged k s s' t"
+  shows "{t. eligible_reads (\<lambda>t. cl_state (cls s (get_cl_txn t))) (svr_state (svrs s k))
             (svr_key_fp (svrs s k)) t} =
-          insert t {t. eligible_reads (\<lambda>t. tm_state (cls s (get_cl_txn t))) (km_state (svrs s' k))
+          insert t {t. eligible_reads (\<lambda>t. cl_state (cls s (get_cl_txn t))) (svr_state (svrs s' k))
             (svr_key_fp (svrs s k)) t}"
-  using assms by (auto simp add: km_unchanged_defs)
+  using assms by (auto simp add: svr_unchanged_defs)
 
 lemma eligible_reads_write_lock_s_the_t:
   assumes "RLockInv s k" and "WLockInv s k"
-    and "km_state (svrs s k) t = write_lock"
-    and "tm_state (cls s (get_cl_txn t)) = tm_committed"
-    and "tm_km_k'_t'_unchanged k s s' t"
-  shows "{t. eligible_reads (\<lambda>t. tm_state (cls s (get_cl_txn t))) (km_state (svrs s k))
+    and "svr_state (svrs s k) t = write_lock"
+    and "cl_state (cls s (get_cl_txn t)) = cl_committed"
+    and "cl_svr_k'_t'_unchanged k s s' t"
+  shows "{t. eligible_reads (\<lambda>t. cl_state (cls s (get_cl_txn t))) (svr_state (svrs s k))
             (svr_key_fp (svrs s k)) t} =
          (case (svr_key_fp (svrs s k) t R) of None \<Rightarrow> {} | Some y \<Rightarrow> {t})"
   using assms
   apply (auto intro: Collect_empty_eq split: option.split)
-  subgoal for t' by (cases "t' = t"; auto simp add: RLockInv_def WLockInv_def km_unchanged_defs).
+  subgoal for t' by (cases "t' = t"; auto simp add: RLockInv_def WLockInv_def svr_unchanged_defs).
 
 lemma update_kv_reads_commit_w_s_inv:
   assumes "RLockInv s k" and "WLockInv s k"
-    and "km_state (svrs s k) t = write_lock"
-    and "tm_state (cls s (get_cl_txn t)) = tm_committed"
-    and "tm_km_k'_t'_unchanged k s s' t"
-  shows "update_kv_reads_all_txn (\<lambda>t. tm_state (cls s (get_cl_txn t))) 
-                (km_state (svrs s k)) (svr_key_fp (svrs s k)) vl =
+    and "svr_state (svrs s k) t = write_lock"
+    and "cl_state (cls s (get_cl_txn t)) = cl_committed"
+    and "cl_svr_k'_t'_unchanged k s s' t"
+  shows "update_kv_reads_all_txn (\<lambda>t. cl_state (cls s (get_cl_txn t))) 
+                (svr_state (svrs s k)) (svr_key_fp (svrs s k)) vl =
         (case (svr_key_fp (svrs s k) t R) of None \<Rightarrow> vl | Some y \<Rightarrow> 
           vl[Max (full_view vl) := last_version vl (full_view vl)
                 \<lparr>v_readerset := v_readerset (last_version vl (full_view vl)) \<union> {t}\<rparr>])"
@@ -674,206 +674,206 @@ lemma update_kv_reads_commit_w_s_inv:
 
 lemma eligible_reads_write_lock_s'_empty:
   assumes "RLockInv s k" and "WLockInv s k"
-    and "km_state (svrs s k) t = write_lock"
-    and "km_state (svrs s' k) t = committed"
-    and "tm_km_k'_t'_unchanged k s s' t"
-  shows "{t. eligible_reads (\<lambda>t. tm_state (cls s (get_cl_txn t))) (km_state (svrs s' k))
+    and "svr_state (svrs s k) t = write_lock"
+    and "svr_state (svrs s' k) t = committed"
+    and "cl_svr_k'_t'_unchanged k s s' t"
+  shows "{t. eligible_reads (\<lambda>t. cl_state (cls s (get_cl_txn t))) (svr_state (svrs s' k))
             (svr_key_fp (svrs s k)) t} = {}"
   using assms
   apply (auto intro: Collect_empty_eq)
-  subgoal for t' by (cases "t' = t"; auto simp add: RLockInv_def WLockInv_def km_unchanged_defs)
-  subgoal for t' by (cases "t' = t"; auto simp add: RLockInv_def WLockInv_def km_unchanged_defs).
+  subgoal for t' by (cases "t' = t"; auto simp add: RLockInv_def WLockInv_def svr_unchanged_defs)
+  subgoal for t' by (cases "t' = t"; auto simp add: RLockInv_def WLockInv_def svr_unchanged_defs).
 
 lemma update_kv_reads_commit_w_s'_inv:
   assumes "RLockInv s k" and "WLockInv s k"
-    and "km_state (svrs s k) t = write_lock"
-    and "km_state (svrs s' k) t = committed"
-    and "tm_km_k'_t'_unchanged k s s' t"
-  shows "update_kv_reads_all_txn (\<lambda>t. tm_state (cls s (get_cl_txn t))) (km_state (svrs s' k))
+    and "svr_state (svrs s k) t = write_lock"
+    and "svr_state (svrs s' k) t = committed"
+    and "cl_svr_k'_t'_unchanged k s s' t"
+  shows "update_kv_reads_all_txn (\<lambda>t. cl_state (cls s (get_cl_txn t))) (svr_state (svrs s' k))
     (svr_key_fp (svrs s k)) vl = vl"
   using assms eligible_reads_write_lock_s'_empty[of s k t s']
   unfolding update_kv_reads_all_defs
   by (metis (lifting) last_version_def none_eligible version.unfold_congs(3))
 
 lemma eligible_reads_no_lock_inv:
-  assumes "km_state (svrs s k) t = no_lock"
-    and "km_state (svrs s' k) t = committed"
-    and "tm_km_k'_t'_unchanged k s s' t"
+  assumes "svr_state (svrs s k) t = no_lock"
+    and "svr_state (svrs s' k) t = committed"
+    and "cl_svr_k'_t'_unchanged k s s' t"
   shows "
-  eligible_reads (\<lambda>t. tm_state (cls s (get_cl_txn t))) (km_state (svrs s' k)) (svr_key_fp (svrs s k)) t' =
-  eligible_reads (\<lambda>t. tm_state (cls s (get_cl_txn t))) (km_state (svrs s k)) (svr_key_fp (svrs s k)) t'"
-  using assms apply (auto simp add: km_unchanged_defs)
-  apply (metis state_km.distinct(33))
-  apply (metis state_km.distinct(41))
-  apply (metis state_km.distinct(29))
-  by (metis state_km.distinct(37))
+  eligible_reads (\<lambda>t. cl_state (cls s (get_cl_txn t))) (svr_state (svrs s' k)) (svr_key_fp (svrs s k)) t' =
+  eligible_reads (\<lambda>t. cl_state (cls s (get_cl_txn t))) (svr_state (svrs s k)) (svr_key_fp (svrs s k)) t'"
+  using assms apply (auto simp add: svr_unchanged_defs)
+  apply (metis state_svr.distinct(33))
+  apply (metis state_svr.distinct(41))
+  apply (metis state_svr.distinct(29))
+  by (metis state_svr.distinct(37))
 
 \<comment> \<open>write updates\<close>
-lemma update_kv_writes_km_inv:
+lemma update_kv_writes_svr_inv:
   assumes "WLockInv s k"
-    and "(\<forall>t. km_state (svrs s k) t \<noteq> write_lock) \<or> 
-              km_state (svrs s' k) t \<noteq> write_lock"
-    and "tm_state (cls s (get_cl_txn t)) \<noteq> tm_committed"
-    and "tm_km_k'_t'_unchanged k s s' t"
-  shows "update_kv_writes_all_txn (\<lambda>t. tm_state (cls s (get_cl_txn t)))
-                (km_state (svrs s' k')) (svr_key_fp (svrs s' k')) vl =
-               update_kv_writes_all_txn (\<lambda>t. tm_state (cls s (get_cl_txn t)))
-                (km_state (svrs s k')) (svr_key_fp (svrs s k')) vl"
+    and "(\<forall>t. svr_state (svrs s k) t \<noteq> write_lock) \<or> 
+              svr_state (svrs s' k) t \<noteq> write_lock"
+    and "cl_state (cls s (get_cl_txn t)) \<noteq> cl_committed"
+    and "cl_svr_k'_t'_unchanged k s s' t"
+  shows "update_kv_writes_all_txn (\<lambda>t. cl_state (cls s (get_cl_txn t)))
+                (svr_state (svrs s' k')) (svr_key_fp (svrs s' k')) vl =
+               update_kv_writes_all_txn (\<lambda>t. cl_state (cls s (get_cl_txn t)))
+                (svr_state (svrs s k')) (svr_key_fp (svrs s k')) vl"
   using assms apply (auto simp add: update_kv_writes_all_txn_def)
-  apply (cases "k' = k"; simp add: km_unchanged_defs)
-  subgoal for t' by (cases "k' = k"; cases "t' = t"; simp add: km_unchanged_defs)
-  apply (cases "k' = k"; simp add: km_unchanged_defs)
-  apply (cases "k' = k", simp_all add: km_unchanged_defs, smt (verit) WLockInv_def theI)
-  subgoal for t' by (cases "k' = k"; cases "t' = t"; simp add: km_unchanged_defs the_wr_tI)
-  by (cases "k' = k"; auto simp add: km_unchanged_defs the_wr_tI)
+  apply (cases "k' = k"; simp add: svr_unchanged_defs)
+  subgoal for t' by (cases "k' = k"; cases "t' = t"; simp add: svr_unchanged_defs)
+  apply (cases "k' = k"; simp add: svr_unchanged_defs)
+  apply (cases "k' = k", simp_all add: svr_unchanged_defs, smt (verit) WLockInv_def theI)
+  subgoal for t' by (cases "k' = k"; cases "t' = t"; simp add: svr_unchanged_defs the_wr_tI)
+  by (cases "k' = k"; auto simp add: svr_unchanged_defs the_wr_tI)
 
 lemma update_kv_writes_commit_r_inv:
   assumes "RLockInv s k"
-    and "km_state (svrs s k) t = read_lock"
-    and "km_state (svrs s' k) t = committed"
-    and "tm_km_k'_t'_unchanged k s s' t"
-  shows "update_kv_writes_all_txn tStm (km_state (svrs s' k)) (svr_key_fp (svrs s k)) vl = 
-         update_kv_writes_all_txn tStm (km_state (svrs s k)) (svr_key_fp (svrs s k)) vl"
-  using assms apply (auto simp add: update_kv_writes_all_txn_def km_unchanged_defs)
-  by (metis state_km.distinct(41))
+    and "svr_state (svrs s k) t = read_lock"
+    and "svr_state (svrs s' k) t = committed"
+    and "cl_svr_k'_t'_unchanged k s s' t"
+  shows "update_kv_writes_all_txn tStm (svr_state (svrs s' k)) (svr_key_fp (svrs s k)) vl = 
+         update_kv_writes_all_txn tStm (svr_state (svrs s k)) (svr_key_fp (svrs s k)) vl"
+  using assms apply (auto simp add: update_kv_writes_all_txn_def svr_unchanged_defs)
+  by (metis state_svr.distinct(41))
 
 lemma update_kv_writes_commit_w_s_inv:
   assumes "WLockInv s k"
-    and "km_state (svrs s k) t = write_lock"
-    and "tm_state (cls s (get_cl_txn t)) = tm_committed"
-    and "tm_km_k'_t'_unchanged k s s' t"
-  shows "update_kv_writes_all_txn (\<lambda>t. tm_state (cls s (get_cl_txn t))) (km_state (svrs s k))
+    and "svr_state (svrs s k) t = write_lock"
+    and "cl_state (cls s (get_cl_txn t)) = cl_committed"
+    and "cl_svr_k'_t'_unchanged k s s' t"
+  shows "update_kv_writes_all_txn (\<lambda>t. cl_state (cls s (get_cl_txn t))) (svr_state (svrs s k))
            (svr_key_fp (svrs s k)) vl = update_kv_writes t (svr_key_fp (svrs s k) t) vl"
   using assms apply (auto simp add: update_kv_writes_all_txn_def)
   using the_wr_tI by blast
 
 lemma update_kv_writes_commit_w_s'_inv:
   assumes "WLockInv s k"
-    and "km_state (svrs s k) t = write_lock"
-    and "km_state (svrs s' k) t = committed"
-    and "tm_km_k'_t'_unchanged k s s' t"
-  shows "update_kv_writes_all_txn tStm (km_state (svrs s' k)) (svr_key_fp (svrs s k)) vl = vl"
-  using assms apply (auto simp add: update_kv_writes_all_txn_def km_unchanged_defs)
-  by (metis state_km.distinct(41) the_wr_tI)
+    and "svr_state (svrs s k) t = write_lock"
+    and "svr_state (svrs s' k) t = committed"
+    and "cl_svr_k'_t'_unchanged k s s' t"
+  shows "update_kv_writes_all_txn tStm (svr_state (svrs s' k)) (svr_key_fp (svrs s k)) vl = vl"
+  using assms apply (auto simp add: update_kv_writes_all_txn_def svr_unchanged_defs)
+  by (metis state_svr.distinct(41) the_wr_tI)
 
 lemma update_kv_writes_commit_n_inv:
   assumes "WLockInv s k"
-    and "km_state (svrs s k) t = no_lock"
-    and "km_state (svrs s' k) t = committed"
-    and "tm_km_k'_t'_unchanged k s s' t"
-  shows "update_kv_writes_all_txn (\<lambda>t. tm_state (cls s (get_cl_txn t))) (km_state (svrs s' k))
+    and "svr_state (svrs s k) t = no_lock"
+    and "svr_state (svrs s' k) t = committed"
+    and "cl_svr_k'_t'_unchanged k s s' t"
+  shows "update_kv_writes_all_txn (\<lambda>t. cl_state (cls s (get_cl_txn t))) (svr_state (svrs s' k))
            (svr_key_fp (svrs s k)) vl =
-         update_kv_writes_all_txn (\<lambda>t. tm_state (cls s (get_cl_txn t))) (km_state (svrs s k))
+         update_kv_writes_all_txn (\<lambda>t. cl_state (cls s (get_cl_txn t))) (svr_state (svrs s k))
            (svr_key_fp (svrs s k)) vl"
   using assms apply (auto simp add: update_kv_writes_all_txn_def)
-  subgoal for t' apply (cases "t' = t"; simp add: km_unchanged_defs)
-    by (smt (verit) state_km.distinct(41) theI the_wr_tI)
-  subgoal for t' by (cases "t' = t"; simp add: km_unchanged_defs the_wr_tI)
-  subgoal for t' by (cases "t' = t"; auto simp add: km_unchanged_defs the_wr_tI).
+  subgoal for t' apply (cases "t' = t"; simp add: svr_unchanged_defs)
+    by (smt (verit) state_svr.distinct(41) theI the_wr_tI)
+  subgoal for t' by (cases "t' = t"; simp add: svr_unchanged_defs the_wr_tI)
+  subgoal for t' by (cases "t' = t"; auto simp add: svr_unchanged_defs the_wr_tI).
 
 \<comment> \<open>kvs_of_gs\<close>
-lemma kvs_of_gs_km_inv:
+lemma kvs_of_gs_svr_inv:
   assumes "WLockInv s k" and "RLockInv s k"
-    and "(\<forall>t. km_state (svrs s k) t \<noteq> write_lock) \<or> 
-              km_state (svrs s' k) t \<noteq> write_lock"
-    and "tm_state (cls s (get_cl_txn t)) \<noteq> tm_committed"
+    and "(\<forall>t. svr_state (svrs s k) t \<noteq> write_lock) \<or> 
+              svr_state (svrs s' k) t \<noteq> write_lock"
+    and "cl_state (cls s (get_cl_txn t)) \<noteq> cl_committed"
     and "\<And>k. svr_vl (svrs s' k) = svr_vl (svrs s k)"
-    and "tm_km_k'_t'_unchanged k s s' t"
+    and "cl_svr_k'_t'_unchanged k s s' t"
   shows "kvs_of_gs s' = kvs_of_gs s"
   using assms apply (auto simp add: kvs_of_gs_def del: disjE) apply (rule ext)
-  subgoal for k' using eligible_reads_km_inv[of s k t s'] update_kv_writes_km_inv
-  by (cases "k' = k"; simp add: update_kv_all_txn_def update_kv_reads_all_txn_def km_unchanged_defs).
+  subgoal for k' using eligible_reads_svr_inv[of s k t s'] update_kv_writes_svr_inv
+  by (cases "k' = k"; simp add: update_kv_all_txn_def update_kv_reads_all_txn_def svr_unchanged_defs).
 
 (*TM events*)
 \<comment> \<open>eligible reads\<close>
-lemma eligible_reads_tm_inv:
+lemma eligible_reads_cl_inv:
   assumes "TIDFutureKm s cl" and "TIDPastKm s cl"
-    and "tm_state (cls s cl) \<noteq> tm_committed \<or>
-         (\<forall>k. km_state (svrs s k) (get_txn_cl cl s) = committed)"
-    and "tm_state (cls s' cl) \<noteq> tm_committed"
-    and "km_tm_cl'_unchanged cl s s'"
+    and "cl_state (cls s cl) \<noteq> cl_committed \<or>
+         (\<forall>k. svr_state (svrs s k) (get_txn_cl cl s) = committed)"
+    and "cl_state (cls s' cl) \<noteq> cl_committed"
+    and "svr_cl_cl'_unchanged cl s s'"
   shows "
-  eligible_reads (\<lambda>t. tm_state (cls s' (get_cl_txn t))) (km_state (svrs s k)) (svr_key_fp (svrs s k)) t =
-  eligible_reads (\<lambda>t. tm_state (cls s (get_cl_txn t))) (km_state (svrs s k)) (svr_key_fp (svrs s k)) t"
-  using assms apply (auto simp add: update_kv_writes_all_txn_def tm_unchanged_defs)
+  eligible_reads (\<lambda>t. cl_state (cls s' (get_cl_txn t))) (svr_state (svrs s k)) (svr_key_fp (svrs s k)) t =
+  eligible_reads (\<lambda>t. cl_state (cls s (get_cl_txn t))) (svr_state (svrs s k)) (svr_key_fp (svrs s k)) t"
+  using assms apply (auto simp add: update_kv_writes_all_txn_def cl_unchanged_defs)
   subgoal
     apply (cases "get_cl_txn t = cl"; cases "get_sn_txn t = cl_sn (cls s cl)";
-            simp add: tm_unchanged_defs)
-    apply (metis txid0.collapse state_km.distinct(33))
-    by (metis empty_iff insert_iff other_sn_idle state_km.distinct(3)
-        state_km.distinct(33) state_km.distinct(35))
+            simp add: cl_unchanged_defs)
+    apply (metis txid0.collapse state_svr.distinct(33))
+    by (metis empty_iff insert_iff other_sn_idle state_svr.distinct(3)
+        state_svr.distinct(33) state_svr.distinct(35))
   subgoal
     apply (cases "get_cl_txn t = cl"; cases "get_sn_txn t = cl_sn (cls s cl)";
-            simp add: tm_unchanged_defs)
-    apply (metis txid0.collapse state_km.distinct(41))
-    by (metis empty_iff insert_iff other_sn_idle state_km.distinct(41)
-        state_km.distinct(43) state_km.distinct(5))
+            simp add: cl_unchanged_defs)
+    apply (metis txid0.collapse state_svr.distinct(41))
+    by (metis empty_iff insert_iff other_sn_idle state_svr.distinct(41)
+        state_svr.distinct(43) state_svr.distinct(5))
   done
 
-lemma eligible_reads_tm_commit_no_lock_inv:
+lemma eligible_reads_cl_commit_no_lock_inv:
   assumes "TIDPastKm s cl" and "TIDFutureKm s cl"
-    and "tm_state (cls s cl) = tm_prepared"
-    and "tm_state (cls s' cl) = tm_committed"
+    and "cl_state (cls s cl) = cl_prepared"
+    and "cl_state (cls s' cl) = cl_committed"
     and "other_insts_unchanged cl (cls s) (cls s')"
-    and "km_state (svrs s k) (get_txn_cl cl s) = no_lock"
+    and "svr_state (svrs s k) (get_txn_cl cl s) = no_lock"
   shows "
-  eligible_reads (\<lambda>t. tm_state (cls s' (get_cl_txn t))) (km_state (svrs s k)) (svr_key_fp (svrs s k)) t =
-  eligible_reads (\<lambda>t. tm_state (cls s (get_cl_txn t))) (km_state (svrs s k)) (svr_key_fp (svrs s k)) t"
+  eligible_reads (\<lambda>t. cl_state (cls s' (get_cl_txn t))) (svr_state (svrs s k)) (svr_key_fp (svrs s k)) t =
+  eligible_reads (\<lambda>t. cl_state (cls s (get_cl_txn t))) (svr_state (svrs s k)) (svr_key_fp (svrs s k)) t"
   using assms apply (cases "get_cl_txn t = cl"; simp add: other_insts_unchanged_def)
   by (metis empty_iff txid0.collapse insert_iff other_sn_idle
-      state_km.distinct(29) state_km.distinct(3) state_km.distinct(33) state_km.distinct(35)
-      state_km.distinct(37) state_km.distinct(41) state_km.distinct(43) state_km.distinct(5))
+      state_svr.distinct(29) state_svr.distinct(3) state_svr.distinct(33) state_svr.distinct(35)
+      state_svr.distinct(37) state_svr.distinct(41) state_svr.distinct(43) state_svr.distinct(5))
 
 \<comment> \<open>write updates\<close>
-lemma update_kv_writes_tm_inv:
+lemma update_kv_writes_cl_inv:
   assumes "TIDFutureKm s cl" and "TIDPastKm s cl"
-    and "tm_state (cls s cl) \<noteq> tm_committed \<or>
-         (\<forall>k. km_state (svrs s k) (get_txn_cl cl s) = committed)"
-    and "tm_state (cls s' cl) \<noteq> tm_committed"
-    and "km_tm_cl'_unchanged cl s s'"
-  shows "update_kv_writes_all_txn (\<lambda>t. tm_state (cls s' (get_cl_txn t)))
-                (km_state (svrs s k)) (svr_key_fp (svrs s k)) vl =
-               update_kv_writes_all_txn (\<lambda>t. tm_state (cls s (get_cl_txn t)))
-                (km_state (svrs s k)) (svr_key_fp (svrs s k)) vl"
-  using assms apply (auto simp add: update_kv_writes_all_txn_def tm_unchanged_defs)
+    and "cl_state (cls s cl) \<noteq> cl_committed \<or>
+         (\<forall>k. svr_state (svrs s k) (get_txn_cl cl s) = committed)"
+    and "cl_state (cls s' cl) \<noteq> cl_committed"
+    and "svr_cl_cl'_unchanged cl s s'"
+  shows "update_kv_writes_all_txn (\<lambda>t. cl_state (cls s' (get_cl_txn t)))
+                (svr_state (svrs s k)) (svr_key_fp (svrs s k)) vl =
+               update_kv_writes_all_txn (\<lambda>t. cl_state (cls s (get_cl_txn t)))
+                (svr_state (svrs s k)) (svr_key_fp (svrs s k)) vl"
+  using assms apply (auto simp add: update_kv_writes_all_txn_def cl_unchanged_defs)
   subgoal for t
     apply (cases "get_cl_txn t = cl"; cases "get_sn_txn t = cl_sn (cls s cl)"; simp)
-    apply (metis txid0.collapse state_km.distinct(41))
-    by (metis ex_in_conv insertE other_sn_idle state_km.distinct(41)
-        state_km.distinct(43) state_km.distinct(5)).
+    apply (metis txid0.collapse state_svr.distinct(41))
+    by (metis ex_in_conv insertE other_sn_idle state_svr.distinct(41)
+        state_svr.distinct(43) state_svr.distinct(5)).
 
 \<comment> \<open>kvs_of_gs\<close>
-lemma kvs_of_gs_tm_inv:
+lemma kvs_of_gs_cl_inv:
   assumes "TIDFutureKm s cl" and "TIDPastKm s cl"
-    and "tm_state (cls s cl) \<noteq> tm_committed \<or>
-         (\<forall>k. km_state (svrs s k) (get_txn_cl cl s) = committed)"
-    and "tm_state (cls s' cl) \<noteq> tm_committed"
-    and "km_tm_cl'_unchanged cl s s'"
+    and "cl_state (cls s cl) \<noteq> cl_committed \<or>
+         (\<forall>k. svr_state (svrs s k) (get_txn_cl cl s) = committed)"
+    and "cl_state (cls s' cl) \<noteq> cl_committed"
+    and "svr_cl_cl'_unchanged cl s s'"
   shows "kvs_of_gs s' = kvs_of_gs s"
   using assms
   apply (simp add: kvs_of_gs_def) apply (rule ext)
-  using update_kv_writes_tm_inv[of s] eligible_reads_tm_inv[of s cl s']
-  by (auto simp add: update_kv_all_txn_def update_kv_reads_all_txn_def tm_unchanged_defs)
+  using update_kv_writes_cl_inv[of s] eligible_reads_cl_inv[of s cl s']
+  by (auto simp add: update_kv_all_txn_def update_kv_reads_all_txn_def cl_unchanged_defs)
 
-lemma update_kv_all_tm_commit_no_lock_inv:
+lemma update_kv_all_cl_commit_no_lock_inv:
   assumes "TIDPastKm s cl" and "TIDFutureKm s cl"
-    and "tm_state (cls s cl) = tm_prepared"
-    and "tm_state (cls s' cl) = tm_committed"
+    and "cl_state (cls s cl) = cl_prepared"
+    and "cl_state (cls s' cl) = cl_committed"
     and "other_insts_unchanged cl (cls s) (cls s')"
-    and "km_state (svrs s k) (get_txn_cl cl s) = no_lock"
-  shows "update_kv_all_txn (\<lambda>t. tm_state (cls s' (get_cl_txn t))) (km_state (svrs s k))
+    and "svr_state (svrs s k) (get_txn_cl cl s) = no_lock"
+  shows "update_kv_all_txn (\<lambda>t. cl_state (cls s' (get_cl_txn t))) (svr_state (svrs s k))
           (svr_key_fp (svrs s k)) (svr_vl (svrs s k)) =
-         update_kv_all_txn (\<lambda>t. tm_state (cls s (get_cl_txn t))) (km_state (svrs s k))
+         update_kv_all_txn (\<lambda>t. cl_state (cls s (get_cl_txn t))) (svr_state (svrs s k))
           (svr_key_fp (svrs s k)) (svr_vl (svrs s k))"
-  using assms eligible_reads_tm_commit_no_lock_inv[of s cl s' k]
+  using assms eligible_reads_cl_commit_no_lock_inv[of s cl s' k]
   apply (auto simp add: NoLockFpInv_def update_kv_all_defs other_insts_unchanged_def)
   apply (metis (mono_tags, lifting) txid0.collapse insert_compr mem_Collect_eq other_sn_idle singleton_conv2
-    state_km.distinct(37) state_km.distinct(41) state_km.distinct(43) state_km.distinct(5))
+    state_svr.distinct(37) state_svr.distinct(41) state_svr.distinct(43) state_svr.distinct(5))
   by metis
 
 (*All events*)
-abbreviation not_tm_commit where
-  "not_tm_commit e \<equiv> \<forall>cl sn u F. e \<noteq> TM_Commit cl sn u F"
+abbreviation not_cl_commit where
+  "not_cl_commit e \<equiv> \<forall>cl sn u F. e \<noteq> Cl_Commit cl sn u F"
 
 abbreviation invariant_list_kvs where
   "invariant_list_kvs s \<equiv> \<forall>cl k. TIDFutureKm s cl \<and> TIDPastKm s cl \<and> RLockInv s k \<and> WLockInv s k \<and>
@@ -882,29 +882,29 @@ abbreviation invariant_list_kvs where
 lemma kvs_of_gs_inv:
   assumes "gs_trans s e s'"
     and "invariant_list_kvs s"
-    and "not_tm_commit e"
+    and "not_cl_commit e"
   shows "kvs_of_gs s' = kvs_of_gs s"
   using assms
   proof (induction e)
     case (Prepare x1 x2)
-    then show ?case using kvs_of_gs_km_inv[of s x1 s' x2]
-      by (auto simp add: tps_trans_defs km_unchanged_defs dest!: svr_vl_eq_all_k)
+    then show ?case using kvs_of_gs_svr_inv[of s x1 s' x2]
+      by (auto simp add: tps_trans_defs svr_unchanged_defs dest!: svr_vl_eq_all_k)
   next
     case (RLock x1 x2 x3)
-    then show ?case using kvs_of_gs_km_inv[of s x1 s' x3]
-      by (auto simp add: tps_trans_defs km_unchanged_defs dest!: svr_vl_eq_all_k)
+    then show ?case using kvs_of_gs_svr_inv[of s x1 s' x3]
+      by (auto simp add: tps_trans_defs svr_unchanged_defs dest!: svr_vl_eq_all_k)
   next
     case (WLock x1 x2 x3 x4)
-    then show ?case using kvs_of_gs_km_inv[of s x1 s' x4]
-      by (auto simp add: tps_trans_defs km_unchanged_defs dest!: svr_vl_eq_all_k)
+    then show ?case using kvs_of_gs_svr_inv[of s x1 s' x4]
+      by (auto simp add: tps_trans_defs svr_unchanged_defs dest!: svr_vl_eq_all_k)
   next
     case (NoLock x1 x2)
-    then show ?case using kvs_of_gs_km_inv[of s x1 s' x2]
-      by (auto simp add: tps_trans_defs km_unchanged_defs dest!: svr_vl_eq_all_k)
+    then show ?case using kvs_of_gs_svr_inv[of s x1 s' x2]
+      by (auto simp add: tps_trans_defs svr_unchanged_defs dest!: svr_vl_eq_all_k)
   next
     case (NOK x1 x2)
-    then show ?case using kvs_of_gs_km_inv[of s x1 s' x2]
-      by (auto simp add: tps_trans_defs km_unchanged_defs dest!: svr_vl_eq_all_k)
+    then show ?case using kvs_of_gs_svr_inv[of s x1 s' x2]
+      by (auto simp add: tps_trans_defs svr_unchanged_defs dest!: svr_vl_eq_all_k)
   next
     case (Commit x1 x2)
     hence u: "kvs_of_gs s' x1 = kvs_of_gs s x1"
@@ -913,7 +913,7 @@ lemma kvs_of_gs_inv:
         using eligible_reads_read_lock_inv[of s x1 x2 s']
               update_kv_writes_commit_r_inv[of s x1 x2 s']
         by (auto simp add: update_kv_all_txn_def update_kv_reads_all_txn_def Let_def
-            RLockFpInv_def KVSNonEmp_def km_unchanged_defs update_kv_key_ro_set_v_readerset
+            RLockFpInv_def KVSNonEmp_def svr_unchanged_defs update_kv_key_ro_set_v_readerset
             dest!: eq_for_all_k)
       subgoal
         using update_kv_reads_commit_w_s_inv[of s x1 x2 s']
@@ -921,45 +921,45 @@ lemma kvs_of_gs_inv:
               update_kv_writes_commit_w_s_inv[of s x1 x2 s']
               update_kv_writes_commit_w_s'_inv[of s x1 x2 s']
         by (auto simp add: update_kv_all_txn_def update_kv_key_def update_kv_reads_defs
-            km_unchanged_defs dest!: eq_for_all_k split: option.split)
+            svr_unchanged_defs dest!: eq_for_all_k split: option.split)
       subgoal
         using eligible_reads_no_lock_inv[of s x1 x2 s']
         using update_kv_writes_commit_n_inv[of s x1 x2 s']
         by (auto simp add: update_kv_all_txn_def update_kv_reads_all_txn_def
-            NoLockFpInv_def km_unchanged_defs dest!: eq_for_all_k) done
+            NoLockFpInv_def svr_unchanged_defs dest!: eq_for_all_k) done
     hence "\<forall>k. k \<noteq> x1 \<longrightarrow> kvs_of_gs s' k = kvs_of_gs s k" using Commit
-      by (auto simp add: commit_def km_unchanged_defs kvs_of_gs_def)
+      by (auto simp add: commit_def svr_unchanged_defs kvs_of_gs_def)
     then show ?case using u by auto
   next
     case (Abort x1 x2)
-    then show ?case using kvs_of_gs_km_inv[of s x1 s' x2]
-      by (auto simp add: tps_trans_defs km_unchanged_defs dest!: svr_vl_eq_all_k)
+    then show ?case using kvs_of_gs_svr_inv[of s x1 s' x2]
+      by (auto simp add: tps_trans_defs svr_unchanged_defs dest!: svr_vl_eq_all_k)
   next
     case (User_Commit x)
-    then show ?case using kvs_of_gs_tm_inv[of s x s']
-     by (auto simp add: tps_trans_defs tm_unchanged_defs)
+    then show ?case using kvs_of_gs_cl_inv[of s x s']
+     by (auto simp add: tps_trans_defs cl_unchanged_defs)
   next
-    case (TM_Abort x)
-    then show ?case using kvs_of_gs_tm_inv[of s x s']
-     by (auto simp add: tps_trans_defs tm_unchanged_defs)
+    case (Cl_Abort x)
+    then show ?case using kvs_of_gs_cl_inv[of s x s']
+     by (auto simp add: tps_trans_defs cl_unchanged_defs)
   next
-    case (TM_ReadyC x)
-    then show ?case using kvs_of_gs_tm_inv[of s x s']
-     by (auto simp add: tps_trans_defs tm_unchanged_defs)
+    case (Cl_ReadyC x)
+    then show ?case using kvs_of_gs_cl_inv[of s x s']
+     by (auto simp add: tps_trans_defs cl_unchanged_defs)
   next
-    case (TM_ReadyA x)
-    then show ?case using kvs_of_gs_tm_inv[of s x s']
-     by (auto simp add: tps_trans_defs tm_unchanged_defs)
+    case (Cl_ReadyA x)
+    then show ?case using kvs_of_gs_cl_inv[of s x s']
+     by (auto simp add: tps_trans_defs cl_unchanged_defs)
  qed auto
 
 \<comment> \<open>More specific lemmas about TM commit\<close>
 lemma kvs_of_gs_commit_length_increasing:
-  assumes "tm_state (cls s cl) = tm_prepared"
-    and "tm_state (cls s' cl) = tm_committed"
-    and "km_tm_cl'_unchanged cl s s'"
+  assumes "cl_state (cls s cl) = cl_prepared"
+    and "cl_state (cls s' cl) = cl_committed"
+    and "svr_cl_cl'_unchanged cl s s'"
   shows "length (kvs_of_gs s k) \<le> length (kvs_of_gs s' k)"
   using assms
-  apply (auto simp add: kvs_of_gs_def tm_unchanged_defs update_kv_all_txn_def
+  apply (auto simp add: kvs_of_gs_def cl_unchanged_defs update_kv_all_txn_def
       update_kv_writes_all_txn_def update_kv_writes_on_diff_len)
   by (metis (no_types, lifting) update_kv_reads_all_txn_length update_kv_writes_length_increasing)
 
@@ -968,101 +968,101 @@ lemma kvs_of_gs_length_increasing:
     and "invariant_list_kvs s"
   shows "\<And>k. length (kvs_of_gs s k) \<le> length (kvs_of_gs s' k)"
   using assms
-  apply (cases "not_tm_commit e"; simp add: kvs_of_gs_inv)
-  apply auto apply (simp add: tm_commit_def) by (auto dest!: kvs_of_gs_commit_length_increasing)
+  apply (cases "not_cl_commit e"; simp add: kvs_of_gs_inv)
+  apply auto apply (simp add: cl_commit_def) by (auto dest!: kvs_of_gs_commit_length_increasing)
 
-lemma tm_commit_expands_eligible_reads:
-  assumes "tm_state (cls s' cl) = tm_committed"
+lemma cl_commit_expands_eligible_reads:
+  assumes "cl_state (cls s' cl) = cl_committed"
     and "other_insts_unchanged cl (cls s) (cls s')"
   shows
-  "{t. eligible_reads (\<lambda>t. tm_state (cls s (get_cl_txn t))) (km_state (svrs s k)) (svr_key_fp (svrs s k)) t} \<subseteq>
-   {t. eligible_reads (\<lambda>t. tm_state (cls s' (get_cl_txn t))) (km_state (svrs s k)) (svr_key_fp (svrs s k)) t}"
+  "{t. eligible_reads (\<lambda>t. cl_state (cls s (get_cl_txn t))) (svr_state (svrs s k)) (svr_key_fp (svrs s k)) t} \<subseteq>
+   {t. eligible_reads (\<lambda>t. cl_state (cls s' (get_cl_txn t))) (svr_state (svrs s k)) (svr_key_fp (svrs s k)) t}"
   using assms by (auto simp add: other_insts_unchanged_def)
 
-lemma tm_commit_expands_eligible_reads':
+lemma cl_commit_expands_eligible_reads':
   assumes "NoLockFpInv s k" and "TIDPastKm s cl" and "TIDFutureKm s cl"
-    and "tm_state (cls s cl) = tm_prepared"
-    and "tm_state (cls s' cl) = tm_committed"
-    and "km_state (svrs s k) (get_txn_cl cl s) \<in> {read_lock, write_lock, no_lock}"
+    and "cl_state (cls s cl) = cl_prepared"
+    and "cl_state (cls s' cl) = cl_committed"
+    and "is_locked (svr_state (svrs s k) (get_txn_cl cl s))"
     and "other_insts_unchanged cl (cls s) (cls s')"
-  shows "{x. eligible_reads (\<lambda>t. tm_state (cls s' (get_cl_txn t))) (km_state (svrs s k))
+  shows "{x. eligible_reads (\<lambda>t. cl_state (cls s' (get_cl_txn t))) (svr_state (svrs s k))
     (svr_key_fp (svrs s k)) x} = (case svr_key_fp (svrs s k) (get_txn_cl cl s) R of
-   None \<Rightarrow> {x. eligible_reads (\<lambda>t. tm_state (cls s (get_cl_txn t))) (km_state (svrs s k))
+   None \<Rightarrow> {x. eligible_reads (\<lambda>t. cl_state (cls s (get_cl_txn t))) (svr_state (svrs s k))
      (svr_key_fp (svrs s k)) x}|
-   Some _ \<Rightarrow> insert (get_txn_cl cl s) {x. eligible_reads (\<lambda>t. tm_state (cls s (get_cl_txn t)))
-     (km_state (svrs s k)) (svr_key_fp (svrs s k)) x})"
+   Some _ \<Rightarrow> insert (get_txn_cl cl s) {x. eligible_reads (\<lambda>t. cl_state (cls s (get_cl_txn t)))
+     (svr_state (svrs s k)) (svr_key_fp (svrs s k)) x})"
   using assms
   apply (auto simp add: other_insts_unchanged_def NoLockFpInv_def split: option.split del: disjE)
   subgoal for t apply (cases "get_cl_txn t = cl"; cases "get_sn_txn t = cl_sn (cls s cl)"; simp)
     apply (metis txid0.collapse option.distinct(1))
-    by (metis emptyE insert_iff other_sn_idle state_km.distinct(3) state_km.distinct(33)
-        state_km.distinct(35) state_km.distinct(41) state_km.distinct(43) state_km.distinct(5))
+    by (metis emptyE insert_iff other_sn_idle state_svr.distinct(3) state_svr.distinct(33)
+        state_svr.distinct(35) state_svr.distinct(41) state_svr.distinct(43) state_svr.distinct(5))
   subgoal for v t apply (cases "get_cl_txn t = cl"; cases "get_sn_txn t = cl_sn (cls s cl)"; simp)
     apply (metis txid0.collapse)
-    by (metis empty_iff insertE other_sn_idle state_km.distinct(3) state_km.distinct(33)
-        state_km.distinct(35) state_km.distinct(41) state_km.distinct(43) state_km.distinct(5))
+    by (metis empty_iff insertE other_sn_idle state_svr.distinct(3) state_svr.distinct(33)
+        state_svr.distinct(35) state_svr.distinct(41) state_svr.distinct(43) state_svr.distinct(5))
   by auto
   
-lemma tm_commit_updates_kv_reads:
+lemma cl_commit_updates_kv_reads:
   assumes "KVSNonEmp s"
-    and "tm_state (cls s' cl) = tm_committed"
+    and "cl_state (cls s' cl) = cl_committed"
     and "other_insts_unchanged cl (cls s) (cls s')"
   shows
-  "update_kv_reads_all_txn (\<lambda>t. tm_state (cls s' (get_cl_txn t))) (km_state (svrs s k))
+  "update_kv_reads_all_txn (\<lambda>t. cl_state (cls s' (get_cl_txn t))) (svr_state (svrs s k))
       (svr_key_fp (svrs s k)) (svr_vl (svrs s k)) = 
-   update_kv_reads_all_txn (\<lambda>t. tm_state (cls s' (get_cl_txn t))) (km_state (svrs s k))
+   update_kv_reads_all_txn (\<lambda>t. cl_state (cls s' (get_cl_txn t))) (svr_state (svrs s k))
       (svr_key_fp (svrs s k))
-        (update_kv_reads_all_txn (\<lambda>t. tm_state (cls s (get_cl_txn t))) (km_state (svrs s k))
+        (update_kv_reads_all_txn (\<lambda>t. cl_state (cls s (get_cl_txn t))) (svr_state (svrs s k))
           (svr_key_fp (svrs s k)) (svr_vl (svrs s k)))"
-  using assms tm_commit_expands_eligible_reads[of s' cl s k]
+  using assms cl_commit_expands_eligible_reads[of s' cl s k]
   by (auto simp add: update_kv_reads_all_defs Un_assoc subset_Un_eq)
 
-lemma tm_commit_updates_kv_reads':
+lemma cl_commit_updates_kv_reads':
   assumes "TIDPastKm s cl" and "TIDFutureKm s cl"
     and "KVSNonEmp s" and "NoLockFpInv s k"
-    and "tm_state (cls s cl) = tm_prepared"
-    and "tm_state (cls s' cl) = tm_committed"
-    and "km_state (svrs s k) (get_txn_cl cl s) \<in> {read_lock, write_lock, no_lock}"
+    and "cl_state (cls s cl) = cl_prepared"
+    and "cl_state (cls s' cl) = cl_committed"
+    and "is_locked (svr_state (svrs s k) (get_txn_cl cl s))"
     and "other_insts_unchanged cl (cls s) (cls s')"
   shows
-  "update_kv_reads_all_txn (\<lambda>t. tm_state (cls s' (get_cl_txn t))) (km_state (svrs s k))
+  "update_kv_reads_all_txn (\<lambda>t. cl_state (cls s' (get_cl_txn t))) (svr_state (svrs s k))
       (svr_key_fp (svrs s k)) (svr_vl (svrs s k)) = 
    update_kv_reads (get_txn_cl cl s) (svr_key_fp (svrs s k) (get_txn_cl cl s))
-     (full_view (update_kv_reads_all_txn (\<lambda>t. tm_state (cls s (get_cl_txn t))) (km_state (svrs s k))
+     (full_view (update_kv_reads_all_txn (\<lambda>t. cl_state (cls s (get_cl_txn t))) (svr_state (svrs s k))
           (svr_key_fp (svrs s k)) (svr_vl (svrs s k))))
-        (update_kv_reads_all_txn (\<lambda>t. tm_state (cls s (get_cl_txn t))) (km_state (svrs s k))
+        (update_kv_reads_all_txn (\<lambda>t. cl_state (cls s (get_cl_txn t))) (svr_state (svrs s k))
           (svr_key_fp (svrs s k)) (svr_vl (svrs s k)))"
-  using assms tm_commit_expands_eligible_reads'[of s k cl s']
+  using assms cl_commit_expands_eligible_reads'[of s k cl s']
   by (auto simp add: update_kv_reads_all_txn_def update_kv_reads_defs
       del:disjE split: option.split)
 
-lemma tm_commit_writer_update_kv_all:
+lemma cl_commit_writer_update_kv_all:
   assumes "TIDPastKm s cl" and "TIDFutureKm s cl"
     and "WLockInv s k" and "RLockInv s k"
     and "NoLockFpInv s k" and "KVSNonEmp s"
-    and "tm_state (cls s cl) = tm_prepared"
-    and "tm_state (cls s' cl) = tm_committed"
-    and "km_state (svrs s k) (get_txn_cl cl s) \<in> {read_lock, write_lock}"
+    and "cl_state (cls s cl) = cl_prepared"
+    and "cl_state (cls s' cl) = cl_committed"
+    and "svr_state (svrs s k) (get_txn_cl cl s) \<in> {read_lock, write_lock}"
     and "other_insts_unchanged cl (cls s) (cls s')"
   shows
-  "update_kv_all_txn (\<lambda>t. tm_state (cls s' (get_cl_txn t))) (km_state (svrs s k))
+  "update_kv_all_txn (\<lambda>t. cl_state (cls s' (get_cl_txn t))) (svr_state (svrs s k))
       (svr_key_fp (svrs s k)) (svr_vl (svrs s k)) = 
-   update_kv_all_txn (\<lambda>t. tm_state (cls s' (get_cl_txn t))) (km_state (svrs s k))
+   update_kv_all_txn (\<lambda>t. cl_state (cls s' (get_cl_txn t))) (svr_state (svrs s k))
       (svr_key_fp (svrs s k))
-        (update_kv_all_txn (\<lambda>t. tm_state (cls s (get_cl_txn t))) (km_state (svrs s k))
+        (update_kv_all_txn (\<lambda>t. cl_state (cls s (get_cl_txn t))) (svr_state (svrs s k))
           (svr_key_fp (svrs s k)) (svr_vl (svrs s k)))"
   using assms apply auto
   subgoal apply (simp add: read_only_update')
-    using tm_commit_updates_kv_reads by blast
+    using cl_commit_updates_kv_reads by blast
   subgoal apply (simp add: writer_update_before)
-    by (auto simp add: update_kv_all_txn_def tm_commit_updates_kv_reads[of s s' cl k])
+    by (auto simp add: update_kv_all_txn_def cl_commit_updates_kv_reads[of s s' cl k])
   done
 
 \<comment> \<open>Fingerprint content invariant and Lemmas for proving the fp_property\<close>
 
 lemma svr_vl_read_lock_commit_eq_length:
   assumes "RLockFpInv s k"
-    and "km_state (svrs s k) t = read_lock"
+    and "svr_state (svrs s k) t = read_lock"
     and "svr_vl (svrs s' k) =
           update_kv_key t (svr_key_fp (svrs s k) t) (full_view (svr_vl (svrs s k))) (svr_vl (svrs s k))"
   shows "length (svr_vl (svrs s' k)) = length (svr_vl (svrs s k))"
@@ -1072,8 +1072,8 @@ lemma svr_vl_read_lock_commit_eq_length:
 
 lemma svr_vl_read_commit_eq_lv:
   assumes "RLockFpInv s k"
-    and "km_state (svrs s k) t = read_lock"
-    and "km_state (svrs s' k) t = committed"
+    and "svr_state (svrs s k) t = read_lock"
+    and "svr_state (svrs s' k) t = committed"
     and "svr_vl (svrs s' k) =
           update_kv_key t (svr_key_fp (svrs s k) t) (full_view (svr_vl (svrs s k))) (svr_vl (svrs s k))"
   shows "v_value (last_version (svr_vl (svrs s' k)) (full_view (svr_vl (svrs s' k)))) =
@@ -1083,7 +1083,7 @@ lemma svr_vl_read_commit_eq_lv:
   by (metis full_view_def max_in_full_view update_kv_key_v_value_inv)
 
 definition RLockFpContentInv where
-  "RLockFpContentInv s k \<longleftrightarrow> (\<forall>t. km_state (svrs s k) t = read_lock \<longrightarrow>
+  "RLockFpContentInv s k \<longleftrightarrow> (\<forall>t. svr_state (svrs s k) t = read_lock \<longrightarrow>
     svr_key_fp (svrs s k) t R =
       Some (v_value (last_version (svr_vl (svrs s k)) (full_view (svr_vl (svrs s k))))))"
 
@@ -1100,44 +1100,44 @@ next
   proof (cases e)
     case (Prepare x31 x32)
     then show ?thesis using reach_trans
-      apply (auto simp add: tps_trans_defs km_unchanged_defs RLockFpContentInv_def)
-      by (metis state_km.distinct(15))+
+      apply (auto simp add: tps_trans_defs svr_unchanged_defs RLockFpContentInv_def)
+      by (metis state_svr.distinct(15))+
   next
     case (RLock x41 x42 x43)
     then show ?thesis using reach_trans
-      apply (auto simp add: tps_trans_defs km_unchanged_defs RLockFpContentInv_def)
+      apply (auto simp add: tps_trans_defs svr_unchanged_defs RLockFpContentInv_def)
       by metis+
   next
     case (WLock x51 x52 x53 x54)
     then show ?thesis using reach_trans
-      apply (auto simp add: tps_trans_defs km_unchanged_defs RLockFpContentInv_def)
-      by (metis state_km.distinct(27))+
+      apply (auto simp add: tps_trans_defs svr_unchanged_defs RLockFpContentInv_def)
+      by (metis state_svr.distinct(27))+
   next
     case (NoLock x61 x62)
     then show ?thesis using reach_trans
-      apply (auto simp add: tps_trans_defs km_unchanged_defs RLockFpContentInv_def)
-      by (metis state_km.distinct(29))+
+      apply (auto simp add: tps_trans_defs svr_unchanged_defs RLockFpContentInv_def)
+      by (metis state_svr.distinct(29))+
   next
     case (NOK x71 x72)
     then show ?thesis using reach_trans
-      apply (auto simp add: tps_trans_defs km_unchanged_defs RLockFpContentInv_def)
-      by (metis state_km.distinct(31))+
+      apply (auto simp add: tps_trans_defs svr_unchanged_defs RLockFpContentInv_def)
+      by (metis state_svr.distinct(31))+
   next
     case (Commit x81 x82)
     then show ?thesis using reach_trans svr_vl_read_commit_eq_lv[of s x81 x82 s']
-      apply (auto simp add: tps_trans_defs km_unchanged_defs RLockFpContentInv_def del: disjE)
-      by (metis NoLockFpInv_def RLockInv_def reach_nolockfp reach_rlock state_km.distinct(33)
+      apply (auto simp add: tps_trans_defs svr_unchanged_defs RLockFpContentInv_def del: disjE)
+      by (metis NoLockFpInv_def RLockInv_def reach_nolockfp reach_rlock state_svr.distinct(33)
           update_kv_key_empty_fp)
   next
     case (Abort x91 x92)
     then show ?thesis using reach_trans
-      apply (auto simp add: tps_trans_defs km_unchanged_defs RLockFpContentInv_def)
-      by (metis state_km.distinct(35))+
-  qed (auto simp add: tps_trans_defs tm_unchanged_defs RLockFpContentInv_def)
+      apply (auto simp add: tps_trans_defs svr_unchanged_defs RLockFpContentInv_def)
+      by (metis state_svr.distinct(35))+
+  qed (auto simp add: tps_trans_defs cl_unchanged_defs RLockFpContentInv_def)
 qed
 
 definition WLockFpContentInv where
-  "WLockFpContentInv s k \<longleftrightarrow> (\<forall>t. km_state (svrs s k) t = write_lock \<longrightarrow>
+  "WLockFpContentInv s k \<longleftrightarrow> (\<forall>t. svr_state (svrs s k) t = write_lock \<longrightarrow>
     svr_key_fp (svrs s k) t R = None \<or>
     svr_key_fp (svrs s k) t R =
       Some (v_value (last_version (svr_vl (svrs s k)) (full_view (svr_vl (svrs s k))))))"
@@ -1155,41 +1155,41 @@ next
   proof (cases e)
     case (Prepare x31 x32)
     then show ?thesis using reach_trans
-      apply (auto simp add: tps_trans_defs km_unchanged_defs WLockFpContentInv_def)
-      by (metis state_km.distinct(17))
+      apply (auto simp add: tps_trans_defs svr_unchanged_defs WLockFpContentInv_def)
+      by (metis state_svr.distinct(17))
   next
     case (RLock x41 x42 x43)
     then show ?thesis using reach_trans
-      apply (auto simp add: tps_trans_defs km_unchanged_defs WLockFpContentInv_def)
-      by (metis state_km.distinct(27))
+      apply (auto simp add: tps_trans_defs svr_unchanged_defs WLockFpContentInv_def)
+      by (metis state_svr.distinct(27))
   next
     case (WLock x51 x52 x53 x54)
     then show ?thesis using reach_trans
-      apply (auto simp add: tps_trans_defs km_unchanged_defs WLockFpContentInv_def)
+      apply (auto simp add: tps_trans_defs svr_unchanged_defs WLockFpContentInv_def)
       by metis+
   next
     case (NoLock x61 x62)
     then show ?thesis using reach_trans
-      apply (auto simp add: tps_trans_defs km_unchanged_defs WLockFpContentInv_def)
-      by (metis state_km.distinct(37))
+      apply (auto simp add: tps_trans_defs svr_unchanged_defs WLockFpContentInv_def)
+      by (metis state_svr.distinct(37))
   next
     case (NOK x71 x72)
     then show ?thesis using reach_trans
-      apply (auto simp add: tps_trans_defs km_unchanged_defs WLockFpContentInv_def)
-      by (metis state_km.distinct(39))+
+      apply (auto simp add: tps_trans_defs svr_unchanged_defs WLockFpContentInv_def)
+      by (metis state_svr.distinct(39))+
   next
     case (Commit x81 x82)
     then show ?thesis using reach_trans
-      apply (auto simp add: tps_trans_defs km_unchanged_defs WLockFpContentInv_def)
-      apply (metis RLockInv_def reach_rlock state_km.distinct(41))
-      apply (smt reach_wlock state_km.distinct(41) the_wr_tI)
+      apply (auto simp add: tps_trans_defs svr_unchanged_defs WLockFpContentInv_def)
+      apply (metis RLockInv_def reach_rlock state_svr.distinct(41))
+      apply (smt reach_wlock state_svr.distinct(41) the_wr_tI)
       by (metis NoLockFpInv_def reach_nolockfp update_kv_key_empty_fp)
   next
     case (Abort x91 x92)
     then show ?thesis using reach_trans
-      apply (auto simp add: tps_trans_defs km_unchanged_defs WLockFpContentInv_def)
-      by (metis state_km.distinct(43))+
-  qed (auto simp add: tps_trans_defs tm_unchanged_defs WLockFpContentInv_def)
+      apply (auto simp add: tps_trans_defs svr_unchanged_defs WLockFpContentInv_def)
+      by (metis state_svr.distinct(43))+
+  qed (auto simp add: tps_trans_defs cl_unchanged_defs WLockFpContentInv_def)
 qed
 
 lemma update_kv_all_txn_v_value_inv:
@@ -1201,8 +1201,8 @@ lemma update_kv_all_txn_v_value_inv:
 
 lemma svr_vl_kvs_eq_length:
   assumes "WLockInv s k" and "RLockInv s k"
-    and "tm_state (cls s cl) = tm_prepared"
-    and "km_state (svrs s k) (get_txn_cl cl s) \<in> {read_lock, write_lock}"
+    and "cl_state (cls s cl) = cl_prepared"
+    and "svr_state (svrs s k) (get_txn_cl cl s) \<in> {read_lock, write_lock}"
   shows "length (kvs_of_gs s k) = length (svr_vl (svrs s k))"
   using assms
   apply (auto simp add: WLockInv_def RLockInv_def kvs_of_gs_def)
@@ -1210,8 +1210,8 @@ lemma svr_vl_kvs_eq_length:
 
 lemma svr_vl_kvs_eq_lv:
   assumes "WLockInv s k" and "RLockInv s k" and "KVSNonEmp s"
-    and "tm_state (cls s cl) = tm_prepared"
-    and "km_state (svrs s k) (get_txn_cl cl s) \<in> {read_lock, write_lock}"
+    and "cl_state (cls s cl) = cl_prepared"
+    and "svr_state (svrs s k) (get_txn_cl cl s) \<in> {read_lock, write_lock}"
   shows "v_value (last_version (kvs_of_gs s k) (full_view (kvs_of_gs s k))) =
          v_value (last_version (svr_vl (svrs s k)) (full_view (svr_vl (svrs s k))))"
   using assms svr_vl_kvs_eq_length[of s]
@@ -1223,9 +1223,9 @@ lemma svr_vl_kvs_eq_lv:
 \<comment> \<open>Lemmas for view growth after commit\<close>
 
 lemma committed_kvs_view_grows:
-  assumes "tm_state (cls s cl) = tm_prepared"
-    and "tm_state (cls s' cl) = tm_committed"
-    and "km_tm_cl'_unchanged cl s s'"
+  assumes "cl_state (cls s cl) = cl_prepared"
+    and "cl_state (cls s' cl) = cl_committed"
+    and "svr_cl_cl'_unchanged cl s s'"
   shows "(\<lambda>k. full_view (kvs_of_gs s k)) \<sqsubseteq> (\<lambda>k. full_view (kvs_of_gs s' k))"
   using assms
   by (metis view_order_full_view_increasing kvs_of_gs_commit_length_increasing)
@@ -1242,9 +1242,18 @@ lemma updated_vl_view_grows:
 
 lemma cl_view_inv:
   assumes "gs_trans s e s'"
-    and "not_tm_commit e"
+    and "not_cl_commit e"
   shows "cl_view (cls s' cl) = cl_view (cls s cl)"
   using assms by (induction e) (auto simp add: tps_trans_defs unchanged_defs dest!:eq_for_all_cl)
+
+lemma updated_is_kvs_of_gs':
+  assumes "cl_state (cls s' cl) = cl_committed"
+      and "svr_cl_cl'_unchanged cl s s'"
+  shows "(\<lambda>k. full_view (updated_kvs s cl k)) = (\<lambda>k. full_view (kvs_of_gs s' k))"
+  using assms
+  apply (auto simp add: kvs_of_gs_def updated_kvs_def cl_unchanged_defs)
+  apply (rule ext, rule arg_cong[where f=full_view])
+  apply (rule arg_cong[where f="\<lambda>tStm. update_kv_all_txn tStm _ _ _"]) by auto
 
 definition TMFullView where
   "TMFullView s cl \<longleftrightarrow> cl_view (cls s cl) \<sqsubseteq> (\<lambda>k. full_view (kvs_of_gs s k))"
@@ -1252,7 +1261,7 @@ definition TMFullView where
 lemmas TMFullViewI = TMFullView_def[THEN iffD2, rule_format]
 lemmas TMFullViewE[elim] = TMFullView_def[THEN iffD1, elim_format, rule_format]
 
-lemma reach_tm_full_view [simp, dest]:
+lemma reach_cl_full_view [simp, dest]:
   assumes "reach tps s"
   shows "TMFullView s cl"
   using assms
@@ -1263,14 +1272,14 @@ proof(induction s arbitrary: cl rule: reach.induct)
         view_init_def kvs_of_gs_def)
 next
   case (reach_trans s e s')
-  then show ?case apply (cases "not_tm_commit e") using kvs_of_gs_inv[of s e s']
-    apply (auto simp add: TMFullView_def unchanged_defs cl_view_inv)
-    using committed_kvs_view_grows[of s]
-    apply (auto simp add: TMFullView_def tps_trans_defs tm_unchanged_defs)
+  then show ?case apply (cases "not_cl_commit e") using kvs_of_gs_inv[of s e s']
+    apply (auto simp add: TMFullView_def cl_view_inv)
+    using committed_kvs_view_grows[of s] updated_is_kvs_of_gs'[of s']
+    apply (auto simp add: TMFullView_def tps_trans_defs cl_unchanged_defs o_def)
     by (metis (no_types, lifting) view_order_refl view_order_transitive)
 qed
 
-\<comment> \<open>TM_commit updating kv\<close>
+\<comment> \<open>Cl_commit updating kv\<close>
 
 lemma or3_not_eq:
   assumes "\<forall>k. P k = a \<or> P k = b \<or> P k = c"
@@ -1278,30 +1287,30 @@ lemma or3_not_eq:
   shows "P k = a \<or> P k = b"
   using assms by auto
 
-lemma kvs_of_gs_tm_commit:
+lemma kvs_of_gs_cl_commit:
   assumes "TIDFutureKm s cl" and "TIDPastKm s cl"
     and "WLockInv s k" and "WLockFpInv s k"
     and "RLockInv s k" and "RLockFpInv s k"
     and "NoLockFpInv s k" and "KVSNonEmp s"
-    and "tm_state (cls s cl) = tm_prepared"
-    and "km_state (svrs s k) (get_txn_cl cl s) \<in> {read_lock, write_lock, no_lock}"
-    and "tm_state (cls s' cl) = tm_committed"
+    and "cl_state (cls s cl) = cl_prepared"
+    and "is_locked (svr_state (svrs s k) (get_txn_cl cl s))"
+    and "cl_state (cls s' cl) = cl_committed"
     and "other_insts_unchanged cl (cls s) (cls s')"
-  shows "update_kv_all_txn (\<lambda>t. tm_state (cls s' (get_cl_txn t))) (km_state (svrs s k))
+  shows "update_kv_all_txn (\<lambda>t. cl_state (cls s' (get_cl_txn t))) (svr_state (svrs s k))
           (svr_key_fp (svrs s k)) (svr_vl (svrs s k)) =
     update_kv_key (get_txn_cl cl s) (svr_key_fp (svrs s k) (get_txn_cl cl s))
-      (full_view (update_kv_all_txn (\<lambda>t. tm_state (cls s (get_cl_txn t))) (km_state (svrs s k))
+      (full_view (update_kv_all_txn (\<lambda>t. cl_state (cls s (get_cl_txn t))) (svr_state (svrs s k))
         (svr_key_fp (svrs s k)) (svr_vl (svrs s k))))
-      (update_kv_all_txn (\<lambda>t. tm_state (cls s (get_cl_txn t))) (km_state (svrs s k))
+      (update_kv_all_txn (\<lambda>t. cl_state (cls s (get_cl_txn t))) (svr_state (svrs s k))
         (svr_key_fp (svrs s k)) (svr_vl (svrs s k)))"
   using assms
   apply (auto simp add: update_kv_key_def)
-  subgoal using tm_commit_updates_kv_reads'[of s cl k s']
+  subgoal using cl_commit_updates_kv_reads'[of s cl k s']
     by (auto simp add: read_only_update' update_kv_writes_def)
-  subgoal using tm_commit_updates_kv_reads'[of s cl k s']
+  subgoal using cl_commit_updates_kv_reads'[of s cl k s']
     apply (simp add: writer_update_before)
     by (auto simp add: update_kv_all_txn_def update_kv_writes_all_txn_def the_wr_tI)
-  by (auto simp add: update_kv_writes_def update_kv_reads_def update_kv_all_tm_commit_no_lock_inv)
+  by (auto simp add: update_kv_writes_def update_kv_reads_def update_kv_all_cl_commit_no_lock_inv)
 
 \<comment> \<open>Lemmas about reader and writer transaction sets\<close>
 lemma update_kv_writes_all_txn_v_readerset_set:
@@ -1311,7 +1320,7 @@ lemma update_kv_writes_all_txn_v_readerset_set:
 \<comment> \<open>Lemmas for showing transaction id freshness\<close>
 
 lemma vl_writers_sqns_reads_other_cl_inv:
-  "vl_writers_sqns (update_kv_reads_all_txn (\<lambda>t. tm_state (cls s (get_cl_txn t))) tSkm tFk vl) = 
+  "vl_writers_sqns (update_kv_reads_all_txn (\<lambda>t. cl_state (cls s (get_cl_txn t))) tSkm tFk vl) = 
    vl_writers_sqns vl"
   unfolding vl_writers_sqns_def apply (rule ext)
   apply (auto simp add: vl_writers_def in_set_conv_nth image_iff)
@@ -1320,7 +1329,7 @@ lemma vl_writers_sqns_reads_other_cl_inv:
     by (metis (lifting) nth_list_update_eq nth_list_update_neq version.select_convs(2)
         version.surjective version.update_convs(3))
   subgoal for cl x i apply (rule bexI[where x="update_kv_reads_all_txn
-      (\<lambda>t. tm_state (cls s (get_cl_txn t))) tSkm tFk vl ! i"])
+      (\<lambda>t. cl_state (cls s (get_cl_txn t))) tSkm tFk vl ! i"])
      apply (auto simp add: update_kv_reads_all_defs)
     by (metis (lifting) nth_list_update_eq nth_list_update_neq version.select_convs(2)
         version.surjective version.update_convs(3))
@@ -1342,19 +1351,19 @@ lemma kvs_readers_sqns_other_cl_inv:
     and "\<And>k. WLockInv s k" and "\<And>k. WLockFpInv s k"
     and "\<And>k. RLockInv s k" and "\<And>k. RLockFpInv s k"
     and "\<And>k. NoLockFpInv s k" and "KVSNonEmp s"
-    and "tm_state (cls s cl) = tm_prepared"
-    and "tm_state (cls s' cl) = tm_committed"
-    and "\<And>k. km_state (svrs s k) (get_txn_cl cl s) \<in> {read_lock, write_lock, no_lock}"
+    and "cl_state (cls s cl) = cl_prepared"
+    and "cl_state (cls s' cl) = cl_committed"
+    and "\<And>k. is_locked (svr_state (svrs s k) (get_txn_cl cl s))"
     and "other_insts_unchanged cl (cls s) (cls s')"
     and "svrs s' = svrs s"
     and "cl' \<noteq> cl"
   shows "kvs_readers_sqns (kvs_of_gs s') cl' = kvs_readers_sqns (kvs_of_gs s) cl'"
   using assms
   apply (auto simp add: kvs_readers_sqns_def kvs_of_gs_def)
-  subgoal for x k using kvs_of_gs_tm_commit[of s cl k s'] apply (simp add: KVSNonEmp_def)
+  subgoal for x k using kvs_of_gs_cl_commit[of s cl k s'] apply (simp add: KVSNonEmp_def)
   apply (rule exI[where x=k])
   by (smt (verit) other_insts_unchanged_def update_kv_all_txn_non_empty vl_readers_sqns_other_cl_inv)
-  subgoal for x k using kvs_of_gs_tm_commit[of s cl k s'] apply (simp add: KVSNonEmp_def)
+  subgoal for x k using kvs_of_gs_cl_commit[of s cl k s'] apply (simp add: KVSNonEmp_def)
   apply (rule exI[where x=k])
     by (smt (verit) assms(10, 12, 14) other_insts_unchanged_def update_kv_all_txn_non_empty
         vl_readers_sqns_other_cl_inv)
@@ -1376,18 +1385,18 @@ lemma kvs_writers_sqns_other_cl_inv:
     and "\<And>k. WLockInv s k" and "\<And>k. WLockFpInv s k"
     and "\<And>k. RLockInv s k" and "\<And>k. RLockFpInv s k"
     and "\<And>k. NoLockFpInv s k" and "KVSNonEmp s"
-    and "tm_state (cls s cl) = tm_prepared"
-    and "tm_state (cls s' cl) = tm_committed"
-    and "\<And>k. km_state (svrs s k) (get_txn_cl cl s) \<in> {read_lock, write_lock, no_lock}"
+    and "cl_state (cls s cl) = cl_prepared"
+    and "cl_state (cls s' cl) = cl_committed"
+    and "\<And>k. is_locked (svr_state (svrs s k) (get_txn_cl cl s))"
     and "other_insts_unchanged cl (cls s) (cls s')"
     and "svrs s' = svrs s"
     and "cl' \<noteq> cl"
   shows "kvs_writers_sqns (kvs_of_gs s') cl' = kvs_writers_sqns (kvs_of_gs s) cl'"
   using assms
   apply (auto simp add: kvs_writers_sqns_def kvs_of_gs_def)
-  subgoal for x k using kvs_of_gs_tm_commit[of s cl k s'] apply simp apply (rule exI[where x=k])
+  subgoal for x k using kvs_of_gs_cl_commit[of s cl k s'] apply simp apply (rule exI[where x=k])
     by (smt (verit) other_insts_unchanged_def vl_writers_sqns_other_cl_inv)
-  subgoal for x k using kvs_of_gs_tm_commit[of s cl k s'] apply simp apply (rule exI[where x=k])
+  subgoal for x k using kvs_of_gs_cl_commit[of s cl k s'] apply simp apply (rule exI[where x=k])
     by (smt (verit) other_insts_unchanged_def vl_writers_sqns_other_cl_inv)
   done
 
@@ -1396,29 +1405,29 @@ lemma get_sqns_other_cl_inv:
     and "\<And>k. WLockInv s k" and "\<And>k. WLockFpInv s k"
     and "\<And>k. RLockInv s k" and "\<And>k. RLockFpInv s k"
     and "\<And>k. NoLockFpInv s k" and "KVSNonEmp s"
-    and "tm_state (cls s cl) = tm_prepared"
-    and "tm_state (cls s' cl) = tm_committed"
-    and "\<And>k. km_state (svrs s k) (get_txn_cl cl s) = read_lock \<or>
-             km_state (svrs s k) (get_txn_cl cl s) = write_lock \<or> 
-             km_state (svrs s k) (get_txn_cl cl s) = no_lock"
-    and "km_tm_cl'_unchanged cl s s'"
+    and "cl_state (cls s cl) = cl_prepared"
+    and "cl_state (cls s' cl) = cl_committed"
+    and "\<And>k. svr_state (svrs s k) (get_txn_cl cl s) = read_lock \<or>
+             svr_state (svrs s k) (get_txn_cl cl s) = write_lock \<or> 
+             svr_state (svrs s k) (get_txn_cl cl s) = no_lock"
+    and "svr_cl_cl'_unchanged cl s s'"
     and "cl' \<noteq> cl"
   shows "get_sqns (kvs_of_gs s') cl' = get_sqns (kvs_of_gs s) cl'"
   using assms by (auto simp add: get_sqns_def kvs_writers_sqns_other_cl_inv
-      kvs_readers_sqns_other_cl_inv tm_unchanged_defs)
+      kvs_readers_sqns_other_cl_inv cl_unchanged_defs)
 
 lemma new_t_is_in_writers:
   assumes "TIDFutureKm s cl" and "TIDPastKm s cl"
     and "\<And>k. WLockInv s k" and "\<And>k. WLockFpInv s k"
     and "\<And>k. RLockInv s k" and "\<And>k. RLockFpInv s k"
     and "\<And>k. NoLockFpInv s k" and "KVSNonEmp s"
-    and "tm_state (cls s cl) = tm_prepared"
-    and "tm_state (cls s' cl) = tm_committed"
-    and "km_state (svrs s k) (get_txn_cl cl s) = write_lock"
+    and "cl_state (cls s cl) = cl_prepared"
+    and "cl_state (cls s' cl) = cl_committed"
+    and "svr_state (svrs s k) (get_txn_cl cl s) = write_lock"
     and "other_insts_unchanged cl (cls s) (cls s')"
     and "svrs s' = svrs s"
   shows "vl_writers_sqns (kvs_of_gs s' k) cl = vl_writers_sqns (kvs_of_gs s k) cl \<union> {cl_sn (cls s cl)}"
-  using assms kvs_of_gs_tm_commit[of s cl k s']
+  using assms kvs_of_gs_cl_commit[of s cl k s']
   by (auto simp add: kvs_of_gs_def vl_writers_sqns_def update_kv_key_def
       update_kv_writes_def split: option.split)
 
@@ -1427,13 +1436,13 @@ lemma new_t_is_in_writers2:
     and "\<And>k. WLockInv s k" and "\<And>k. WLockFpInv s k"
     and "\<And>k. RLockInv s k" and "\<And>k. RLockFpInv s k"
     and "\<And>k. NoLockFpInv s k" and "KVSNonEmp s"
-    and "tm_state (cls s cl) = tm_prepared"
-    and "tm_state (cls s' cl) = tm_committed"
-    and "km_state (svrs s k) (get_txn_cl cl s) = read_lock"
+    and "cl_state (cls s cl) = cl_prepared"
+    and "cl_state (cls s' cl) = cl_committed"
+    and "svr_state (svrs s k) (get_txn_cl cl s) = read_lock"
     and "other_insts_unchanged cl (cls s) (cls s')"
     and "svrs s' = svrs s"
   shows "vl_writers_sqns (kvs_of_gs s' k) cl = vl_writers_sqns (kvs_of_gs s k) cl"
-  using assms kvs_of_gs_tm_commit[of s cl k s']
+  using assms kvs_of_gs_cl_commit[of s cl k s']
   apply (auto simp add: kvs_of_gs_def vl_writers_sqns_def update_kv_key_def update_kv_writes_def
       split: option.split)
   by (metis RLockFpInv_def option.discI)
@@ -1443,13 +1452,13 @@ lemma new_t_is_in_readers:
     and "\<And>k. WLockInv s k" and "\<And>k. WLockFpInv s k"
     and "\<And>k. RLockInv s k" and "\<And>k. RLockFpInv s k"
     and "\<And>k. NoLockFpInv s k" and "KVSNonEmp s"
-    and "tm_state (cls s cl) = tm_prepared"
-    and "tm_state (cls s' cl) = tm_committed"
-    and "km_state (svrs s k) (get_txn_cl cl s) = read_lock"
+    and "cl_state (cls s cl) = cl_prepared"
+    and "cl_state (cls s' cl) = cl_committed"
+    and "svr_state (svrs s k) (get_txn_cl cl s) = read_lock"
     and "other_insts_unchanged cl (cls s) (cls s')"
     and "svrs s' = svrs s"
   shows "vl_readers_sqns (kvs_of_gs s' k) cl = vl_readers_sqns (kvs_of_gs s k) cl \<union> {cl_sn (cls s cl)}"
-  using assms kvs_of_gs_tm_commit[of s cl k s']
+  using assms kvs_of_gs_cl_commit[of s cl k s']
   apply (auto simp add: kvs_of_gs_def update_kv_key_def update_kv_writes_def vl_readers_sqns_def
       RLockFpInv_def update_kv_reads_vl_readers_inv KVSNonEmp_def split: option.split)
   by (meson RLockFpInv_def assms(6))
@@ -1459,14 +1468,14 @@ lemma new_t_is_in_readers2:
     and "\<And>k. WLockInv s k" and "\<And>k. WLockFpInv s k"
     and "\<And>k. RLockInv s k" and "\<And>k. RLockFpInv s k"
     and "\<And>k. NoLockFpInv s k" and "KVSNonEmp s"
-    and "tm_state (cls s cl) = tm_prepared"
-    and "tm_state (cls s' cl) = tm_committed"
-    and "km_state (svrs s k) (get_txn_cl cl s) = write_lock"
+    and "cl_state (cls s cl) = cl_prepared"
+    and "cl_state (cls s' cl) = cl_committed"
+    and "svr_state (svrs s k) (get_txn_cl cl s) = write_lock"
     and "svr_key_fp (svrs s k) (get_txn_cl cl s) R \<noteq> None"
     and "other_insts_unchanged cl (cls s) (cls s')"
     and "svrs s' = svrs s"
   shows "vl_readers_sqns (kvs_of_gs s' k) cl = vl_readers_sqns (kvs_of_gs s k) cl \<union> {cl_sn (cls s cl)}"
-  using assms kvs_of_gs_tm_commit[of s cl k s']
+  using assms kvs_of_gs_cl_commit[of s cl k s']
   by (auto simp add: kvs_of_gs_def update_kv_key_def update_kv_writes_def vl_readers_sqns_def
        update_kv_reads_vl_readers_inv split: option.split)
 
@@ -1475,26 +1484,26 @@ lemma new_t_is_in_readers3:
     and "\<And>k. WLockInv s k" and "\<And>k. WLockFpInv s k"
     and "\<And>k. RLockInv s k" and "\<And>k. RLockFpInv s k"
     and "\<And>k. NoLockFpInv s k" and "KVSNonEmp s"
-    and "tm_state (cls s cl) = tm_prepared"
-    and "tm_state (cls s' cl) = tm_committed"
-    and "km_state (svrs s k) (get_txn_cl cl s) = write_lock"
+    and "cl_state (cls s cl) = cl_prepared"
+    and "cl_state (cls s' cl) = cl_committed"
+    and "svr_state (svrs s k) (get_txn_cl cl s) = write_lock"
     and "svr_key_fp (svrs s k) (get_txn_cl cl s) R = None"
     and "other_insts_unchanged cl (cls s) (cls s')"
     and "svrs s' = svrs s"
   shows "vl_readers_sqns (kvs_of_gs s' k) cl = vl_readers_sqns (kvs_of_gs s k) cl"
-  using assms kvs_of_gs_tm_commit[of s cl k s']
+  using assms kvs_of_gs_cl_commit[of s cl k s']
   by (auto simp add: kvs_of_gs_def update_kv_key_def update_kv_writes_def vl_readers_sqns_def
        update_kv_reads_vl_readers_inv split: option.split)
 
-lemma kvs_writers_tm_commit_grows:
+lemma kvs_writers_cl_commit_grows:
   assumes "TIDFutureKm s cl" and "TIDPastKm s cl"
     and "\<And>k. WLockInv s k" and "\<And>k. WLockFpInv s k"
     and "\<And>k. RLockInv s k" and "\<And>k. RLockFpInv s k"
     and "\<And>k. NoLockFpInv s k" and "KVSNonEmp s"
-    and "tm_state (cls s cl) = tm_prepared"
-    and "tm_state (cls s' cl) = tm_committed"
-    and "\<forall>k. km_state (svrs s k) (get_txn_cl cl s) \<in> {read_lock, write_lock, no_lock}"
-    and "km_state (svrs s k) (get_txn_cl cl s) = write_lock"
+    and "cl_state (cls s cl) = cl_prepared"
+    and "cl_state (cls s' cl) = cl_committed"
+    and "\<forall>k. is_locked (svr_state (svrs s k) (get_txn_cl cl s))"
+    and "svr_state (svrs s k) (get_txn_cl cl s) = write_lock"
     and "other_insts_unchanged cl (cls s) (cls s')"
     and "svrs s' = svrs s"
   shows "kvs_writers_sqns (kvs_of_gs s') cl = kvs_writers_sqns (kvs_of_gs s) cl \<union> {cl_sn (cls s cl)}"
@@ -1503,42 +1512,42 @@ lemma kvs_writers_tm_commit_grows:
   subgoal for x k' apply (auto elim!: allE[where x=k']; cases "k' = k", simp_all)
     apply (metis kvs_of_gs_def read_only_update' vl_writers_sqns_reads_other_cl_inv)
     apply (metis Un_empty_right Un_insert_right assms(3-7) insert_iff new_t_is_in_writers)
-    by (metis kvs_of_gs_def update_kv_all_tm_commit_no_lock_inv)
+    by (metis kvs_of_gs_def update_kv_all_cl_commit_no_lock_inv)
   subgoal for x k' apply (rule exI[where x=k'])
     by (smt (verit, ccfv_SIG) UnCI assms(13) kvs_of_gs_def new_t_is_in_writers new_t_is_in_writers2
-        update_kv_all_tm_commit_no_lock_inv)
+        update_kv_all_cl_commit_no_lock_inv)
   done
 
-lemma kvs_writers_tm_commit_doesnt_grow:
+lemma kvs_writers_cl_commit_doesnt_grow:
   assumes "TIDFutureKm s cl" and "TIDPastKm s cl"
     and "\<And>k. WLockInv s k" and "\<And>k. WLockFpInv s k"
     and "\<And>k. RLockInv s k" and "\<And>k. RLockFpInv s k"
     and "\<And>k. NoLockFpInv s k" and "KVSNonEmp s"
-    and "tm_state (cls s cl) = tm_prepared"
-    and "tm_state (cls s' cl) = tm_committed"
-    and "\<forall>k. km_state (svrs s k) (get_txn_cl cl s) \<in> {read_lock, no_lock}"
+    and "cl_state (cls s cl) = cl_prepared"
+    and "cl_state (cls s' cl) = cl_committed"
+    and "\<forall>k. svr_state (svrs s k) (get_txn_cl cl s) \<in> {read_lock, no_lock}"
     and "other_insts_unchanged cl (cls s) (cls s')"
     and "svrs s' = svrs s"
   shows "kvs_writers_sqns (kvs_of_gs s') cl = kvs_writers_sqns (kvs_of_gs s) cl"
   using assms apply (auto simp add: kvs_writers_sqns_def)
   subgoal for x k apply (auto elim!: allE[where x=k])
     apply (metis assms(3-7) new_t_is_in_writers2)
-    by (metis kvs_of_gs_def update_kv_all_tm_commit_no_lock_inv)
+    by (metis kvs_of_gs_def update_kv_all_cl_commit_no_lock_inv)
   subgoal for x k  apply (auto elim!: allE[where x=k])
     apply (metis assms(3-7) new_t_is_in_writers2)
-    by (metis kvs_of_gs_def update_kv_all_tm_commit_no_lock_inv)
+    by (metis kvs_of_gs_def update_kv_all_cl_commit_no_lock_inv)
   done
 
-lemma kvs_readers_sqns_tm_commit_grows:
+lemma kvs_readers_sqns_cl_commit_grows:
   assumes "TIDFutureKm s cl" and "TIDPastKm s cl"
     and "\<And>k. WLockInv s k" and "\<And>k. WLockFpInv s k"
     and "\<And>k. RLockInv s k" and "\<And>k. RLockFpInv s k"
     and "\<And>k. NoLockFpInv s k" and "KVSNonEmp s"
-    and "tm_state (cls s cl) = tm_prepared"
-    and "tm_state (cls s' cl) = tm_committed"
-    and "\<forall>k. km_state (svrs s k) (get_txn_cl cl s) \<in> {read_lock, write_lock, no_lock}"
-    and "km_state (svrs s k) (get_txn_cl cl s) = read_lock \<or>
-         (km_state (svrs s k) (get_txn_cl cl s) = write_lock \<and>
+    and "cl_state (cls s cl) = cl_prepared"
+    and "cl_state (cls s' cl) = cl_committed"
+    and "\<forall>k. is_locked (svr_state (svrs s k) (get_txn_cl cl s))"
+    and "svr_state (svrs s k) (get_txn_cl cl s) = read_lock \<or>
+         (svr_state (svrs s k) (get_txn_cl cl s) = write_lock \<and>
           svr_key_fp (svrs s k) (get_txn_cl cl s) R \<noteq> None)"
     and "other_insts_unchanged cl (cls s) (cls s')"
     and "svrs s' = svrs s"
@@ -1549,33 +1558,33 @@ lemma kvs_readers_sqns_tm_commit_grows:
     apply (metis (no_types) Un_insert_right assms(3-7) insert_iff new_t_is_in_readers sup_bot_right)
     apply (metis (no_types) Un_insert_right assms(3-7) insert_iff new_t_is_in_readers2
       new_t_is_in_readers3 sup_bot_right)
-    apply (metis kvs_of_gs_def update_kv_all_tm_commit_no_lock_inv)
+    apply (metis kvs_of_gs_def update_kv_all_cl_commit_no_lock_inv)
     apply (metis (no_types) Un_insert_right assms(3-7) insert_iff new_t_is_in_readers sup_bot_right)
     apply (metis (no_types) Un_insert_right assms(3-7) insert_iff new_t_is_in_readers2
       new_t_is_in_readers3 sup_bot_right)
-    by (metis kvs_of_gs_def update_kv_all_tm_commit_no_lock_inv)
+    by (metis kvs_of_gs_def update_kv_all_cl_commit_no_lock_inv)
    subgoal apply (rule exI[where x=k])
      by (metis UnI2 assms(12,13) new_t_is_in_readers new_t_is_in_readers2 singletonI)
    subgoal for x k' apply (auto elim!: allE[where x=k'])
      apply (metis Un_iff assms(3-7) new_t_is_in_readers)
      apply (smt (verit) Un_insert_left assms(3-7) insert_iff mk_disjoint_insert
        new_t_is_in_readers2 new_t_is_in_readers3)
-     apply (metis kvs_of_gs_def update_kv_all_tm_commit_no_lock_inv)
+     apply (metis kvs_of_gs_def update_kv_all_cl_commit_no_lock_inv)
      apply (metis Un_iff assms(3-7) new_t_is_in_readers)
      apply (smt (verit) Un_insert_left assms(3-7) insert_iff mk_disjoint_insert
        new_t_is_in_readers2 new_t_is_in_readers3)
-     by (metis kvs_of_gs_def update_kv_all_tm_commit_no_lock_inv)
+     by (metis kvs_of_gs_def update_kv_all_cl_commit_no_lock_inv)
    done
 
-lemma kvs_readers_sqns_tm_commit_doesnt_grow:
+lemma kvs_readers_sqns_cl_commit_doesnt_grow:
   assumes "TIDFutureKm s cl" and "TIDPastKm s cl"
     and "\<And>k. WLockInv s k" and "\<And>k. WLockFpInv s k"
     and "\<And>k. RLockInv s k" and "\<And>k. RLockFpInv s k"
     and "\<And>k. NoLockFpInv s k" and "KVSNonEmp s"
-    and "tm_state (cls s cl) = tm_prepared"
-    and "tm_state (cls s' cl) = tm_committed"
-    and "\<forall>k. km_state (svrs s k) (get_txn_cl cl s) \<in> {write_lock, no_lock}"
-    and "\<forall>k. km_state (svrs s k) (get_txn_cl cl s) \<noteq> write_lock \<or>
+    and "cl_state (cls s cl) = cl_prepared"
+    and "cl_state (cls s' cl) = cl_committed"
+    and "\<forall>k. svr_state (svrs s k) (get_txn_cl cl s) \<in> {write_lock, no_lock}"
+    and "\<forall>k. svr_state (svrs s k) (get_txn_cl cl s) \<noteq> write_lock \<or>
              svr_key_fp (svrs s k) (get_txn_cl cl s) R = None"
     and "other_insts_unchanged cl (cls s) (cls s')"
     and "svrs s' = svrs s"
@@ -1583,41 +1592,41 @@ lemma kvs_readers_sqns_tm_commit_doesnt_grow:
   using assms apply (auto simp add: kvs_readers_sqns_def)
   subgoal for x k apply (auto elim!: allE[where x=k])
     apply (metis assms(1, 3-7) new_t_is_in_readers3)
-    by (metis kvs_of_gs_def update_kv_all_tm_commit_no_lock_inv)+
+    by (metis kvs_of_gs_def update_kv_all_cl_commit_no_lock_inv)+
   subgoal for x k  apply (auto elim!: allE[where x=k])
     apply (metis assms(1, 3-7) new_t_is_in_readers3)
-    by (metis kvs_of_gs_def update_kv_all_tm_commit_no_lock_inv)+
+    by (metis kvs_of_gs_def update_kv_all_cl_commit_no_lock_inv)+
   done
 
-lemma get_sqns_tm_commit_grows:
+lemma get_sqns_cl_commit_grows:
   assumes "TIDFutureKm s cl" and "TIDPastKm s cl"
     and "\<And>k. WLockInv s k" and "\<And>k. WLockFpInv s k"
     and "\<And>k. RLockInv s k" and "\<And>k. RLockFpInv s k"
     and "\<And>k. NoLockFpInv s k" and "KVSNonEmp s"
-    and "tm_state (cls s cl) = tm_prepared"
-    and "tm_state (cls s' cl) = tm_committed"
-    and "\<And>k. km_state (svrs s k) (get_txn_cl cl s) \<in> {read_lock, write_lock, no_lock}"
+    and "cl_state (cls s cl) = cl_prepared"
+    and "cl_state (cls s' cl) = cl_committed"
+    and "\<And>k. is_locked (svr_state (svrs s k) (get_txn_cl cl s))"
     and "other_insts_unchanged cl (cls s) (cls s')"
     and "svrs s' = svrs s"
   shows "get_sqns (kvs_of_gs s') cl =
-         (if \<forall>k. km_state (svrs s k) (get_txn_cl cl s) = no_lock then
+         (if \<forall>k. svr_state (svrs s k) (get_txn_cl cl s) = no_lock then
           get_sqns (kvs_of_gs s) cl else
           get_sqns (kvs_of_gs s) cl \<union> {cl_sn (cls s cl)})"
   using assms
-  apply (cases "\<forall>k. km_state (svrs s k) (get_txn_cl cl s) = no_lock")
-   apply (simp add: kvs_of_gs_def update_kv_all_tm_commit_no_lock_inv)
+  apply (cases "\<forall>k. svr_state (svrs s k) (get_txn_cl cl s) = no_lock")
+   apply (simp add: kvs_of_gs_def update_kv_all_cl_commit_no_lock_inv)
   apply simp apply (rule conjI) apply blast
   apply (simp add: get_sqns_def)
-  using kvs_readers_sqns_tm_commit_doesnt_grow[of s cl s']
-        kvs_readers_sqns_tm_commit_grows[of s cl s']
-        kvs_writers_tm_commit_doesnt_grow[of s cl s']
-        kvs_writers_tm_commit_grows[of s cl s']
+  using kvs_readers_sqns_cl_commit_doesnt_grow[of s cl s']
+        kvs_readers_sqns_cl_commit_grows[of s cl s']
+        kvs_writers_cl_commit_doesnt_grow[of s cl s']
+        kvs_writers_cl_commit_grows[of s cl s']
   by (smt (z3) Un_insert_right insertCI sup.right_idem sup_bot_right sup_commute)
 
 definition SqnInv where
   "SqnInv s cl \<longleftrightarrow>
-    (tm_state (cls s cl) \<noteq> tm_committed \<longrightarrow> (\<forall>m \<in> get_sqns (kvs_of_gs s) cl. m < cl_sn (cls s cl))) \<and>
-    (tm_state (cls s cl) = tm_committed \<longrightarrow> (\<forall>m \<in> get_sqns (kvs_of_gs s) cl. m \<le> cl_sn (cls s cl)))"
+    (cl_state (cls s cl) \<noteq> cl_committed \<longrightarrow> (\<forall>m \<in> get_sqns (kvs_of_gs s) cl. m < cl_sn (cls s cl))) \<and>
+    (cl_state (cls s cl) = cl_committed \<longrightarrow> (\<forall>m \<in> get_sqns (kvs_of_gs s) cl. m \<le> cl_sn (cls s cl)))"
 
 lemmas SqnInvI = SqnInv_def[THEN iffD2, rule_format]
 lemmas SqnInvE[elim] = SqnInv_def[THEN iffD1, elim_format, rule_format]
@@ -1639,88 +1648,88 @@ next
   proof (induction e)
     case (WLock x1 x2 x3 x4)
     then show ?case
-      by (auto simp add: SqnInv_def tps_trans_defs km_unchanged_defs)
+      by (auto simp add: SqnInv_def tps_trans_defs svr_unchanged_defs)
   next
     case (NoLock x1 x2)
     then show ?case
-      by (auto simp add: SqnInv_def tps_trans_defs km_unchanged_defs)
+      by (auto simp add: SqnInv_def tps_trans_defs svr_unchanged_defs)
   next
     case (User_Commit x)
     then show ?case
-      apply (auto simp add: SqnInv_def tps_trans_defs tm_unchanged_defs)
-      apply (metis state_tm.distinct(3))
-      by (metis state_tm.distinct(7))
+      apply (auto simp add: SqnInv_def tps_trans_defs cl_unchanged_defs)
+      apply (metis state_cl.distinct(3))
+      by (metis state_cl.distinct(7))
   next
-    case (TM_Commit x1 x2 x3 x4)
+    case (Cl_Commit x1 x2 x3 x4)
     then show ?case
       apply (auto simp add: SqnInv_def tps_trans_defs) using get_sqns_other_cl_inv
-      apply (smt (verit) tm_unchanged_defs reach_kvs_non_emp reach_nolockfp reach_rlock
+      apply (smt (verit) cl_unchanged_defs reach_kvs_non_emp reach_nolockfp reach_rlock
           reach_rlockfp reach_tidfuturekm reach_tidpastkm reach_wlock reach_wlockfp)
       apply (cases "cl = x1")
-      using get_sqns_tm_commit_grows[of s cl s']
-      apply (smt (z3) tm_unchanged_defs UnE insert_absorb insert_iff insert_not_empty order.strict_implies_order
+      using get_sqns_cl_commit_grows[of s cl s']
+      apply (smt (z3) cl_unchanged_defs UnE insert_absorb insert_iff insert_not_empty order.strict_implies_order
         order_class.order_eq_iff other_insts_unchanged_def reach_kvs_non_emp reach_nolockfp
         reach_rlock reach_rlockfp reach_tidfuturekm reach_tidpastkm reach_wlock reach_wlockfp)
       using get_sqns_other_cl_inv
-      by (smt (verit) tm_unchanged_defs reach_kvs_non_emp reach_nolockfp reach_rlock
+      by (smt (verit) cl_unchanged_defs reach_kvs_non_emp reach_nolockfp reach_rlock
           reach_rlockfp reach_tidfuturekm reach_tidpastkm reach_wlock reach_wlockfp)
   next
-    case (TM_Abort x)
-    then show ?case apply (auto simp add: SqnInv_def tps_trans_defs tm_unchanged_defs)
-    apply (metis state_tm.distinct(7)) by (metis state_tm.distinct(11))
+    case (Cl_Abort x)
+    then show ?case apply (auto simp add: SqnInv_def tps_trans_defs cl_unchanged_defs)
+    apply (metis state_cl.distinct(7)) by (metis state_cl.distinct(11))
   next
-    case (TM_ReadyC x)
-    then show ?case apply (auto simp add: SqnInv_def tps_trans_defs tm_unchanged_defs)
-    apply (metis less_Suc_eq_le) by (metis state_tm.distinct(3))
+    case (Cl_ReadyC x)
+    then show ?case apply (auto simp add: SqnInv_def tps_trans_defs cl_unchanged_defs)
+    apply (metis less_Suc_eq_le) by (metis state_cl.distinct(3))
   next
-    case (TM_ReadyA x)
-    then show ?case apply (auto simp add: SqnInv_def tps_trans_defs tm_unchanged_defs)
-    apply (metis less_Suc_eq state_tm.distinct(11)) by (metis state_tm.distinct(3))
-  qed (auto simp add: SqnInv_def tps_trans_defs km_unchanged_defs)
+    case (Cl_ReadyA x)
+    then show ?case apply (auto simp add: SqnInv_def tps_trans_defs cl_unchanged_defs)
+    apply (metis less_Suc_eq state_cl.distinct(11)) by (metis state_cl.distinct(3))
+  qed (auto simp add: SqnInv_def tps_trans_defs svr_unchanged_defs)
 qed
 
 \<comment> \<open>Lemmas for proving view wellformedness of cl_view\<close>
 
 lemma helper_lemma:
-  assumes "i \<in> full_view (update_kv_reads_all_txn (\<lambda>t. tm_state (cls s (get_cl_txn t)))
-    (km_state (svrs s k)) (svr_key_fp (svrs s k)) (svr_vl (svrs s k)))"
+  assumes "i \<in> full_view (update_kv_reads_all_txn (\<lambda>t. cl_state (cls s (get_cl_txn t)))
+    (svr_state (svrs s k)) (svr_key_fp (svrs s k)) (svr_vl (svrs s k)))"
   shows "
-  update_kv_writes (the_wr_t (km_state (svrs s k))) (svr_key_fp (svrs s k) (the_wr_t (km_state (svrs s k))))
-    (update_kv_reads_all_txn (\<lambda>t. tm_state (cls s' (get_cl_txn t))) (km_state (svrs s k))
+  update_kv_writes (the_wr_t (svr_state (svrs s k))) (svr_key_fp (svrs s k) (the_wr_t (svr_state (svrs s k))))
+    (update_kv_reads_all_txn (\<lambda>t. cl_state (cls s' (get_cl_txn t))) (svr_state (svrs s k))
       (svr_key_fp (svrs s k)) (svr_vl (svrs s k))) ! i =
-  update_kv_reads_all_txn (\<lambda>t. tm_state (cls s' (get_cl_txn t))) (km_state (svrs s k))
+  update_kv_reads_all_txn (\<lambda>t. cl_state (cls s' (get_cl_txn t))) (svr_state (svrs s k))
     (svr_key_fp (svrs s k)) (svr_vl (svrs s k)) ! i"
   using assms
-  update_kv_writes_version_inv[of i "update_kv_reads_all_txn (\<lambda>t. tm_state (cls s' (get_cl_txn t)))
-   (km_state (svrs s k)) (svr_key_fp (svrs s k)) (svr_vl (svrs s k))" "the_wr_t (km_state (svrs s k))"
-   "svr_key_fp (svrs s k) (the_wr_t (km_state (svrs s k)))"]
+  update_kv_writes_version_inv[of i "update_kv_reads_all_txn (\<lambda>t. cl_state (cls s' (get_cl_txn t)))
+   (svr_state (svrs s k)) (svr_key_fp (svrs s k)) (svr_vl (svrs s k))" "the_wr_t (svr_state (svrs s k))"
+   "svr_key_fp (svrs s k) (the_wr_t (svr_state (svrs s k)))"]
   by (simp add: full_view_def)
 
 lemma kvs_of_gs_version_order:
   assumes "TIDPastKm s cl" and "TIDFutureKm s cl" and "WLockInv s k" and "RLockInv s k" and "KVSNonEmp s"
     and "i \<in> full_view (kvs_of_gs s k)"
-    and "tm_state (cls s cl) = tm_prepared"
-    and "tm_state (cls s' cl) = tm_committed"
-    and "km_state (svrs s k) (get_txn_cl cl s) \<in> {read_lock, write_lock, no_lock}"
-    and "km_tm_cl'_unchanged cl s s'"
+    and "cl_state (cls s cl) = cl_prepared"
+    and "cl_state (cls s' cl) = cl_committed"
+    and "is_locked (svr_state (svrs s k) (get_txn_cl cl s))"
+    and "svr_cl_cl'_unchanged cl s s'"
   shows "kvs_of_gs s k ! i \<sqsubseteq>\<^sub>v\<^sub>e\<^sub>r kvs_of_gs s' k ! i"
   using assms
-  apply (auto simp add: kvs_of_gs_def km_tm_cl'_unchanged_def update_kv_all_tm_commit_no_lock_inv)
+  apply (auto simp add: kvs_of_gs_def svr_cl_cl'_unchanged_def update_kv_all_cl_commit_no_lock_inv)
    apply (simp_all add: writer_update_before read_only_update')
    apply (auto simp add: update_kv_all_txn_def update_kv_writes_all_txn_def helper_lemma)
    apply (auto simp add: version_order_def)
-   using tm_commit_updates_kv_reads[of s s' cl k] 
-     expanding_feature3'[where vl="update_kv_reads_all_txn (\<lambda>t. tm_state (cls s (get_cl_txn t)))
-      (km_state (svrs s k)) (svr_key_fp (svrs s k)) (svr_vl (svrs s k))"]
+   using cl_commit_updates_kv_reads[of s s' cl k] 
+     expanding_feature3'[where vl="update_kv_reads_all_txn (\<lambda>t. cl_state (cls s (get_cl_txn t)))
+      (svr_state (svrs s k)) (svr_key_fp (svrs s k)) (svr_vl (svrs s k))"]
    by (auto simp add: update_kv_reads_all_defs)
 
 lemma new_writer:
   assumes "WLockInv s k" and "WLockFpInv s k"
-    and "tm_state (cls s' cl) = tm_committed"
-    and "km_state (svrs s k) (get_txn_cl cl s) = write_lock"
-  shows "v_writer (update_kv_all_txn (\<lambda>t. tm_state (cls s' (get_cl_txn t))) (km_state (svrs s k))
+    and "cl_state (cls s' cl) = cl_committed"
+    and "svr_state (svrs s k) (get_txn_cl cl s) = write_lock"
+  shows "v_writer (update_kv_all_txn (\<lambda>t. cl_state (cls s' (get_cl_txn t))) (svr_state (svrs s k))
     (svr_key_fp (svrs s k)) (svr_vl (svrs s k)) ! length (svr_vl (svrs s k))) =
-   Tn (the_wr_t (km_state (svrs s k)))"
+   Tn (the_wr_t (svr_state (svrs s k)))"
   using assms
   apply (auto simp add: update_kv_all_txn_def update_kv_writes_all_txn_def update_kv_writes_def
       the_wr_tI split: option.split)
@@ -1735,21 +1744,21 @@ lemma update_kv_all_txn_v_writer_inv:
 lemma new_version_index:
   assumes "TIDPastKm s cl" and "TIDFutureKm s cl"
     and "WLockInv s k" and "KVSNonEmp s"
-    and "tm_state (cls s cl) = tm_prepared"
-    and "tm_state (cls s' cl) = tm_committed"
-    and "km_state (svrs s k) (get_txn_cl cl s) = write_lock"
+    and "cl_state (cls s cl) = cl_prepared"
+    and "cl_state (cls s' cl) = cl_committed"
+    and "svr_state (svrs s k) (get_txn_cl cl s) = write_lock"
     and "other_insts_unchanged cl (cls s) (cls s')"
-    and "i \<in> full_view (update_kv_all_txn (\<lambda>t. tm_state (cls s' (get_cl_txn t)))
-    (km_state (svrs s k)) (svr_key_fp (svrs s k)) (svr_vl (svrs s k)))"
-    and "i \<notin> full_view (update_kv_all_txn (\<lambda>t. tm_state (cls s (get_cl_txn t)))
-    (km_state (svrs s k)) (svr_key_fp (svrs s k)) (svr_vl (svrs s k)))"
+    and "i \<in> full_view (update_kv_all_txn (\<lambda>t. cl_state (cls s' (get_cl_txn t)))
+    (svr_state (svrs s k)) (svr_key_fp (svrs s k)) (svr_vl (svrs s k)))"
+    and "i \<notin> full_view (update_kv_all_txn (\<lambda>t. cl_state (cls s (get_cl_txn t)))
+    (svr_state (svrs s k)) (svr_key_fp (svrs s k)) (svr_vl (svrs s k)))"
   shows "i = length (svr_vl (svrs s k))"
   using assms
   by (meson full_view_length_increasing index_in_longer_kv update_kv_all_txn_length_increasing)
 
 lemma t_is_fresh:
   assumes "SqnInv s cl"
-    and "tm_state (cls s cl) = tm_prepared"
+    and "cl_state (cls s cl) = cl_prepared"
   shows "get_txn_cl cl s \<in> next_txids (kvs_of_gs s) cl"
   using assms by (auto simp add: kvs_of_gs_def next_txids_def SqnInv_def)
 
@@ -1758,27 +1767,27 @@ lemma kvs_of_gs_view_atomic:
     and "\<And>k. WLockInv s k" and "\<And>k. WLockFpInv s k"
     and "\<And>k. RLockInv s k" and "\<And>k. NoLockFpInv s k"
     and "SqnInv s cl" and "KVSNonEmp s"
-    and "tm_state (cls s cl) = tm_prepared"
-    and "tm_state (cls s' cl) = tm_committed"
-    and "\<forall>k. km_state (svrs s k) (get_txn_cl cl s) \<in> {read_lock, write_lock, no_lock}"
-    and "km_tm_cl'_unchanged cl s s'"
+    and "cl_state (cls s cl) = cl_prepared"
+    and "cl_state (cls s' cl) = cl_committed"
+    and "\<forall>k. is_locked (svr_state (svrs s k) (get_txn_cl cl s))"
+    and "svr_cl_cl'_unchanged cl s s'"
   shows "view_atomic (kvs_of_gs s') (\<lambda>k. full_view (kvs_of_gs s k))"
   using assms
-  apply (auto simp add: kvs_of_gs_def km_tm_cl'_unchanged_def view_atomic_def)
+  apply (auto simp add: kvs_of_gs_def svr_cl_cl'_unchanged_def view_atomic_def)
   subgoal for k k' i i'
     apply (auto elim!: allE[where x=k'])
-    apply (auto simp add: update_kv_all_tm_commit_no_lock_inv read_only_update')
+    apply (auto simp add: update_kv_all_cl_commit_no_lock_inv read_only_update')
      apply (metis full_view_same_length update_kv_reads_all_txn_length)
-    apply (cases "i' \<in> full_view (update_kv_all_txn (\<lambda>t. tm_state (cls s (get_cl_txn t)))
-      (km_state (svrs s k')) (svr_key_fp (svrs s k')) (svr_vl (svrs s k')))"; simp)
+    apply (cases "i' \<in> full_view (update_kv_all_txn (\<lambda>t. cl_state (cls s (get_cl_txn t)))
+      (svr_state (svrs s k')) (svr_key_fp (svrs s k')) (svr_vl (svrs s k')))"; simp)
     using new_version_index[of s cl k' s' i'] apply (auto simp add: writer_update_before)
      apply (simp add: new_writer the_wr_tI)
-    using tm_commit_writer_update_kv_all[of s cl k s'] apply simp
+    using cl_commit_writer_update_kv_all[of s cl k s'] apply simp
     using update_kv_all_txn_v_writer_inv[of i
-        "update_kv_all_txn (\<lambda>t. tm_state (cls s (get_cl_txn t))) (km_state (svrs s k))
+        "update_kv_all_txn (\<lambda>t. cl_state (cls s (get_cl_txn t))) (svr_state (svrs s k))
           (svr_key_fp (svrs s k)) (svr_vl (svrs s k))"] assms(3, 5, 6, 11)
     apply (auto elim!: allE[where x=k])
-    apply (simp_all add: update_kv_all_tm_commit_no_lock_inv)
+    apply (simp_all add: update_kv_all_cl_commit_no_lock_inv)
     by (metis t_is_fresh fresh_txid_v_writer kvs_of_gs_def)+
   done
 
@@ -1789,7 +1798,7 @@ lemma reach_kvs_expands [simp, dest]:
     and "\<And>k. RLockFpInv s k" and "\<And>k. NoLockFpInv s k"
     and "KVSNonEmp s"
   shows "kvs_of_gs s \<sqsubseteq>\<^sub>k\<^sub>v\<^sub>s kvs_of_gs s'"
-  using assms kvs_of_gs_inv[of s e s'] apply (cases "not_tm_commit e"; auto)
+  using assms kvs_of_gs_inv[of s e s'] apply (cases "not_cl_commit e"; auto)
   using kvs_of_gs_view_atomic[of s]
   apply (auto simp add: tps_trans_defs kvs_expands_def vlist_order_def)
   apply (meson kvs_of_gs_commit_length_increasing)
@@ -1817,37 +1826,37 @@ next
   proof (induction e)
     case (WLock x1 x2 x3 x4)
     then show ?case
-      by (auto simp add: KVSView_def tps_trans_defs km_unchanged_defs)
+      by (auto simp add: KVSView_def tps_trans_defs svr_unchanged_defs)
   next
     case (NoLock x1 x2)
     then show ?case
-      by (auto simp add: KVSView_def tps_trans_defs km_unchanged_defs)
+      by (auto simp add: KVSView_def tps_trans_defs svr_unchanged_defs)
   next
     case (User_Commit x)
     then show ?case
-      by (auto simp add: KVSView_def tps_trans_defs tm_unchanged_defs, metis)
+      by (auto simp add: KVSView_def tps_trans_defs cl_unchanged_defs, metis)
   next
-    case (TM_Commit x1 x2 x3 x4)
-    then show ?case
-      apply (auto simp add: KVSView_def tps_trans_defs tm_unchanged_defs)
+    case (Cl_Commit x1 x2 x3 x4)
+    then show ?case using updated_is_kvs_of_gs'[of s' x1 s]
+      apply (auto simp add: KVSView_def tps_trans_defs cl_unchanged_defs o_def)
       apply (cases "cl = x1")
-        apply (simp add: KVSGSNonEmp_def full_view_wellformed)
+      apply (simp add: KVSGSNonEmp_def full_view_wellformed)
       by (smt (verit) kvs_expanded_view_wellformed reach_kvs_expands reach_kvs_non_emp 
           reach_nolockfp reach_rlock reach_rlockfp reach_tidfuturekm reach_tidpastkm
           reach_trans.hyps(1) reach_wlock tps_trans)
   next
-    case (TM_Abort x)
+    case (Cl_Abort x)
     then show ?case
-      by (auto simp add: KVSView_def tps_trans_defs tm_unchanged_defs, metis)
+      by (auto simp add: KVSView_def tps_trans_defs cl_unchanged_defs, metis)
   next
-    case (TM_ReadyC x)
+    case (Cl_ReadyC x)
     then show ?case
-      by (auto simp add: KVSView_def tps_trans_defs tm_unchanged_defs, metis)
+      by (auto simp add: KVSView_def tps_trans_defs cl_unchanged_defs, metis)
   next
-    case (TM_ReadyA x)
+    case (Cl_ReadyA x)
     then show ?case
-      by (auto simp add: KVSView_def tps_trans_defs tm_unchanged_defs, metis)
-  qed (auto simp add: KVSView_def tps_trans_defs km_unchanged_defs)
+      by (auto simp add: KVSView_def tps_trans_defs cl_unchanged_defs, metis)
+  qed (auto simp add: KVSView_def tps_trans_defs svr_unchanged_defs)
 qed
 
 \<comment> \<open>CanCommit\<close>
@@ -1903,20 +1912,21 @@ next
   then show "ET_SER.ET_ES: sim gs\<midarrow>med a\<rightarrow> sim gs'"
   using kvs_of_gs_inv[of gs a gs'] cl_view_inv[of gs a gs']
   proof (induction a)
-  case (TM_Commit cl sn u F)
+  case (Cl_Commit cl sn u F)
   then show ?case using p apply simp
-    apply (auto simp add: tm_commit_def tm_unchanged_defs sim_def)
+    using updated_is_kvs_of_gs'[of gs' cl gs]
+    apply (auto simp add: cl_commit_def cl_unchanged_defs sim_def o_def)
     subgoal apply (rule exI [where x="(\<lambda>k. full_view (kvs_of_gs gs' k))"])
       apply (auto simp add: views_of_gs_def)
       apply (auto simp add: ET_SER.ET_cl_txn_def t_is_fresh KVSGSNonEmp_def full_view_wellformed)
       subgoal by (metis kvs_of_gs_length_increasing full_view_wellformed longer_list_not_empty)
       subgoal by (simp add: full_view_satisfies_ET_SER_canCommit)
       subgoal apply (auto simp add: kvs_of_gs_def update_kv_def) apply (rule ext)
-        using kvs_of_gs_tm_commit[of gs cl] by (simp add: other_insts_unchanged_def)
+        using kvs_of_gs_cl_commit[of gs cl] by (simp add: other_insts_unchanged_def)
       done
     subgoal apply (auto simp add: fp_property_def view_snapshot_def)
       subgoal for k y
-        apply (cases "km_state (svrs gs k) (get_txn_cl cl gs) = no_lock")
+        apply (cases "svr_state (svrs gs k) (get_txn_cl cl gs) = no_lock")
         apply (auto simp add: svr_vl_kvs_eq_lv NoLockFpInv_def del: disjE dest!:or3_not_eq)
           by (metis RLockFpContentInv_def WLockFpContentInv_def option.discI option.inject).
       done
